PREFIX dcterms: <http://purl.org/dc/terms/>
PREFIX rdfs: <http://www.w3.org/2000/01/rdf-schema#>
PREFIX skos: <http://www.w3.org/2004/02/skos/core#>
PREFIX xsd: <http://www.w3.org/2001/XMLSchema#>

<https://linked.data.gov.au/def/test/dawe-cv/05f83f99-1998-4d11-8837-bb4a68788521>
    skos:member <https://linked.data.gov.au/def/test/dawe-cv/ecdcb81a-cbe9-4113-b9e9-422a0e6c751f> ;
.

<https://linked.data.gov.au/def/test/dawe-cv/12ca1c18-7f58-5a4e-a3ef-a6c767de7396>
    a skos:Concept ;
    dcterms:identifier 16 ;
    dcterms:source <http://vocabs.paratoo.tern.org.au:1337/api/lut-soils-texture-grades> ;
    rdfs:isDefinedBy <https://linked.data.gov.au/def/nrm> ;
    skos:definition "N/A" ;
    skos:notation "NA" ;
    skos:prefLabel "Not Applicable" ;
.

<https://linked.data.gov.au/def/test/dawe-cv/1322b4a9-e520-5f40-b563-07a9a7eb7a34>
    a skos:Concept ;
    dcterms:identifier 5 ;
    dcterms:source <http://vocabs.paratoo.tern.org.au:1337/api/lut-soils-texture-grades> ;
    rdfs:isDefinedBy <https://linked.data.gov.au/def/nrm> ;
    skos:definition "Bolus coherent and rather spongy; smooth feel when manipulated but with no obvious sandiness or 'silkiness'; may be somewhat greasy to the touch if organic matter present; will form ribbon of abouot 25mm" ;
    skos:notation "L" ;
    skos:prefLabel "Loam" ;
.

<https://linked.data.gov.au/def/test/dawe-cv/14d592ff-eb3b-584e-9382-ad2e12acf663>
    a skos:Concept ;
    dcterms:identifier 14 ;
    dcterms:source <http://vocabs.paratoo.tern.org.au:1337/api/lut-soils-texture-grades> ;
    rdfs:isDefinedBy <https://linked.data.gov.au/def/nrm> ;
    skos:definition "Coherent smooth bolus; plastic and silky to the touch; will form ribbon of 40-50mm" ;
    skos:notation "ZCL" ;
    skos:prefLabel "Silty clay loam" ;
.

<https://linked.data.gov.au/def/test/dawe-cv/1666ca90-ed29-5238-8fbe-960769f7eaea>
    a skos:Concept ;
    dcterms:identifier 6 ;
    dcterms:source <http://vocabs.paratoo.tern.org.au:1337/api/lut-soils-texture-grades> ;
    rdfs:isDefinedBy <https://linked.data.gov.au/def/nrm> ;
    skos:definition "Plastic bolus; smooth to touch; slight resistance to shearing between thumb and forefinger; will form ribbon of 50-75mm" ;
    skos:notation "LC" ;
    skos:prefLabel "Light clay" ;
.

<https://linked.data.gov.au/def/test/dawe-cv/1af956c2-0bee-5f47-a13c-682ab34e6b70>
    a skos:Concept ;
    dcterms:identifier 9 ;
    dcterms:source <http://vocabs.paratoo.tern.org.au:1337/api/lut-soils-texture-grades> ;
    rdfs:isDefinedBy <https://linked.data.gov.au/def/nrm> ;
    skos:definition "Smooth plastic bolus; handles like plasticine and can be moulded into rods withouot fracture; has some resistance to ribboning shear; will form ribbon of 75mm or more" ;
    skos:notation "MC" ;
    skos:prefLabel "Medium clay" ;
.

<https://linked.data.gov.au/def/test/dawe-cv/2769f26f-8f77-54fd-9dc4-acf1a94f4da7>
    a skos:Concept ;
    dcterms:identifier 15 ;
    dcterms:source <http://vocabs.paratoo.tern.org.au:1337/api/lut-soils-texture-grades> ;
    rdfs:isDefinedBy <https://linked.data.gov.au/def/nrm> ;
    skos:definition "Coherent bolus; very smooth to often silky when manipulated; will form ribbon of about 25mm" ;
    skos:notation "ZL" ;
    skos:prefLabel "Silty loam" ;
.

<https://linked.data.gov.au/def/test/dawe-cv/39952d67-cca5-57d0-87ce-93235e7143b4>
    a skos:Concept ;
    dcterms:identifier 8 ;
    dcterms:source <http://vocabs.paratoo.tern.org.au:1337/api/lut-soils-texture-grades> ;
    rdfs:isDefinedBy <https://linked.data.gov.au/def/nrm> ;
    skos:definition "Slight coherence; sand grains of medium size; can be sheared between thumb and forefinger to give minimal ribbon of about 5mm" ;
    skos:notation "LS" ;
    skos:prefLabel "Loamy sand" ;
.

<https://linked.data.gov.au/def/test/dawe-cv/3b82fa97-54a4-5a47-b084-bdc928b4d632>
    a skos:Concept ;
    dcterms:identifier 4 ;
    dcterms:source <http://vocabs.paratoo.tern.org.au:1337/api/lut-soils-texture-grades> ;
    rdfs:isDefinedBy <https://linked.data.gov.au/def/nrm> ;
    skos:definition "Smooth plastic bolus; handles like stiff plasticine; can be moulded into rods without fracture; has firm resistance to ribboning shear; will form ribbon of 75mm or more" ;
    skos:notation "HC" ;
    skos:prefLabel "Heavy clay" ;
.

<https://linked.data.gov.au/def/test/dawe-cv/492e1076-dd8a-520f-a4ca-d608817b6673>
    a skos:Concept ;
    dcterms:identifier 12 ;
    dcterms:source <http://vocabs.paratoo.tern.org.au:1337/api/lut-soils-texture-grades> ;
    rdfs:isDefinedBy <https://linked.data.gov.au/def/nrm> ;
    skos:definition "Strongly coherent bolus; sandy to touch; medium size sand grains visible in finer matrix; will form ribbon of 25-40mm" ;
    skos:notation "SCL" ;
    skos:prefLabel "Sandy clay loam" ;
.

<https://linked.data.gov.au/def/test/dawe-cv/6d7112f8-d5bb-5266-b511-1439bd40b2a3>
    a skos:Concept ;
    dcterms:identifier 10 ;
    dcterms:source <http://vocabs.paratoo.tern.org.au:1337/api/lut-soils-texture-grades> ;
    rdfs:isDefinedBy <https://linked.data.gov.au/def/nrm> ;
    skos:definition "Smooth plastic bolus; handles like plasticine and can be moulded into rods withouot fracture; has moderate to firm resistance to ribboning shear; will form ribbon of 75mm or more" ;
    skos:notation "MHC" ;
    skos:prefLabel "Medium heavy clay" ;
.

<https://linked.data.gov.au/def/test/dawe-cv/8dad4228-5eca-50c7-889e-77e1af8472a4>
    a skos:Concept ;
    dcterms:identifier 2 ;
    dcterms:source <http://vocabs.paratoo.tern.org.au:1337/api/lut-soils-texture-grades> ;
    rdfs:isDefinedBy <https://linked.data.gov.au/def/nrm> ;
    skos:definition "Coherent plastic bolus; medium sized sand grains visible in the finer matrix; will form ribbon of 40-50mm" ;
    skos:notation "CLS" ;
    skos:prefLabel "Clay loam sandy" ;
.

<https://linked.data.gov.au/def/test/dawe-cv/8e1b9f94-1652-57e2-8aa0-cd612f351b6f>
    a skos:Concept ;
    dcterms:identifier 1 ;
    dcterms:source <http://vocabs.paratoo.tern.org.au:1337/api/lut-soils-texture-grades> ;
    rdfs:isDefinedBy <https://linked.data.gov.au/def/nrm> ;
    skos:definition "Coherent plastic bolus; smooth to manipulate; will form ribbon of 40-50mm" ;
    skos:notation "CL" ;
    skos:prefLabel "Clay loam" ;
.

<https://linked.data.gov.au/def/test/dawe-cv/8edb35c1-0ede-5cba-bc45-61c7175faee1>
    a skos:Concept ;
    dcterms:identifier 3 ;
    dcterms:source <http://vocabs.paratoo.tern.org.au:1337/api/lut-soils-texture-grades> ;
    rdfs:isDefinedBy <https://linked.data.gov.au/def/nrm> ;
    skos:definition "Slight coherence; sand grains of medium size; sticky when wet; many sand grains stick to fingers; will form minimal ribbon of 5-15mm; discolours fingers with clay stain" ;
    skos:notation "CS" ;
    skos:prefLabel "Clayey sand" ;
.

<https://linked.data.gov.au/def/test/dawe-cv/940fabc9-c37a-5e6a-accf-6c209840a329>
    a skos:Concept ;
    dcterms:identifier 13 ;
    dcterms:source <http://vocabs.paratoo.tern.org.au:1337/api/lut-soils-texture-grades> ;
    rdfs:isDefinedBy <https://linked.data.gov.au/def/nrm> ;
    skos:definition "Boluscoherent but very sandy to touch; will form ribbon of 15-25mm; dominant sand grains are of medium size and are readily visible" ;
    skos:notation "SL" ;
    skos:prefLabel "Sandy loam" ;
.

<https://linked.data.gov.au/def/test/dawe-cv/95edbfd3-d894-5e0e-9afc-4ab4265c278b>
    a skos:Concept ;
    dcterms:identifier 7 ;
    dcterms:source <http://vocabs.paratoo.tern.org.au:1337/api/lut-soils-texture-grades> ;
    rdfs:isDefinedBy <https://linked.data.gov.au/def/nrm> ;
    skos:definition "Plastic bolus; smooth to touch; slight to moderate resistance to ribboning shear; will form ribbon of about 75mm" ;
    skos:notation "LMC" ;
    skos:prefLabel "Light medium clay" ;
.

<https://linked.data.gov.au/def/test/dawe-cv/a1f4502b-0ac4-5ca0-871e-7f30216d2fa7>
    a skos:Concept ;
    dcterms:identifier 17 ;
    dcterms:source <http://vocabs.paratoo.tern.org.au:1337/api/lut-soils-texture-grades> ;
    rdfs:isDefinedBy <https://linked.data.gov.au/def/nrm> ;
    skos:definition "N/C" ;
    skos:notation "NC" ;
    skos:prefLabel "Not Collected" ;
.

<https://linked.data.gov.au/def/test/dawe-cv/d09959fd-227e-500d-9fb1-4d6c3cc7c878>
    a skos:Concept ;
    dcterms:identifier 11 ;
    dcterms:source <http://vocabs.paratoo.tern.org.au:1337/api/lut-soils-texture-grades> ;
    rdfs:isDefinedBy <https://linked.data.gov.au/def/nrm> ;
    skos:definition "Coherence nil to very slight; cannot be moulded; sand grains of medium size; single sand grains adhere to fingers" ;
    skos:notation "S" ;
    skos:prefLabel "Sand" ;
.

<https://linked.data.gov.au/def/test/dawe-cv/ecdcb81a-cbe9-4113-b9e9-422a0e6c751f>
    a skos:Collection ;
    dcterms:description "A collection of soils texture grades and its codes." ;
    dcterms:source <http://vocabs.paratoo.tern.org.au:1337/api/lut-soils-texture-grades> ;
    rdfs:isDefinedBy <https://linked.data.gov.au/def/nrm> ;
    skos:member
        <https://linked.data.gov.au/def/test/dawe-cv/12ca1c18-7f58-5a4e-a3ef-a6c767de7396> ,
        <https://linked.data.gov.au/def/test/dawe-cv/1322b4a9-e520-5f40-b563-07a9a7eb7a34> ,
        <https://linked.data.gov.au/def/test/dawe-cv/14d592ff-eb3b-584e-9382-ad2e12acf663> ,
        <https://linked.data.gov.au/def/test/dawe-cv/1666ca90-ed29-5238-8fbe-960769f7eaea> ,
        <https://linked.data.gov.au/def/test/dawe-cv/1af956c2-0bee-5f47-a13c-682ab34e6b70> ,
        <https://linked.data.gov.au/def/test/dawe-cv/2769f26f-8f77-54fd-9dc4-acf1a94f4da7> ,
        <https://linked.data.gov.au/def/test/dawe-cv/39952d67-cca5-57d0-87ce-93235e7143b4> ,
        <https://linked.data.gov.au/def/test/dawe-cv/3b82fa97-54a4-5a47-b084-bdc928b4d632> ,
        <https://linked.data.gov.au/def/test/dawe-cv/492e1076-dd8a-520f-a4ca-d608817b6673> ,
        <https://linked.data.gov.au/def/test/dawe-cv/6d7112f8-d5bb-5266-b511-1439bd40b2a3> ,
        <https://linked.data.gov.au/def/test/dawe-cv/8dad4228-5eca-50c7-889e-77e1af8472a4> ,
        <https://linked.data.gov.au/def/test/dawe-cv/8e1b9f94-1652-57e2-8aa0-cd612f351b6f> ,
        <https://linked.data.gov.au/def/test/dawe-cv/8edb35c1-0ede-5cba-bc45-61c7175faee1> ,
        <https://linked.data.gov.au/def/test/dawe-cv/940fabc9-c37a-5e6a-accf-6c209840a329> ,
        <https://linked.data.gov.au/def/test/dawe-cv/95edbfd3-d894-5e0e-9afc-4ab4265c278b> ,
        <https://linked.data.gov.au/def/test/dawe-cv/a1f4502b-0ac4-5ca0-871e-7f30216d2fa7> ,
        <https://linked.data.gov.au/def/test/dawe-cv/d09959fd-227e-500d-9fb1-4d6c3cc7c878> ;
    skos:prefLabel "Soils texture grades codes" ;
.

