PREFIX dcterms: <http://purl.org/dc/terms/>
PREFIX rdfs: <http://www.w3.org/2000/01/rdf-schema#>
PREFIX skos: <http://www.w3.org/2004/02/skos/core#>
PREFIX xsd: <http://www.w3.org/2001/XMLSchema#>

<https://linked.data.gov.au/def/test/dawe-cv/05f83f99-1998-4d11-8837-bb4a68788521>
    skos:member <https://linked.data.gov.au/def/test/dawe-cv/0c9132dc-48bf-4a9c-ac9b-0c8b1909afb4> ;
.

<https://linked.data.gov.au/def/test/dawe-cv/0c9132dc-48bf-4a9c-ac9b-0c8b1909afb4>
    a skos:Collection ;
    dcterms:description "A collection of soils drainages and its codes." ;
    dcterms:source <http://vocabs.paratoo.tern.org.au:1337/api/lut-soils-drainages> ;
    rdfs:isDefinedBy <https://linked.data.gov.au/def/nrm> ;
    skos:member
        <https://linked.data.gov.au/def/test/dawe-cv/16413e7c-aadb-5dc0-8f3d-2425e96bde1a> ,
        <https://linked.data.gov.au/def/test/dawe-cv/1a9ca7de-5132-52d4-9fe7-1790c67b640d> ,
        <https://linked.data.gov.au/def/test/dawe-cv/1b51cddb-77f5-56c7-b60c-530eb3502659> ,
        <https://linked.data.gov.au/def/test/dawe-cv/a7cec71c-08d2-559f-a676-8394a7626c8a> ,
        <https://linked.data.gov.au/def/test/dawe-cv/b8ab5000-f630-5bc1-9588-6b960cb69bba> ,
        <https://linked.data.gov.au/def/test/dawe-cv/eaba5c88-9350-5375-86d3-d94ad431b394> ,
        <https://linked.data.gov.au/def/test/dawe-cv/fb373e61-c02f-5305-980e-be9ff1eac488> ;
    skos:prefLabel "Soils drainages codes" ;
.

<https://linked.data.gov.au/def/test/dawe-cv/16413e7c-aadb-5dc0-8f3d-2425e96bde1a>
    a skos:Concept ;
    dcterms:identifier 3 ;
    dcterms:source <http://vocabs.paratoo.tern.org.au:1337/api/lut-soils-drainages> ;
    rdfs:isDefinedBy <https://linked.data.gov.au/def/nrm> ;
    skos:definition "Water is removed on slowly in relation to supply. Precipitation is the main source if available water storage capacity is high; but surface subflow and/or groundwater contribute as available water storage capacity decreases. Soils have a wide range in texture and depth. Some horizons may be mottled and/or have orange or rusty linings of root channels; and are wet for several weeks." ;
    skos:notation "3" ;
    skos:prefLabel "Imperfect" ;
.

<https://linked.data.gov.au/def/test/dawe-cv/1a9ca7de-5132-52d4-9fe7-1790c67b640d>
    a skos:Concept ;
    dcterms:identifier 7 ;
    dcterms:source <http://vocabs.paratoo.tern.org.au:1337/api/lut-soils-drainages> ;
    rdfs:isDefinedBy <https://linked.data.gov.au/def/nrm> ;
    skos:definition "" ;
    skos:notation "7" ;
    skos:prefLabel "Not Collected" ;
.

<https://linked.data.gov.au/def/test/dawe-cv/1b51cddb-77f5-56c7-b60c-530eb3502659>
    a skos:Concept ;
    dcterms:identifier 4 ;
    dcterms:source <http://vocabs.paratoo.tern.org.au:1337/api/lut-soils-drainages> ;
    rdfs:isDefinedBy <https://linked.data.gov.au/def/nrm> ;
    skos:definition "Water is removed from the soil somewhat slowly in relation to supply; due to low permeability; shallow watertable; lack of gradient; or some combination of these. Soils are usually medium to fine in texture. Significant additions of water by subsurface flow are necessary in coarse-textured soil. Some horizons may remain wet for as long as one week after water addition." ;
    skos:notation "4" ;
    skos:prefLabel "Moderately well" ;
.

<https://linked.data.gov.au/def/test/dawe-cv/a7cec71c-08d2-559f-a676-8394a7626c8a>
    a skos:Concept ;
    dcterms:identifier 6 ;
    dcterms:source <http://vocabs.paratoo.tern.org.au:1337/api/lut-soils-drainages> ;
    rdfs:isDefinedBy <https://linked.data.gov.au/def/nrm> ;
    skos:definition "Water is removed from the soil rapidly in relation to supply. Excess water flows downward rapidly if underlying material is highly permeable. There may be rapid subsurface lateral flow during heavy rainfall provided there is a steep gradient. Soils are usually coarse-textured; or shallow; or both. No horizon is normally wet for more than several hours after water addition." ;
    skos:notation "6" ;
    skos:prefLabel "Rapid" ;
.

<https://linked.data.gov.au/def/test/dawe-cv/b8ab5000-f630-5bc1-9588-6b960cb69bba>
    a skos:Concept ;
    dcterms:identifier 1 ;
    dcterms:source <http://vocabs.paratoo.tern.org.au:1337/api/lut-soils-drainages> ;
    rdfs:isDefinedBy <https://linked.data.gov.au/def/nrm> ;
    skos:definition "Water is removed from the soil so slowly that the watertable remains at or near the surface for most of the year. Surface flow; groundwater and subsurface flow are major sources of water; although precipitation may be important where there is a perched watertable and precipitation exceeds evapotranspiration. Soils have a wide range in texture and depth; and often occur in depressed sites. Strong gleying and accumulation of surface organic matter are usually features of most soils." ;
    skos:notation "1" ;
    skos:prefLabel "Very poor" ;
.

<https://linked.data.gov.au/def/test/dawe-cv/eaba5c88-9350-5375-86d3-d94ad431b394>
    a skos:Concept ;
    dcterms:identifier 5 ;
    dcterms:source <http://vocabs.paratoo.tern.org.au:1337/api/lut-soils-drainages> ;
    rdfs:isDefinedBy <https://linked.data.gov.au/def/nrm> ;
    skos:definition "Water is removed from the soil readily but not rapidly. Excess water flows downward readily into underlying; moderately permeable material or laterally as subsurface flow. The soils are often medium in texture. Some horizons may remain wet for several days after water addition." ;
    skos:notation "5" ;
    skos:prefLabel "Well" ;
.

<https://linked.data.gov.au/def/test/dawe-cv/fb373e61-c02f-5305-980e-be9ff1eac488>
    a skos:Concept ;
    dcterms:identifier 2 ;
    dcterms:source <http://vocabs.paratoo.tern.org.au:1337/api/lut-soils-drainages> ;
    rdfs:isDefinedBy <https://linked.data.gov.au/def/nrm> ;
    skos:definition "Water is removed very slowly in relation to supply. Subsurface and/or groundwater flow; as well as precipitation; may be a significant water source. Seasonal ponding; resulting from runon and insufficient outfall; also occurs.  A perched watertable may be present. Soils have a wide range in texture and depth; many have horizons that are gleyed; mottled; or possess orange or rusty linings of root channels. All horizons remain wet for several months." ;
    skos:notation "2" ;
    skos:prefLabel "Poor" ;
.

