PREFIX dcterms: <http://purl.org/dc/terms/>
PREFIX rdfs: <http://www.w3.org/2000/01/rdf-schema#>
PREFIX schema: <https://schema.org/>
PREFIX skos: <http://www.w3.org/2004/02/skos/core#>
PREFIX xsd: <http://www.w3.org/2001/XMLSchema#>

<https://linked.data.gov.au/def/test/dawe-cv/b7066d4c-2d7b-4c1b-a8f2-401fd243ac3f>
    a skos:Collection ;
    dcterms:description "A collection of condition growth stage shrubs and its codes." ;
    dcterms:source <http://vocabs.paratoo.tern.org.au:1337/api/lut-condition-growth-stage-shrubs> ;
    rdfs:isDefinedBy <https://linked.data.gov.au/def/nrm> ;
    skos:member
        <https://linked.data.gov.au/def/test/dawe-cv/03057fd7-9f6f-5508-ab25-35181e6723eb> ,
        <https://linked.data.gov.au/def/test/dawe-cv/3e36c813-9ab0-5e22-bc92-e6c93c725e9e> ,
        <https://linked.data.gov.au/def/test/dawe-cv/a147d195-7b46-538f-ad4f-69ca719c6c50> ,
        <https://linked.data.gov.au/def/test/dawe-cv/b0b50ba6-d367-582d-8175-60eee47b7f6f> ,
        <https://linked.data.gov.au/def/test/dawe-cv/c9e1d86d-f174-593d-bcd3-d8718830edf5> ;
    skos:prefLabel "Condition growth stage shrubs codes" ;
    schema:url "https://github.com/ternaustralia/dawe-rlp-vocabs/tree/main/vocab_files/categorical_collections/luts/condition-growth-stage-shrubs.ttl"^^xsd:anyURI ;
.

<https://linked.data.gov.au/def/test/dawe-cv/03057fd7-9f6f-5508-ab25-35181e6723eb>
    a skos:Concept ;
    dcterms:identifier 4 ;
    dcterms:source <http://vocabs.paratoo.tern.org.au:1337/api/lut-condition-growth-stage-shrubs> ;
    rdfs:isDefinedBy <https://linked.data.gov.au/def/nrm> ;
    skos:definition "Crown form contracting and decrease in crown diameter and crown leaf area. Dead branches more common â€“ approx. >80 years" ;
    skos:notation "S" ;
    skos:prefLabel "Senescent" ;
    schema:url "https://github.com/ternaustralia/dawe-rlp-vocabs/tree/main/vocab_files/categorical_collections/luts/condition-growth-stage-shrubs.ttl"^^xsd:anyURI ;
.

<https://linked.data.gov.au/def/test/dawe-cv/3e36c813-9ab0-5e22-bc92-e6c93c725e9e>
    a skos:Concept ;
    dcterms:identifier 1 ;
    dcterms:source <http://vocabs.paratoo.tern.org.au:1337/api/lut-condition-growth-stage-shrubs> ;
    rdfs:isDefinedBy <https://linked.data.gov.au/def/nrm> ;
    skos:definition "Juvenile stage, shrub has not reached maximum height, apical dominance." ;
    skos:notation "RC" ;
    skos:prefLabel "Recruiting" ;
    schema:url "https://github.com/ternaustralia/dawe-rlp-vocabs/tree/main/vocab_files/categorical_collections/luts/condition-growth-stage-shrubs.ttl"^^xsd:anyURI ;
.

<https://linked.data.gov.au/def/test/dawe-cv/a147d195-7b46-538f-ad4f-69ca719c6c50>
    a skos:Concept ;
    dcterms:identifier 5 ;
    dcterms:source <http://vocabs.paratoo.tern.org.au:1337/api/lut-condition-growth-stage-shrubs> ;
    rdfs:isDefinedBy <https://linked.data.gov.au/def/nrm> ;
    skos:definition "Dead individuals in all stages." ;
    skos:notation "D" ;
    skos:prefLabel "Dead" ;
    schema:url "https://github.com/ternaustralia/dawe-rlp-vocabs/tree/main/vocab_files/categorical_collections/luts/condition-growth-stage-shrubs.ttl"^^xsd:anyURI ;
.

<https://linked.data.gov.au/def/test/dawe-cv/b0b50ba6-d367-582d-8175-60eee47b7f6f>
    a skos:Concept ;
    dcterms:identifier 3 ;
    dcterms:source <http://vocabs.paratoo.tern.org.au:1337/api/lut-condition-growth-stage-shrubs> ;
    rdfs:isDefinedBy <https://linked.data.gov.au/def/nrm> ;
    skos:definition "Shrub has reached maximum height, crown has reached full lateral development." ;
    skos:notation "M" ;
    skos:prefLabel "Mature" ;
    schema:url "https://github.com/ternaustralia/dawe-rlp-vocabs/tree/main/vocab_files/categorical_collections/luts/condition-growth-stage-shrubs.ttl"^^xsd:anyURI ;
.

<https://linked.data.gov.au/def/test/dawe-cv/c9e1d86d-f174-593d-bcd3-d8718830edf5>
    a skos:Concept ;
    dcterms:identifier 2 ;
    dcterms:source <http://vocabs.paratoo.tern.org.au:1337/api/lut-condition-growth-stage-shrubs> ;
    rdfs:isDefinedBy <https://linked.data.gov.au/def/nrm> ;
    skos:definition "Woody perennial which is resprouting after significant loss of foliage." ;
    skos:notation "RS" ;
    skos:prefLabel "Resprouting" ;
    schema:url "https://github.com/ternaustralia/dawe-rlp-vocabs/tree/main/vocab_files/categorical_collections/luts/condition-growth-stage-shrubs.ttl"^^xsd:anyURI ;
.

