PREFIX dcterms: <http://purl.org/dc/terms/>
PREFIX rdfs: <http://www.w3.org/2000/01/rdf-schema#>
PREFIX schema: <https://schema.org/>
PREFIX skos: <http://www.w3.org/2004/02/skos/core#>
PREFIX xsd: <http://www.w3.org/2001/XMLSchema#>

<https://linked.data.gov.au/def/test/dawe-cv/c7a0692c-113c-4593-ae04-5e49aba70fdf>
    a skos:Collection ;
    dcterms:description "A collection of fire substrate types and its codes." ;
    dcterms:source <http://vocabs.paratoo.tern.org.au:1337/api/lut-fire-substrate-types> ;
    rdfs:isDefinedBy <https://linked.data.gov.au/def/nrm> ;
    skos:member
        <https://linked.data.gov.au/def/test/dawe-cv/91ab6f7c-1118-5f30-92ba-af59b5a60021> ,
        <https://linked.data.gov.au/def/test/dawe-cv/a2749e44-e95b-56c4-9fbc-16fb3c36dd1f> ,
        <https://linked.data.gov.au/def/test/dawe-cv/b489fc69-ae73-505a-8ca2-c6af1eb7bb5d> ,
        <https://linked.data.gov.au/def/test/dawe-cv/c423223e-0bf3-5fdb-bf15-70ecf31d80d2> ,
        <https://linked.data.gov.au/def/test/dawe-cv/eb2d2c73-3422-5534-93f7-168bb2d74969> ;
    skos:prefLabel "Fire substrate types codes" ;
    schema:url "https://github.com/ternaustralia/dawe-rlp-vocabs/tree/main/vocab_files/categorical_collections/luts/fire-substrate.ttl" ;
.

<https://linked.data.gov.au/def/test/dawe-cv/91ab6f7c-1118-5f30-92ba-af59b5a60021>
    a skos:Concept ;
    dcterms:identifier 3 ;
    dcterms:source <http://vocabs.paratoo.tern.org.au:1337/api/lut-fire-substrate-types> ;
    rdfs:isDefinedBy <https://linked.data.gov.au/def/nrm> ;
    skos:definition "Coarse Woody Debris â€“ detached wood with >10 cm diameter at the intercept point. Can be marked as charred." ;
    skos:notation "CWD" ;
    skos:prefLabel "Coarse Woody Debris" ;
    schema:url "https://github.com/ternaustralia/dawe-rlp-vocabs/tree/main/vocab_files/categorical_collections/luts/fire-substrate.ttl" ;
.

<https://linked.data.gov.au/def/test/dawe-cv/a2749e44-e95b-56c4-9fbc-16fb3c36dd1f>
    a skos:Concept ;
    dcterms:identifier 4 ;
    dcterms:source <http://vocabs.paratoo.tern.org.au:1337/api/lut-fire-substrate-types> ;
    rdfs:isDefinedBy <https://linked.data.gov.au/def/nrm> ;
    skos:definition "Powdery black residue remaining after the incomplete combustion of wood during a bushfire." ;
    skos:notation "BA" ;
    skos:prefLabel "Black ash" ;
    schema:url "https://github.com/ternaustralia/dawe-rlp-vocabs/tree/main/vocab_files/categorical_collections/luts/fire-substrate.ttl" ;
.

<https://linked.data.gov.au/def/test/dawe-cv/b489fc69-ae73-505a-8ca2-c6af1eb7bb5d>
    a skos:Concept ;
    dcterms:identifier 2 ;
    dcterms:source <http://vocabs.paratoo.tern.org.au:1337/api/lut-fire-substrate-types> ;
    rdfs:isDefinedBy <https://linked.data.gov.au/def/nrm> ;
    skos:definition "Dead vegetation not attached or identifiable; if litter is attached and identifiable as a species, it should be recorded as this species but flagged as being dead. Can be marked as charred." ;
    skos:notation "LT" ;
    skos:prefLabel "Litter" ;
    schema:url "https://github.com/ternaustralia/dawe-rlp-vocabs/tree/main/vocab_files/categorical_collections/luts/fire-substrate.ttl" ;
.

<https://linked.data.gov.au/def/test/dawe-cv/c423223e-0bf3-5fdb-bf15-70ecf31d80d2>
    a skos:Concept ;
    dcterms:identifier 5 ;
    dcterms:source <http://vocabs.paratoo.tern.org.au:1337/api/lut-fire-substrate-types> ;
    rdfs:isDefinedBy <https://linked.data.gov.au/def/nrm> ;
    skos:definition "Powdery white residue remaining after the complete combustion of wood during a bushfire." ;
    skos:notation "WA" ;
    skos:prefLabel "White ash" ;
    schema:url "https://github.com/ternaustralia/dawe-rlp-vocabs/tree/main/vocab_files/categorical_collections/luts/fire-substrate.ttl" ;
.

<https://linked.data.gov.au/def/test/dawe-cv/eb2d2c73-3422-5534-93f7-168bb2d74969>
    a skos:Concept ;
    dcterms:identifier 1 ;
    dcterms:source <http://vocabs.paratoo.tern.org.au:1337/api/lut-fire-substrate-types> ;
    rdfs:isDefinedBy <https://linked.data.gov.au/def/nrm> ;
    skos:definition "Bare soil. Can be marked as charred." ;
    skos:notation "BR" ;
    skos:prefLabel "Bare" ;
    schema:url "https://github.com/ternaustralia/dawe-rlp-vocabs/tree/main/vocab_files/categorical_collections/luts/fire-substrate.ttl" ;
.

