PREFIX dcterms: <http://purl.org/dc/terms/>
PREFIX rdfs: <http://www.w3.org/2000/01/rdf-schema#>
PREFIX schema: <https://schema.org/>
PREFIX skos: <http://www.w3.org/2004/02/skos/core#>
PREFIX xsd: <http://www.w3.org/2001/XMLSchema#>

<https://linked.data.gov.au/def/test/dawe-cv/032ed6fa-4c55-4752-b625-3e6b32672444>
    a skos:Collection ;
    dcterms:description "A collection of fire growth forms and its codes." ;
    dcterms:source <http://vocabs.paratoo.tern.org.au:1337/api/lut-fire-growth-forms> ;
    rdfs:isDefinedBy <https://linked.data.gov.au/def/nrm> ;
    skos:member
        <https://linked.data.gov.au/def/test/dawe-cv/052ecd8e-298a-5082-a9c2-9d8c32588550> ,
        <https://linked.data.gov.au/def/test/dawe-cv/2919939d-d65f-52ef-a064-9f53829e7b9f> ,
        <https://linked.data.gov.au/def/test/dawe-cv/2a83901c-55fe-53e1-999a-720a7157797d> ,
        <https://linked.data.gov.au/def/test/dawe-cv/3eda0751-2618-512a-9bb3-c638c2146ab7> ,
        <https://linked.data.gov.au/def/test/dawe-cv/41cc7acf-27a8-5987-af68-9b477b57b28d> ,
        <https://linked.data.gov.au/def/test/dawe-cv/4545603c-30a2-5a78-aace-f0e33fabaebc> ,
        <https://linked.data.gov.au/def/test/dawe-cv/4dccc82f-8f78-5106-bc18-d7a22216e858> ,
        <https://linked.data.gov.au/def/test/dawe-cv/51b83cb8-61ca-5f4d-87d5-5ebb98493985> ,
        <https://linked.data.gov.au/def/test/dawe-cv/51eec2ab-909e-575c-8a5d-3e1ce801a000> ,
        <https://linked.data.gov.au/def/test/dawe-cv/6d4fdc25-35ab-56d0-ae0f-01e0efb1df95> ,
        <https://linked.data.gov.au/def/test/dawe-cv/6dd41f76-6edc-518e-be65-19fde731e748> ,
        <https://linked.data.gov.au/def/test/dawe-cv/767e711f-b6ed-531f-b48c-ae3a24211e34> ,
        <https://linked.data.gov.au/def/test/dawe-cv/7bc7f3fe-9e53-5a3b-97b9-27f983f302b1> ,
        <https://linked.data.gov.au/def/test/dawe-cv/7cb044f6-1975-53e6-8378-22b506429ccc> ,
        <https://linked.data.gov.au/def/test/dawe-cv/849a5ac6-2769-5f19-b05b-fdaeda4a88a4> ,
        <https://linked.data.gov.au/def/test/dawe-cv/93180d7c-0203-5b2f-a622-e977fd8deef0> ,
        <https://linked.data.gov.au/def/test/dawe-cv/93835815-2750-599d-b63a-494699ac8802> ,
        <https://linked.data.gov.au/def/test/dawe-cv/a97240fa-ad87-55d1-b4ed-2889fc7d5637> ,
        <https://linked.data.gov.au/def/test/dawe-cv/ac2c4f2d-2e96-590f-ab4c-b6cb39f4c9df> ,
        <https://linked.data.gov.au/def/test/dawe-cv/af735a8f-0adf-505f-a15a-cd4c95e8ef6f> ,
        <https://linked.data.gov.au/def/test/dawe-cv/b6900225-7940-5f7b-96f8-721f653dd1ba> ,
        <https://linked.data.gov.au/def/test/dawe-cv/b772fc98-c494-50c4-8a4a-876c38c362cd> ,
        <https://linked.data.gov.au/def/test/dawe-cv/c801b65c-80fd-5d1a-b0a7-f38f964732db> ,
        <https://linked.data.gov.au/def/test/dawe-cv/ddecfd49-5e0b-5684-8147-dcb798710c7c> ,
        <https://linked.data.gov.au/def/test/dawe-cv/f6ee4df7-f138-55e2-a1fd-4f93bee18a9e> ,
        <https://linked.data.gov.au/def/test/dawe-cv/fa1f7cef-6c5a-5487-83cb-f8700b0f67e5> ;
    skos:prefLabel "Fire growth forms codes" ;
    schema:url "https://github.com/ternaustralia/dawe-rlp-vocabs/tree/main/vocab_files/categorical_collections/luts/fire-growth-forms.ttl"^^xsd:anyURI ;
.

<https://linked.data.gov.au/def/test/dawe-cv/052ecd8e-298a-5082-a9c2-9d8c32588550>
    a skos:Concept ;
    dcterms:identifier 26 ;
    dcterms:source <http://vocabs.paratoo.tern.org.au:1337/api/lut-fire-growth-forms> ;
    rdfs:isDefinedBy <https://linked.data.gov.au/def/nrm> ;
    skos:definition "Unknown." ;
    skos:notation "U" ;
    skos:prefLabel "Unknown" ;
    schema:url "https://github.com/ternaustralia/dawe-rlp-vocabs/tree/main/vocab_files/categorical_collections/luts/fire-growth-forms.ttl"^^xsd:anyURI ;
.

<https://linked.data.gov.au/def/test/dawe-cv/2919939d-d65f-52ef-a064-9f53829e7b9f>
    a skos:Concept ;
    dcterms:identifier 8 ;
    dcterms:source <http://vocabs.paratoo.tern.org.au:1337/api/lut-fire-growth-forms> ;
    rdfs:isDefinedBy <https://linked.data.gov.au/def/nrm> ;
    skos:definition "Grass forming discrete but open tussocks usually with distinct individual shoots, or if not, then forming a hummock. These are the common agricultural grasses." ;
    skos:notation "TG" ;
    skos:prefLabel "Tussock Grass" ;
    schema:url "https://github.com/ternaustralia/dawe-rlp-vocabs/tree/main/vocab_files/categorical_collections/luts/fire-growth-forms.ttl"^^xsd:anyURI ;
.

<https://linked.data.gov.au/def/test/dawe-cv/2a83901c-55fe-53e1-999a-720a7157797d>
    a skos:Concept ;
    dcterms:identifier 6 ;
    dcterms:source <http://vocabs.paratoo.tern.org.au:1337/api/lut-fire-growth-forms> ;
    rdfs:isDefinedBy <https://linked.data.gov.au/def/nrm> ;
    skos:definition "Single or multi-stemmed, semi-succulent shrub of the family Chenopodiaceae exhibiting drought and salt tolerance." ;
    skos:notation "CS" ;
    skos:prefLabel "Chenopod Shrub" ;
    schema:url "https://github.com/ternaustralia/dawe-rlp-vocabs/tree/main/vocab_files/categorical_collections/luts/fire-growth-forms.ttl"^^xsd:anyURI ;
.

<https://linked.data.gov.au/def/test/dawe-cv/3eda0751-2618-512a-9bb3-c638c2146ab7>
    a skos:Concept ;
    dcterms:identifier 10 ;
    dcterms:source <http://vocabs.paratoo.tern.org.au:1337/api/lut-fire-growth-forms> ;
    rdfs:isDefinedBy <https://linked.data.gov.au/def/nrm> ;
    skos:definition "Member of the family Poaceae, but having neither a distinctive tussock nor hummock appearance. Examples include stoloniferous species such as Cynodon dactylon." ;
    skos:notation "OG" ;
    skos:prefLabel "Other Grass" ;
    schema:url "https://github.com/ternaustralia/dawe-rlp-vocabs/tree/main/vocab_files/categorical_collections/luts/fire-growth-forms.ttl"^^xsd:anyURI ;
.

<https://linked.data.gov.au/def/test/dawe-cv/41cc7acf-27a8-5987-af68-9b477b57b28d>
    a skos:Concept ;
    dcterms:identifier 22 ;
    dcterms:source <http://vocabs.paratoo.tern.org.au:1337/api/lut-fire-growth-forms> ;
    rdfs:isDefinedBy <https://linked.data.gov.au/def/nrm> ;
    skos:definition "Members of the families Cycadaceae and Zamiaceae." ;
    skos:notation "C" ;
    skos:prefLabel "Cycad" ;
    schema:url "https://github.com/ternaustralia/dawe-rlp-vocabs/tree/main/vocab_files/categorical_collections/luts/fire-growth-forms.ttl"^^xsd:anyURI ;
.

<https://linked.data.gov.au/def/test/dawe-cv/4545603c-30a2-5a78-aace-f0e33fabaebc>
    a skos:Concept ;
    dcterms:identifier 20 ;
    dcterms:source <http://vocabs.paratoo.tern.org.au:1337/api/lut-fire-growth-forms> ;
    rdfs:isDefinedBy <https://linked.data.gov.au/def/nrm> ;
    skos:definition "Palms and other arborescent monocotyledons. Members of the Arecaceae family or the genus Pandanus. (Pandanus is often multi-stemmed)." ;
    skos:notation "P" ;
    skos:prefLabel "Palm" ;
    schema:url "https://github.com/ternaustralia/dawe-rlp-vocabs/tree/main/vocab_files/categorical_collections/luts/fire-growth-forms.ttl"^^xsd:anyURI ;
.

<https://linked.data.gov.au/def/test/dawe-cv/4dccc82f-8f78-5106-bc18-d7a22216e858>
    a skos:Concept ;
    dcterms:identifier 5 ;
    dcterms:source <http://vocabs.paratoo.tern.org.au:1337/api/lut-fire-growth-forms> ;
    rdfs:isDefinedBy <https://linked.data.gov.au/def/nrm> ;
    skos:definition "Shrub usually less than 2 m, with sclerophyllous leaves having high fibre:protein ratios and with an area of nanophyll or smaller (less than 225 mm2). Often a member of one the following families: Ericaceae, Myrtaceae, Fabaceae and Proteaceae. Commonly occur on nutrient-poor substrates." ;
    skos:notation "HS" ;
    skos:prefLabel "Health Shrub" ;
    schema:url "https://github.com/ternaustralia/dawe-rlp-vocabs/tree/main/vocab_files/categorical_collections/luts/fire-growth-forms.ttl"^^xsd:anyURI ;
.

<https://linked.data.gov.au/def/test/dawe-cv/51b83cb8-61ca-5f4d-87d5-5ebb98493985>
    a skos:Concept ;
    dcterms:identifier 19 ;
    dcterms:source <http://vocabs.paratoo.tern.org.au:1337/api/lut-fire-growth-forms> ;
    rdfs:isDefinedBy <https://linked.data.gov.au/def/nrm> ;
    skos:definition "Climbing, twining, winding or sprawling plants usually with a woody stem." ;
    skos:notation "V" ;
    skos:prefLabel "Vine" ;
    schema:url "https://github.com/ternaustralia/dawe-rlp-vocabs/tree/main/vocab_files/categorical_collections/luts/fire-growth-forms.ttl"^^xsd:anyURI ;
.

<https://linked.data.gov.au/def/test/dawe-cv/51eec2ab-909e-575c-8a5d-3e1ce801a000>
    a skos:Concept ;
    dcterms:identifier 17 ;
    dcterms:source <http://vocabs.paratoo.tern.org.au:1337/api/lut-fire-growth-forms> ;
    rdfs:isDefinedBy <https://linked.data.gov.au/def/nrm> ;
    skos:definition "Composite plant consisting of a fungus living symbiotically with algae; without true roots, stems or leaves." ;
    skos:notation "L" ;
    skos:prefLabel "Lichen" ;
    schema:url "https://github.com/ternaustralia/dawe-rlp-vocabs/tree/main/vocab_files/categorical_collections/luts/fire-growth-forms.ttl"^^xsd:anyURI ;
.

<https://linked.data.gov.au/def/test/dawe-cv/6d4fdc25-35ab-56d0-ae0f-01e0efb1df95>
    a skos:Concept ;
    dcterms:identifier 23 ;
    dcterms:source <http://vocabs.paratoo.tern.org.au:1337/api/lut-fire-growth-forms> ;
    rdfs:isDefinedBy <https://linked.data.gov.au/def/nrm> ;
    skos:definition "Flowering angiosperms forming sparse to dense mats of material at the subtidal and down to 30 m below MSL. Occasionally exposed." ;
    skos:notation "SG" ;
    skos:prefLabel "Seagrass" ;
    schema:url "https://github.com/ternaustralia/dawe-rlp-vocabs/tree/main/vocab_files/categorical_collections/luts/fire-growth-forms.ttl"^^xsd:anyURI ;
.

<https://linked.data.gov.au/def/test/dawe-cv/6dd41f76-6edc-518e-be65-19fde731e748>
    a skos:Concept ;
    dcterms:identifier 16 ;
    dcterms:source <http://vocabs.paratoo.tern.org.au:1337/api/lut-fire-growth-forms> ;
    rdfs:isDefinedBy <https://linked.data.gov.au/def/nrm> ;
    skos:definition "Mosses and Liverworts. Mosses are small plants usually with a slender leafbearing stem with no true vascular tissue. Liverworts are often moss-like in appearance or consisting of a flat, ribbon-like green thallus." ;
    skos:notation "B" ;
    skos:prefLabel "Bryophyte" ;
    schema:url "https://github.com/ternaustralia/dawe-rlp-vocabs/tree/main/vocab_files/categorical_collections/luts/fire-growth-forms.ttl"^^xsd:anyURI ;
.

<https://linked.data.gov.au/def/test/dawe-cv/767e711f-b6ed-531f-b48c-ae3a24211e34>
    a skos:Concept ;
    dcterms:identifier 13 ;
    dcterms:source <http://vocabs.paratoo.tern.org.au:1337/api/lut-fire-growth-forms> ;
    rdfs:isDefinedBy <https://linked.data.gov.au/def/nrm> ;
    skos:definition "Herbaceous or slightly woody, annual or sometimes perennial plant. (Usually a dicotyledon)." ;
    skos:notation "F" ;
    skos:prefLabel "Forb" ;
    schema:url "https://github.com/ternaustralia/dawe-rlp-vocabs/tree/main/vocab_files/categorical_collections/luts/fire-growth-forms.ttl"^^xsd:anyURI ;
.

<https://linked.data.gov.au/def/test/dawe-cv/7bc7f3fe-9e53-5a3b-97b9-27f983f302b1>
    a skos:Concept ;
    dcterms:identifier 2 ;
    dcterms:source <http://vocabs.paratoo.tern.org.au:1337/api/lut-fire-growth-forms> ;
    rdfs:isDefinedBy <https://linked.data.gov.au/def/nrm> ;
    skos:definition "Woody perennial plant usually of the genus Eucalyptus. Multi-stemmed with fewer than five trunks of which at least three exceed 100 mm diameter at breast height (1.3 m). Usually 8 m or more." ;
    skos:notation "TM" ;
    skos:prefLabel "Tree Mallee" ;
    schema:url "https://github.com/ternaustralia/dawe-rlp-vocabs/tree/main/vocab_files/categorical_collections/luts/fire-growth-forms.ttl"^^xsd:anyURI ;
.

<https://linked.data.gov.au/def/test/dawe-cv/7cb044f6-1975-53e6-8378-22b506429ccc>
    a skos:Concept ;
    dcterms:identifier 11 ;
    dcterms:source <http://vocabs.paratoo.tern.org.au:1337/api/lut-fire-growth-forms> ;
    rdfs:isDefinedBy <https://linked.data.gov.au/def/nrm> ;
    skos:definition "Herbaceous, usually perennial erect plant generally with a tufted habit and of the families Cyperaceae (true sedges) or Restionaceae (node sedges)." ;
    skos:notation "SE" ;
    skos:prefLabel "Sedge" ;
    schema:url "https://github.com/ternaustralia/dawe-rlp-vocabs/tree/main/vocab_files/categorical_collections/luts/fire-growth-forms.ttl"^^xsd:anyURI ;
.

<https://linked.data.gov.au/def/test/dawe-cv/849a5ac6-2769-5f19-b05b-fdaeda4a88a4>
    a skos:Concept ;
    dcterms:identifier 18 ;
    dcterms:source <http://vocabs.paratoo.tern.org.au:1337/api/lut-fire-growth-forms> ;
    rdfs:isDefinedBy <https://linked.data.gov.au/def/nrm> ;
    skos:definition "Epiphytes, mistletoes and parasites. Plant with roots attached to the aerial portions of other plants. Can often be another growth form, such as fern or forb." ;
    skos:notation "E" ;
    skos:prefLabel "Epiphyte" ;
    schema:url "https://github.com/ternaustralia/dawe-rlp-vocabs/tree/main/vocab_files/categorical_collections/luts/fire-growth-forms.ttl"^^xsd:anyURI ;
.

<https://linked.data.gov.au/def/test/dawe-cv/93180d7c-0203-5b2f-a622-e977fd8deef0>
    a skos:Concept ;
    dcterms:identifier 21 ;
    dcterms:source <http://vocabs.paratoo.tern.org.au:1337/api/lut-fire-growth-forms> ;
    rdfs:isDefinedBy <https://linked.data.gov.au/def/nrm> ;
    skos:definition "Australian grass trees. Members of the Xanthorrhoeaceae family." ;
    skos:notation "GT" ;
    skos:prefLabel "Grass-Tree" ;
    schema:url "https://github.com/ternaustralia/dawe-rlp-vocabs/tree/main/vocab_files/categorical_collections/luts/fire-growth-forms.ttl"^^xsd:anyURI ;
.

<https://linked.data.gov.au/def/test/dawe-cv/93835815-2750-599d-b63a-494699ac8802>
    a skos:Concept ;
    dcterms:identifier 4 ;
    dcterms:source <http://vocabs.paratoo.tern.org.au:1337/api/lut-fire-growth-forms> ;
    rdfs:isDefinedBy <https://linked.data.gov.au/def/nrm> ;
    skos:definition "Commonly less than 8 m tall, usually with five or more trunks, of which at least three of the largest do not exceed 100 mm diameter at breast height (1.3 m)." ;
    skos:notation "MS" ;
    skos:prefLabel "Mallee Shrub" ;
    schema:url "https://github.com/ternaustralia/dawe-rlp-vocabs/tree/main/vocab_files/categorical_collections/luts/fire-growth-forms.ttl"^^xsd:anyURI ;
.

<https://linked.data.gov.au/def/test/dawe-cv/a97240fa-ad87-55d1-b4ed-2889fc7d5637>
    a skos:Concept ;
    dcterms:identifier 25 ;
    dcterms:source <http://vocabs.paratoo.tern.org.au:1337/api/lut-fire-growth-forms> ;
    rdfs:isDefinedBy <https://linked.data.gov.au/def/nrm> ;
    skos:definition "Algae, fungus" ;
    skos:notation "LP" ;
    skos:prefLabel "Lower Plant" ;
    schema:url "https://github.com/ternaustralia/dawe-rlp-vocabs/tree/main/vocab_files/categorical_collections/luts/fire-growth-forms.ttl"^^xsd:anyURI ;
.

<https://linked.data.gov.au/def/test/dawe-cv/ac2c4f2d-2e96-590f-ab4c-b6cb39f4c9df>
    a skos:Concept ;
    dcterms:identifier 12 ;
    dcterms:source <http://vocabs.paratoo.tern.org.au:1337/api/lut-fire-growth-forms> ;
    rdfs:isDefinedBy <https://linked.data.gov.au/def/nrm> ;
    skos:definition "Herbaceous, usually perennial erect monocot that is neither a grass nor a sedge. For the purposes of NVIS, rushes include the monocotyledon families Juncaceae, Typhaceae, Liliaceae, Iridaceae, Xyridaceae and the genus Lomandra. (i.e. 'graminoid' or grass-like genera)." ;
    skos:notation "R" ;
    skos:prefLabel "Rush" ;
    schema:url "https://github.com/ternaustralia/dawe-rlp-vocabs/tree/main/vocab_files/categorical_collections/luts/fire-growth-forms.ttl"^^xsd:anyURI ;
.

<https://linked.data.gov.au/def/test/dawe-cv/af735a8f-0adf-505f-a15a-cd4c95e8ef6f>
    a skos:Concept ;
    dcterms:identifier 15 ;
    dcterms:source <http://vocabs.paratoo.tern.org.au:1337/api/lut-fire-growth-forms> ;
    rdfs:isDefinedBy <https://linked.data.gov.au/def/nrm> ;
    skos:definition "Ferns and fern allies, except tree-fern, above. Characterised by large and usually branched leaves (fronds), herbaceous and terrestrial to aquatic; spores in sporangia on the leaves." ;
    skos:notation "FE" ;
    skos:prefLabel "Fern" ;
    schema:url "https://github.com/ternaustralia/dawe-rlp-vocabs/tree/main/vocab_files/categorical_collections/luts/fire-growth-forms.ttl"^^xsd:anyURI ;
.

<https://linked.data.gov.au/def/test/dawe-cv/b6900225-7940-5f7b-96f8-721f653dd1ba>
    a skos:Concept ;
    dcterms:identifier 24 ;
    dcterms:source <http://vocabs.paratoo.tern.org.au:1337/api/lut-fire-growth-forms> ;
    rdfs:isDefinedBy <https://linked.data.gov.au/def/nrm> ;
    skos:definition "Plant growing in an inland waterway or wetland with the majority of its biomass under water for most of the year. Fresh, saline or brackish water." ;
    skos:notation "A" ;
    skos:prefLabel "Aquatic" ;
    schema:url "https://github.com/ternaustralia/dawe-rlp-vocabs/tree/main/vocab_files/categorical_collections/luts/fire-growth-forms.ttl"^^xsd:anyURI ;
.

<https://linked.data.gov.au/def/test/dawe-cv/b772fc98-c494-50c4-8a4a-876c38c362cd>
    a skos:Concept ;
    dcterms:identifier 7 ;
    dcterms:source <http://vocabs.paratoo.tern.org.au:1337/api/lut-fire-growth-forms> ;
    rdfs:isDefinedBy <https://linked.data.gov.au/def/nrm> ;
    skos:definition "Genera (of Tribe Salicornioideae, viz.: Halosarcia, Pachycornia, Sarcocornia, Sclerostegia, Tecticornia andTegicornia) with articulate branches, fleshy stems and reduced flowers within the Chenopodiaceae family, succulent chenopods (Wilson 1980). Also the genus Suaeda." ;
    skos:notation " SS" ;
    skos:prefLabel "Samphire Shrub" ;
    schema:url "https://github.com/ternaustralia/dawe-rlp-vocabs/tree/main/vocab_files/categorical_collections/luts/fire-growth-forms.ttl"^^xsd:anyURI ;
.

<https://linked.data.gov.au/def/test/dawe-cv/c801b65c-80fd-5d1a-b0a7-f38f964732db>
    a skos:Concept ;
    dcterms:identifier 9 ;
    dcterms:source <http://vocabs.paratoo.tern.org.au:1337/api/lut-fire-growth-forms> ;
    rdfs:isDefinedBy <https://linked.data.gov.au/def/nrm> ;
    skos:definition "Coarse xeromorphic grass with a mound-like form often dead in the middle; genus is Triodia." ;
    skos:notation "HG" ;
    skos:prefLabel "Hummock Grass" ;
    schema:url "https://github.com/ternaustralia/dawe-rlp-vocabs/tree/main/vocab_files/categorical_collections/luts/fire-growth-forms.ttl"^^xsd:anyURI ;
.

<https://linked.data.gov.au/def/test/dawe-cv/ddecfd49-5e0b-5684-8147-dcb798710c7c>
    a skos:Concept ;
    dcterms:identifier 3 ;
    dcterms:source <http://vocabs.paratoo.tern.org.au:1337/api/lut-fire-growth-forms> ;
    rdfs:isDefinedBy <https://linked.data.gov.au/def/nrm> ;
    skos:definition "Woody plants multi-stemmed at the base (or within 200 mm from ground level) or if single stemmed, less than 2 m." ;
    skos:notation "S" ;
    skos:prefLabel "Shrub" ;
    schema:url "https://github.com/ternaustralia/dawe-rlp-vocabs/tree/main/vocab_files/categorical_collections/luts/fire-growth-forms.ttl"^^xsd:anyURI ;
.

<https://linked.data.gov.au/def/test/dawe-cv/f6ee4df7-f138-55e2-a1fd-4f93bee18a9e>
    a skos:Concept ;
    dcterms:identifier 1 ;
    dcterms:source <http://vocabs.paratoo.tern.org.au:1337/api/lut-fire-growth-forms> ;
    rdfs:isDefinedBy <https://linked.data.gov.au/def/nrm> ;
    skos:definition "Woody plants, more than 2 m tall with a single stem or branches well above the base." ;
    skos:notation "T" ;
    skos:prefLabel "Tree" ;
    schema:url "https://github.com/ternaustralia/dawe-rlp-vocabs/tree/main/vocab_files/categorical_collections/luts/fire-growth-forms.ttl"^^xsd:anyURI ;
.

<https://linked.data.gov.au/def/test/dawe-cv/fa1f7cef-6c5a-5487-83cb-f8700b0f67e5>
    a skos:Concept ;
    dcterms:identifier 14 ;
    dcterms:source <http://vocabs.paratoo.tern.org.au:1337/api/lut-fire-growth-forms> ;
    rdfs:isDefinedBy <https://linked.data.gov.au/def/nrm> ;
    skos:definition "Characterised by large and usually branched leaves (fronds), arborescent and terrestrial; spores in sporangia on the leaves." ;
    skos:notation "TF" ;
    skos:prefLabel "Tree-Fern" ;
    schema:url "https://github.com/ternaustralia/dawe-rlp-vocabs/tree/main/vocab_files/categorical_collections/luts/fire-growth-forms.ttl"^^xsd:anyURI ;
.

