# Do not edit this file directly. This file is generated by `make luts` with endpoints from src/dawe_nrm/api/categorical_values/endpoints.py
PREFIX dcterms: <http://purl.org/dc/terms/>
PREFIX rdfs: <http://www.w3.org/2000/01/rdf-schema#>
PREFIX schema: <https://schema.org/>
PREFIX skos: <http://www.w3.org/2004/02/skos/core#>
PREFIX xsd: <http://www.w3.org/2001/XMLSchema#>

<https://linked.data.gov.au/def/test/dawe-cv/096e018a-fb8f-4ba1-9fdc-302164e57682>
    a skos:Collection ;
    dcterms:description "A collection of growth stages and its codes." ;
    dcterms:source <http://vocabs.paratoo.tern.org.au:1337/api/lut-targeted-survey-flora-growth-stages> ;
    rdfs:isDefinedBy <https://linked.data.gov.au/def/nrm> ;
    skos:member
        <https://linked.data.gov.au/def/test/dawe-cv/1215ec81-a8a8-5100-b846-c50931e6fa27> ,
        <https://linked.data.gov.au/def/test/dawe-cv/3d82ced2-4ca3-5800-9e03-7ac1be45514e> ,
        <https://linked.data.gov.au/def/test/dawe-cv/3f62aa2c-4f5b-51b1-b90a-926d8219b9da> ,
        <https://linked.data.gov.au/def/test/dawe-cv/5bce18a8-4e8c-574f-881b-625bd9240cbc> ,
        <https://linked.data.gov.au/def/test/dawe-cv/999f3504-4cfd-5f88-9cc4-9bf1718992b0> ;
    skos:prefLabel "Growth stages codes" ;
    schema:url "https://github.com/ternaustralia/dawe-rlp-vocabs/tree/main/vocab_files/categorical_collections/luts/growth-stages.ttl"^^xsd:anyURI ;
.

<https://linked.data.gov.au/def/test/dawe-cv/1215ec81-a8a8-5100-b846-c50931e6fa27>
    a skos:Concept ;
    dcterms:identifier 5 ;
    dcterms:source <http://vocabs.paratoo.tern.org.au:1337/api/lut-targeted-survey-flora-growth-stages> ;
    rdfs:isDefinedBy <https://linked.data.gov.au/def/nrm> ;
    skos:definition "Tree description: Dead individuals in all stages - from presence of tertiary branches and bark to no remaining crown structure and absence of bark.  Shrub description: Dead individuals in all stages. " ;
    skos:notation "Dead" ;
    skos:prefLabel "Dead" ;
    schema:url "https://github.com/ternaustralia/dawe-rlp-vocabs/tree/main/vocab_files/categorical_collections/luts/growth-stages.ttl"^^xsd:anyURI ;
.

<https://linked.data.gov.au/def/test/dawe-cv/3d82ced2-4ca3-5800-9e03-7ac1be45514e>
    a skos:Concept ;
    dcterms:identifier 1 ;
    dcterms:source <http://vocabs.paratoo.tern.org.au:1337/api/lut-targeted-survey-flora-growth-stages> ;
    rdfs:isDefinedBy <https://linked.data.gov.au/def/nrm> ;
    skos:definition "Tree description: From the juvenile and sapling stages to well-developed individuals with a crown of small branches, but below maximum height for a stand, crown exhibits apical dominance - approx. 0-30 years.  Shrub description: Juvenile stage, shrub has not reached maximum height, apical dominance. " ;
    skos:notation "Recruiting" ;
    skos:prefLabel "Recruiting" ;
    schema:url "https://github.com/ternaustralia/dawe-rlp-vocabs/tree/main/vocab_files/categorical_collections/luts/growth-stages.ttl"^^xsd:anyURI ;
.

<https://linked.data.gov.au/def/test/dawe-cv/3f62aa2c-4f5b-51b1-b90a-926d8219b9da>
    a skos:Concept ;
    dcterms:identifier 4 ;
    dcterms:source <http://vocabs.paratoo.tern.org.au:1337/api/lut-targeted-survey-flora-growth-stages> ;
    rdfs:isDefinedBy <https://linked.data.gov.au/def/nrm> ;
    skos:definition "Tree description: Crown form contracting and becoming 'stag headed' decrease in crown diameter and crown leaf area. Distorted branches and burls common - approx. >80 years.  Shrub description: Crown form contracting and decrease in crown diameter and crown leaf area. Dead branches more common - approx. >80 years. " ;
    skos:notation "Senescent" ;
    skos:prefLabel "Senescent" ;
    schema:url "https://github.com/ternaustralia/dawe-rlp-vocabs/tree/main/vocab_files/categorical_collections/luts/growth-stages.ttl"^^xsd:anyURI ;
.

<https://linked.data.gov.au/def/test/dawe-cv/5bce18a8-4e8c-574f-881b-625bd9240cbc>
    a skos:Concept ;
    dcterms:identifier 3 ;
    dcterms:source <http://vocabs.paratoo.tern.org.au:1337/api/lut-targeted-survey-flora-growth-stages> ;
    rdfs:isDefinedBy <https://linked.data.gov.au/def/nrm> ;
    skos:definition "Tree description: Tree has reached maximum height and crown has reached full lateral development although branch thickening can occur. Apical dominance lost - approx. 30-80 years.  Shrub description: Shrub has reached maximum height, crown has reached full lateral development. " ;
    skos:notation "Mature" ;
    skos:prefLabel "Mature" ;
    schema:url "https://github.com/ternaustralia/dawe-rlp-vocabs/tree/main/vocab_files/categorical_collections/luts/growth-stages.ttl"^^xsd:anyURI ;
.

<https://linked.data.gov.au/def/test/dawe-cv/999f3504-4cfd-5f88-9cc4-9bf1718992b0>
    a skos:Concept ;
    dcterms:identifier 2 ;
    dcterms:source <http://vocabs.paratoo.tern.org.au:1337/api/lut-targeted-survey-flora-growth-stages> ;
    rdfs:isDefinedBy <https://linked.data.gov.au/def/nrm> ;
    skos:definition "Tree description: Woody perennial which is resprouting after significant loss of foliage.  Shrub description: Woody perennial which is resprouting after significant loss of foliage. " ;
    skos:notation "Resprouting" ;
    skos:prefLabel "Resprouting" ;
    schema:url "https://github.com/ternaustralia/dawe-rlp-vocabs/tree/main/vocab_files/categorical_collections/luts/growth-stages.ttl"^^xsd:anyURI ;
.

