PREFIX dcterms: <http://purl.org/dc/terms/>
PREFIX rdfs: <http://www.w3.org/2000/01/rdf-schema#>
PREFIX schema: <https://schema.org/>
PREFIX skos: <http://www.w3.org/2004/02/skos/core#>
PREFIX xsd: <http://www.w3.org/2001/XMLSchema#>

<https://linked.data.gov.au/def/test/dawe-cv/b8bfa5aa-b405-454f-b581-f5a9a7aaf71f>
    a skos:Collection ;
    dcterms:description "A collection of intervention types and its codes." ;
    dcterms:source <http://vocabs.paratoo.tern.org.au:1337/api/lut-intervention-types> ;
    rdfs:isDefinedBy <https://linked.data.gov.au/def/nrm> ;
    skos:member
        <https://linked.data.gov.au/def/test/dawe-cv/0a71c6bd-0717-50cf-a1cc-e72d557a3276> ,
        <https://linked.data.gov.au/def/test/dawe-cv/0c589fc6-9546-5470-982e-b70dccc12220> ,
        <https://linked.data.gov.au/def/test/dawe-cv/103c25e2-5caa-56a7-935d-9cd04f7838f1> ,
        <https://linked.data.gov.au/def/test/dawe-cv/26c34c87-0b1d-5c2d-b940-1bfe998292d2> ,
        <https://linked.data.gov.au/def/test/dawe-cv/28025018-ff3f-5cde-8178-01f8d1adcfaf> ,
        <https://linked.data.gov.au/def/test/dawe-cv/2ebf7d29-5e8b-5e9c-b16f-93e8fbbf742a> ,
        <https://linked.data.gov.au/def/test/dawe-cv/486a927d-6330-50c6-ba3e-ffbc7e7aeae9> ,
        <https://linked.data.gov.au/def/test/dawe-cv/5b919978-2f80-5b89-8b3d-e135ff9febe7> ,
        <https://linked.data.gov.au/def/test/dawe-cv/5c532462-2ed6-587d-987c-a88c814137d1> ,
        <https://linked.data.gov.au/def/test/dawe-cv/5cb5d2d5-87c1-5872-be7b-fbdd64eed784> ,
        <https://linked.data.gov.au/def/test/dawe-cv/7295c481-3812-5b03-8782-2073b5d1b96c> ,
        <https://linked.data.gov.au/def/test/dawe-cv/78571899-db4d-5882-9a69-1b519b26a58a> ,
        <https://linked.data.gov.au/def/test/dawe-cv/7b20208f-e0d2-559d-bab4-27f164a37571> ,
        <https://linked.data.gov.au/def/test/dawe-cv/7d6a0172-9861-5b7a-b3e2-ba5458f0d37f> ,
        <https://linked.data.gov.au/def/test/dawe-cv/85029337-b6b1-5c8d-a9d2-e3052b1fe59e> ,
        <https://linked.data.gov.au/def/test/dawe-cv/8a071b2b-0652-5665-9a85-0b7ee7ed00a4> ,
        <https://linked.data.gov.au/def/test/dawe-cv/8c45145c-eadd-5cad-8af7-b405e1f1561e> ,
        <https://linked.data.gov.au/def/test/dawe-cv/9c6baead-9792-5d54-8395-ecb46696e4e7> ,
        <https://linked.data.gov.au/def/test/dawe-cv/a95ac599-fab8-5bc1-836e-9475e0c99376> ,
        <https://linked.data.gov.au/def/test/dawe-cv/bee38f07-8b7c-57c7-95d7-675098959cc4> ,
        <https://linked.data.gov.au/def/test/dawe-cv/c631b672-038c-517a-bd07-402d9e0f3ebc> ,
        <https://linked.data.gov.au/def/test/dawe-cv/d05fb43a-f36f-5372-9497-1bb142708b5f> ,
        <https://linked.data.gov.au/def/test/dawe-cv/d1b9bc16-86f0-52c5-a67a-e42580705c42> ,
        <https://linked.data.gov.au/def/test/dawe-cv/dccd040f-5551-5698-9967-1e34382cd82c> ,
        <https://linked.data.gov.au/def/test/dawe-cv/ff0fcff0-3640-5e7b-9e2f-06fafa8c91aa> ;
    skos:prefLabel "Intervention types codes" ;
    schema:url "https://github.com/ternaustralia/dawe-rlp-vocabs/tree/main/vocab_files/categorical_collections/luts/intervention-types.ttl"^^xsd:anyURI ;
.

<https://linked.data.gov.au/def/test/dawe-cv/0a71c6bd-0717-50cf-a1cc-e72d557a3276>
    a skos:Concept ;
    dcterms:identifier 7 ;
    dcterms:source <http://vocabs.paratoo.tern.org.au:1337/api/lut-intervention-types> ;
    rdfs:isDefinedBy <https://linked.data.gov.au/def/nrm> ;
    skos:definition "Tell us about the breeding programs undertaken across the mapped area." ;
    skos:notation "EMB" ;
    skos:prefLabel "Establishing and Maintaining Breeding Program" ;
    schema:url "https://github.com/ternaustralia/dawe-rlp-vocabs/tree/main/vocab_files/categorical_collections/luts/intervention-types.ttl"^^xsd:anyURI ;
.

<https://linked.data.gov.au/def/test/dawe-cv/0c589fc6-9546-5470-982e-b70dccc12220>
    a skos:Concept ;
    dcterms:identifier 5 ;
    dcterms:source <http://vocabs.paratoo.tern.org.au:1337/api/lut-intervention-types> ;
    rdfs:isDefinedBy <https://linked.data.gov.au/def/nrm> ;
    skos:definition "Tell us about the area affected by erosion, methods used to control or avoid erosion across the mapped area, and any areas that have benefited from this work." ;
    skos:notation "EM" ;
    skos:prefLabel "Erosion Management" ;
    schema:url "https://github.com/ternaustralia/dawe-rlp-vocabs/tree/main/vocab_files/categorical_collections/luts/intervention-types.ttl"^^xsd:anyURI ;
.

<https://linked.data.gov.au/def/test/dawe-cv/103c25e2-5caa-56a7-935d-9cd04f7838f1>
    a skos:Concept ;
    dcterms:identifier 19 ;
    dcterms:source <http://vocabs.paratoo.tern.org.au:1337/api/lut-intervention-types> ;
    rdfs:isDefinedBy <https://linked.data.gov.au/def/nrm> ;
    skos:definition "Tell us about the weed removal activities you have undertaken across the mapped area." ;
    skos:notation "RW" ;
    skos:prefLabel "Removing Weeds" ;
    schema:url "https://github.com/ternaustralia/dawe-rlp-vocabs/tree/main/vocab_files/categorical_collections/luts/intervention-types.ttl"^^xsd:anyURI ;
.

<https://linked.data.gov.au/def/test/dawe-cv/26c34c87-0b1d-5c2d-b940-1bfe998292d2>
    a skos:Concept ;
    dcterms:identifier 14 ;
    dcterms:source <http://vocabs.paratoo.tern.org.au:1337/api/lut-intervention-types> ;
    rdfs:isDefinedBy <https://linked.data.gov.au/def/nrm> ;
    skos:definition "Tell us about the actions you have undertaken to improve land management practices across the mapped area and any areas that have benefitted from this work" ;
    skos:notation "ILMP" ;
    skos:prefLabel "Improving Land Management Practices" ;
    schema:url "https://github.com/ternaustralia/dawe-rlp-vocabs/tree/main/vocab_files/categorical_collections/luts/intervention-types.ttl"^^xsd:anyURI ;
.

<https://linked.data.gov.au/def/test/dawe-cv/28025018-ff3f-5cde-8178-01f8d1adcfaf>
    a skos:Concept ;
    dcterms:identifier 6 ;
    dcterms:source <http://vocabs.paratoo.tern.org.au:1337/api/lut-intervention-types> ;
    rdfs:isDefinedBy <https://linked.data.gov.au/def/nrm> ;
    skos:definition "Tell us about the actions you have undertaken to protect native species or control feral species across the mapped area." ;
    skos:notation "EMF" ;
    skos:prefLabel "Establishing and Maintaining  Feral-Free Enclosures" ;
    schema:url "https://github.com/ternaustralia/dawe-rlp-vocabs/tree/main/vocab_files/categorical_collections/luts/intervention-types.ttl"^^xsd:anyURI ;
.

<https://linked.data.gov.au/def/test/dawe-cv/2ebf7d29-5e8b-5e9c-b16f-93e8fbbf742a>
    a skos:Concept ;
    dcterms:identifier 22 ;
    dcterms:source <http://vocabs.paratoo.tern.org.au:1337/api/lut-intervention-types> ;
    rdfs:isDefinedBy <https://linked.data.gov.au/def/nrm> ;
    skos:definition "Tell us about the soil testing you have undertaken across your mapped area." ;
    skos:notation "ST" ;
    skos:prefLabel "Soil Testing" ;
    schema:url "https://github.com/ternaustralia/dawe-rlp-vocabs/tree/main/vocab_files/categorical_collections/luts/intervention-types.ttl"^^xsd:anyURI ;
.

<https://linked.data.gov.au/def/test/dawe-cv/486a927d-6330-50c6-ba3e-ffbc7e7aeae9>
    a skos:Concept ;
    dcterms:identifier 9 ;
    dcterms:source <http://vocabs.paratoo.tern.org.au:1337/api/lut-intervention-types> ;
    rdfs:isDefinedBy <https://linked.data.gov.au/def/nrm> ;
    skos:definition "Tell us about the fire management actions you have undertaken across the mapped area and any areas that have benefitted from this work." ;
    skos:notation "IFM" ;
    skos:prefLabel "Implementing Fire Management Actions" ;
    schema:url "https://github.com/ternaustralia/dawe-rlp-vocabs/tree/main/vocab_files/categorical_collections/luts/intervention-types.ttl"^^xsd:anyURI ;
.

<https://linked.data.gov.au/def/test/dawe-cv/5b919978-2f80-5b89-8b3d-e135ff9febe7>
    a skos:Concept ;
    dcterms:identifier 16 ;
    dcterms:source <http://vocabs.paratoo.tern.org.au:1337/api/lut-intervention-types> ;
    rdfs:isDefinedBy <https://linked.data.gov.au/def/nrm> ;
    skos:definition "Tell us about the pest animal surveys being conducted across the mapped area." ;
    skos:notation "PAS" ;
    skos:prefLabel "Pest Animal Survey" ;
    schema:url "https://github.com/ternaustralia/dawe-rlp-vocabs/tree/main/vocab_files/categorical_collections/luts/intervention-types.ttl"^^xsd:anyURI ;
.

<https://linked.data.gov.au/def/test/dawe-cv/5c532462-2ed6-587d-987c-a88c814137d1>
    a skos:Concept ;
    dcterms:identifier 4 ;
    dcterms:source <http://vocabs.paratoo.tern.org.au:1337/api/lut-intervention-types> ;
    rdfs:isDefinedBy <https://linked.data.gov.au/def/nrm> ;
    skos:definition "Tell us about the actions you have undertaken to remove debris from land and/or water systems in the mapped area." ;
    skos:notation "DR" ;
    skos:prefLabel "Debris Removal" ;
    schema:url "https://github.com/ternaustralia/dawe-rlp-vocabs/tree/main/vocab_files/categorical_collections/luts/intervention-types.ttl"^^xsd:anyURI ;
.

<https://linked.data.gov.au/def/test/dawe-cv/5cb5d2d5-87c1-5872-be7b-fbdd64eed784>
    a skos:Concept ;
    dcterms:identifier 11 ;
    dcterms:source <http://vocabs.paratoo.tern.org.au:1337/api/lut-intervention-types> ;
    rdfs:isDefinedBy <https://linked.data.gov.au/def/nrm> ;
    skos:definition "Tell us about the habitat augmentation actions you have undertaken across the mapped area and areas that have benefitted from this work." ;
    skos:notation "HA" ;
    skos:prefLabel "Habitat Augmentation" ;
    schema:url "https://github.com/ternaustralia/dawe-rlp-vocabs/tree/main/vocab_files/categorical_collections/luts/intervention-types.ttl"^^xsd:anyURI ;
.

<https://linked.data.gov.au/def/test/dawe-cv/7295c481-3812-5b03-8782-2073b5d1b96c>
    a skos:Concept ;
    dcterms:identifier 20 ;
    dcterms:source <http://vocabs.paratoo.tern.org.au:1337/api/lut-intervention-types> ;
    rdfs:isDefinedBy <https://linked.data.gov.au/def/nrm> ;
    skos:definition "Tell us about the revegetation activities you have undertaken." ;
    skos:notation "RH" ;
    skos:prefLabel "Revegetating Habitat" ;
    schema:url "https://github.com/ternaustralia/dawe-rlp-vocabs/tree/main/vocab_files/categorical_collections/luts/intervention-types.ttl"^^xsd:anyURI ;
.

<https://linked.data.gov.au/def/test/dawe-cv/78571899-db4d-5882-9a69-1b519b26a58a>
    a skos:Concept ;
    dcterms:identifier 21 ;
    dcterms:source <http://vocabs.paratoo.tern.org.au:1337/api/lut-intervention-types> ;
    rdfs:isDefinedBy <https://linked.data.gov.au/def/nrm> ;
    skos:definition "Tell us about the actions and methods used to prepare sites for subsequent activities." ;
    skos:notation "SP" ;
    skos:prefLabel "Site Preparation" ;
    schema:url "https://github.com/ternaustralia/dawe-rlp-vocabs/tree/main/vocab_files/categorical_collections/luts/intervention-types.ttl"^^xsd:anyURI ;
.

<https://linked.data.gov.au/def/test/dawe-cv/7b20208f-e0d2-559d-bab4-27f164a37571>
    a skos:Concept ;
    dcterms:identifier 8 ;
    dcterms:source <http://vocabs.paratoo.tern.org.au:1337/api/lut-intervention-types> ;
    rdfs:isDefinedBy <https://linked.data.gov.au/def/nrm> ;
    skos:definition "Tell us about the fauna surveys being conducted across the mapped areas." ;
    skos:notation "FS" ;
    skos:prefLabel "Fauna Survey" ;
    schema:url "https://github.com/ternaustralia/dawe-rlp-vocabs/tree/main/vocab_files/categorical_collections/luts/intervention-types.ttl"^^xsd:anyURI ;
.

<https://linked.data.gov.au/def/test/dawe-cv/7d6a0172-9861-5b7a-b3e2-ba5458f0d37f>
    a skos:Concept ;
    dcterms:identifier 12 ;
    dcterms:source <http://vocabs.paratoo.tern.org.au:1337/api/lut-intervention-types> ;
    rdfs:isDefinedBy <https://linked.data.gov.au/def/nrm> ;
    skos:definition "Tell us about the potential sites you have identified to deliver your RLP services and briefly describe the works you will undertaken." ;
    skos:notation "ILPS" ;
    skos:prefLabel "Identifying the Location of Potential Sites" ;
    schema:url "https://github.com/ternaustralia/dawe-rlp-vocabs/tree/main/vocab_files/categorical_collections/luts/intervention-types.ttl"^^xsd:anyURI ;
.

<https://linked.data.gov.au/def/test/dawe-cv/85029337-b6b1-5c8d-a9d2-e3052b1fe59e>
    a skos:Concept ;
    dcterms:identifier 17 ;
    dcterms:source <http://vocabs.paratoo.tern.org.au:1337/api/lut-intervention-types> ;
    rdfs:isDefinedBy <https://linked.data.gov.au/def/nrm> ;
    skos:definition "Tell us about the plant survival surveys being conducted across the mapped area." ;
    skos:notation "PSS" ;
    skos:prefLabel "Plant Survival Survey" ;
    schema:url "https://github.com/ternaustralia/dawe-rlp-vocabs/tree/main/vocab_files/categorical_collections/luts/intervention-types.ttl"^^xsd:anyURI ;
.

<https://linked.data.gov.au/def/test/dawe-cv/8a071b2b-0652-5665-9a85-0b7ee7ed00a4>
    a skos:Concept ;
    dcterms:identifier 13 ;
    dcterms:source <http://vocabs.paratoo.tern.org.au:1337/api/lut-intervention-types> ;
    rdfs:isDefinedBy <https://linked.data.gov.au/def/nrm> ;
    skos:definition "Tell us about the treatments implemented to improve water management across the mapped area and any areas that have benefitted from this work." ;
    skos:notation "IHR" ;
    skos:prefLabel "Improving Hydrological Regime" ;
    schema:url "https://github.com/ternaustralia/dawe-rlp-vocabs/tree/main/vocab_files/categorical_collections/luts/intervention-types.ttl"^^xsd:anyURI ;
.

<https://linked.data.gov.au/def/test/dawe-cv/8c45145c-eadd-5cad-8af7-b405e1f1561e>
    a skos:Concept ;
    dcterms:identifier 24 ;
    dcterms:source <http://vocabs.paratoo.tern.org.au:1337/api/lut-intervention-types> ;
    rdfs:isDefinedBy <https://linked.data.gov.au/def/nrm> ;
    skos:definition "Tell us about the water quality surveys being conducted across the mapped area." ;
    skos:notation "WQS" ;
    skos:prefLabel "Water Quality Survey" ;
    schema:url "https://github.com/ternaustralia/dawe-rlp-vocabs/tree/main/vocab_files/categorical_collections/luts/intervention-types.ttl"^^xsd:anyURI ;
.

<https://linked.data.gov.au/def/test/dawe-cv/9c6baead-9792-5d54-8395-ecb46696e4e7>
    a skos:Concept ;
    dcterms:identifier 10 ;
    dcterms:source <http://vocabs.paratoo.tern.org.au:1337/api/lut-intervention-types> ;
    rdfs:isDefinedBy <https://linked.data.gov.au/def/nrm> ;
    skos:definition "Tell us about the flora survey being conducted across the mapped area." ;
    skos:notation "FLS" ;
    skos:prefLabel "Flora Survey" ;
    schema:url "https://github.com/ternaustralia/dawe-rlp-vocabs/tree/main/vocab_files/categorical_collections/luts/intervention-types.ttl"^^xsd:anyURI ;
.

<https://linked.data.gov.au/def/test/dawe-cv/a95ac599-fab8-5bc1-836e-9475e0c99376>
    a skos:Concept ;
    dcterms:identifier 3 ;
    dcterms:source <http://vocabs.paratoo.tern.org.au:1337/api/lut-intervention-types> ;
    rdfs:isDefinedBy <https://linked.data.gov.au/def/nrm> ;
    skos:definition "Tell us about the actions you have undertaken to control pest animals across the mapped area, and your objective." ;
    skos:notation "CPA" ;
    skos:prefLabel "Controlling Pest Animals" ;
    schema:url "https://github.com/ternaustralia/dawe-rlp-vocabs/tree/main/vocab_files/categorical_collections/luts/intervention-types.ttl"^^xsd:anyURI ;
.

<https://linked.data.gov.au/def/test/dawe-cv/bee38f07-8b7c-57c7-95d7-675098959cc4>
    a skos:Concept ;
    dcterms:identifier 23 ;
    dcterms:source <http://vocabs.paratoo.tern.org.au:1337/api/lut-intervention-types> ;
    rdfs:isDefinedBy <https://linked.data.gov.au/def/nrm> ;
    skos:definition "Tell us about emergency interventions you may have undertaken to prevent extinctions in your mapped area." ;
    skos:notation "UEI" ;
    skos:prefLabel "Undertaking Emergency Interventions to Prevent Extinctions" ;
    schema:url "https://github.com/ternaustralia/dawe-rlp-vocabs/tree/main/vocab_files/categorical_collections/luts/intervention-types.ttl"^^xsd:anyURI ;
.

<https://linked.data.gov.au/def/test/dawe-cv/c631b672-038c-517a-bd07-402d9e0f3ebc>
    a skos:Concept ;
    dcterms:identifier 2 ;
    dcterms:source <http://vocabs.paratoo.tern.org.au:1337/api/lut-intervention-types> ;
    rdfs:isDefinedBy <https://linked.data.gov.au/def/nrm> ;
    skos:definition "Tell us about the structures you have installed to control access and any off-site areas showing evidence of beingprotected by this action." ;
    skos:notation "CA" ;
    skos:prefLabel "Controlling Access" ;
    schema:url "https://github.com/ternaustralia/dawe-rlp-vocabs/tree/main/vocab_files/categorical_collections/luts/intervention-types.ttl"^^xsd:anyURI ;
.

<https://linked.data.gov.au/def/test/dawe-cv/d05fb43a-f36f-5372-9497-1bb142708b5f>
    a skos:Concept ;
    dcterms:identifier 18 ;
    dcterms:source <http://vocabs.paratoo.tern.org.au:1337/api/lut-intervention-types> ;
    rdfs:isDefinedBy <https://linked.data.gov.au/def/nrm> ;
    skos:definition "Tell us about the remediation actions you have undertaken across the mapped area and any areas that have benefitted from this work." ;
    skos:notation "RRAA" ;
    skos:prefLabel "Remediating Riparian and Aquatic Area" ;
    schema:url "https://github.com/ternaustralia/dawe-rlp-vocabs/tree/main/vocab_files/categorical_collections/luts/intervention-types.ttl"^^xsd:anyURI ;
.

<https://linked.data.gov.au/def/test/dawe-cv/d1b9bc16-86f0-52c5-a67a-e42580705c42>
    a skos:Concept ;
    dcterms:identifier 15 ;
    dcterms:source <http://vocabs.paratoo.tern.org.au:1337/api/lut-intervention-types> ;
    rdfs:isDefinedBy <https://linked.data.gov.au/def/nrm> ;
    skos:definition "Tell us about the disease/s being managed and the actions you have undertaken across the mapped area and any areas that have benefitted from this work." ;
    skos:notation "MD" ;
    skos:prefLabel "Managing Disease" ;
    schema:url "https://github.com/ternaustralia/dawe-rlp-vocabs/tree/main/vocab_files/categorical_collections/luts/intervention-types.ttl"^^xsd:anyURI ;
.

<https://linked.data.gov.au/def/test/dawe-cv/dccd040f-5551-5698-9967-1e34382cd82c>
    a skos:Concept ;
    dcterms:identifier 1 ;
    dcterms:source <http://vocabs.paratoo.tern.org.au:1337/api/lut-intervention-types> ;
    rdfs:isDefinedBy <https://linked.data.gov.au/def/nrm> ;
    skos:definition "Tell us how many types of data sets you collected and/or synthesised" ;
    skos:notation "CSBD" ;
    skos:prefLabel "Collecting or Synthesising Baseline Data" ;
    schema:url "https://github.com/ternaustralia/dawe-rlp-vocabs/tree/main/vocab_files/categorical_collections/luts/intervention-types.ttl"^^xsd:anyURI ;
.

<https://linked.data.gov.au/def/test/dawe-cv/ff0fcff0-3640-5e7b-9e2f-06fafa8c91aa>
    a skos:Concept ;
    dcterms:identifier 25 ;
    dcterms:source <http://vocabs.paratoo.tern.org.au:1337/api/lut-intervention-types> ;
    rdfs:isDefinedBy <https://linked.data.gov.au/def/nrm> ;
    skos:definition "Tell us about the weed distribution surveys being conducted across the mapped area." ;
    skos:notation "WDS" ;
    skos:prefLabel "Weed Distribution Survey" ;
    schema:url "https://github.com/ternaustralia/dawe-rlp-vocabs/tree/main/vocab_files/categorical_collections/luts/intervention-types.ttl"^^xsd:anyURI ;
.

