# Do not edit this file directly. This file is generated by `make luts` with endpoints from src/dawe_nrm/api/categorical_values/endpoints.py
PREFIX dcterms: <http://purl.org/dc/terms/>
PREFIX rdfs: <http://www.w3.org/2000/01/rdf-schema#>
PREFIX schema: <https://schema.org/>
PREFIX skos: <http://www.w3.org/2004/02/skos/core#>
PREFIX urnc: <urn:class:>
PREFIX urnp: <urn:property:>
PREFIX xsd: <http://www.w3.org/2001/XMLSchema#>

<https://linked.data.gov.au/def/nrm/090ab00d-476e-5b85-afb6-7cca342b3ebc>
    a urnc:CategoricalConceptMeta ;
    schema:url "https://github.com/ternaustralia/dawe-rlp-vocabs/tree/main/vocab_files/categorical_collections/luts/landform-element.ttl"^^xsd:anyURI ;
    urnp:categoricalCollection <https://linked.data.gov.au/def/nrm/c1a58967-cb12-4c2c-a7ca-9cee2589919c> ;
    urnp:categoricalConcept <https://linked.data.gov.au/def/nrm/e705f231-3807-5f0b-9afd-59a1c9093a36> ;
    urnp:conceptDefinition "Long; generally sinuous; low ridge built up from materials originally deposited by stream flow along the line of a former stream channel. The landform element may include a depression marking the old stream bed; and relict levees." ;
    urnp:conceptIdentifier 53 ;
    urnp:conceptNotation "PST" ;
    urnp:conceptSource <https://core.vocabs.paratoo.tern.org.au/api/lut-landform-elements> ;
.

<https://linked.data.gov.au/def/nrm/091d7ea0-3ff7-5bc4-a2ad-c899d79f1997>
    a urnc:CategoricalConceptMeta ;
    schema:url "https://github.com/ternaustralia/dawe-rlp-vocabs/tree/main/vocab_files/categorical_collections/luts/landform-element.ttl"^^xsd:anyURI ;
    urnp:categoricalCollection <https://linked.data.gov.au/def/nrm/c1a58967-cb12-4c2c-a7ca-9cee2589919c> ;
    urnp:categoricalConcept <https://linked.data.gov.au/def/nrm/9fcf1019-135e-5fad-9fab-ea6da190eb05> ;
    urnp:conceptDefinition "Flat of consolidated rock eroded by waves." ;
    urnp:conceptIdentifier 59 ;
    urnp:conceptNotation "RPL" ;
    urnp:conceptSource <https://core.vocabs.paratoo.tern.org.au/api/lut-landform-elements> ;
.

<https://linked.data.gov.au/def/nrm/0984ff0a-ae49-5a2a-907d-431be99f9f2a>
    a urnc:CategoricalConceptMeta ;
    schema:url "https://github.com/ternaustralia/dawe-rlp-vocabs/tree/main/vocab_files/categorical_collections/luts/landform-element.ttl"^^xsd:anyURI ;
    urnp:categoricalCollection <https://linked.data.gov.au/def/nrm/c1a58967-cb12-4c2c-a7ca-9cee2589919c> ;
    urnp:categoricalConcept <https://linked.data.gov.au/def/nrm/dd2d43e4-2a30-509f-817a-407b271e8204> ;
    urnp:conceptDefinition "See Tidal flat." ;
    urnp:conceptIdentifier 69 ;
    urnp:conceptNotation "STF" ;
    urnp:conceptSource <https://core.vocabs.paratoo.tern.org.au/api/lut-landform-elements> ;
.

<https://linked.data.gov.au/def/nrm/0a8fd92c-b8d0-5fba-a4d4-0d4c5d540f34>
    a urnc:CategoricalConceptMeta ;
    schema:url "https://github.com/ternaustralia/dawe-rlp-vocabs/tree/main/vocab_files/categorical_collections/luts/landform-element.ttl"^^xsd:anyURI ;
    urnp:categoricalCollection <https://linked.data.gov.au/def/nrm/c1a58967-cb12-4c2c-a7ca-9cee2589919c> ;
    urnp:categoricalConcept <https://linked.data.gov.au/def/nrm/0eec5735-6c35-58bf-9cc7-d129f4c6b8b2> ;
    urnp:conceptDefinition "Flat built up to sea level by marine organisms." ;
    urnp:conceptIdentifier 54 ;
    urnp:conceptNotation "REF" ;
    urnp:conceptSource <https://core.vocabs.paratoo.tern.org.au/api/lut-landform-elements> ;
.

<https://linked.data.gov.au/def/nrm/0be7b164-3f5b-53d7-a526-d8a97f8a7814>
    a urnc:CategoricalConceptMeta ;
    schema:url "https://github.com/ternaustralia/dawe-rlp-vocabs/tree/main/vocab_files/categorical_collections/luts/landform-element.ttl"^^xsd:anyURI ;
    urnp:categoricalCollection <https://linked.data.gov.au/def/nrm/c1a58967-cb12-4c2c-a7ca-9cee2589919c> ;
    urnp:categoricalConcept <https://linked.data.gov.au/def/nrm/95d1041f-0a82-50d5-9702-f58a95029f95> ;
    urnp:conceptDefinition "Large flat resulting from aggradation by overbank stream flow at some distance from the stream channel and in some cases biological (peat) accumulation; often characterised by a high watertable and the presence of swamps or lakes; part of a covered plain landform pattern." ;
    urnp:conceptIdentifier 2 ;
    urnp:conceptNotation "BKP" ;
    urnp:conceptSource <https://core.vocabs.paratoo.tern.org.au/api/lut-landform-elements> ;
.

<https://linked.data.gov.au/def/nrm/0c5ea218-0495-5aaf-bc9b-ea7316799ac8>
    a urnc:CategoricalConceptMeta ;
    schema:url "https://github.com/ternaustralia/dawe-rlp-vocabs/tree/main/vocab_files/categorical_collections/luts/landform-element.ttl"^^xsd:anyURI ;
    urnp:categoricalCollection <https://linked.data.gov.au/def/nrm/c1a58967-cb12-4c2c-a7ca-9cee2589919c> ;
    urnp:categoricalConcept <https://linked.data.gov.au/def/nrm/b82cfeb6-1194-513a-ba81-5010cb9eb38b> ;
    urnp:conceptDefinition "Intermittently water-filled open depression in parts eroded; excavated; built up and aggraded by channelled tide-water flow; type of stream channel characterised by a rapid increase in width downstream." ;
    urnp:conceptIdentifier 75 ;
    urnp:conceptNotation "TDC" ;
    urnp:conceptSource <https://core.vocabs.paratoo.tern.org.au/api/lut-landform-elements> ;
.

<https://linked.data.gov.au/def/nrm/0d181003-328e-5ef8-bcdc-707a72b36149>
    a urnc:CategoricalConceptMeta ;
    schema:url "https://github.com/ternaustralia/dawe-rlp-vocabs/tree/main/vocab_files/categorical_collections/luts/landform-element.ttl"^^xsd:anyURI ;
    urnp:categoricalCollection <https://linked.data.gov.au/def/nrm/c1a58967-cb12-4c2c-a7ca-9cee2589919c> ;
    urnp:categoricalConcept <https://linked.data.gov.au/def/nrm/69a64f8c-65b5-5185-8e16-39ce4f28a839> ;
    urnp:conceptDefinition "Large flat resulting from aggradation by channelled stream flow as a stream migrates from side to side; the dominant element of a meander plain landform pattern. This landform element may include occurrences of scroll; swale and ox-bow." ;
    urnp:conceptIdentifier 64 ;
    urnp:conceptNotation "SRP" ;
    urnp:conceptSource <https://core.vocabs.paratoo.tern.org.au/api/lut-landform-elements> ;
.

<https://linked.data.gov.au/def/nrm/160d44e9-4010-50df-949b-b2353546d176>
    a urnc:CategoricalConceptMeta ;
    schema:url "https://github.com/ternaustralia/dawe-rlp-vocabs/tree/main/vocab_files/categorical_collections/luts/landform-element.ttl"^^xsd:anyURI ;
    urnp:categoricalCollection <https://linked.data.gov.au/def/nrm/c1a58967-cb12-4c2c-a7ca-9cee2589919c> ;
    urnp:categoricalConcept <https://linked.data.gov.au/def/nrm/1431e5bb-f41a-56cc-b685-9aeed406fe63> ;
    urnp:conceptDefinition "Steep to precipitous closed depression excavated by explosions due to volcanism; human action; or impact of an extraterrestrial object." ;
    urnp:conceptIdentifier 18 ;
    urnp:conceptNotation "CRA" ;
    urnp:conceptSource <https://core.vocabs.paratoo.tern.org.au/api/lut-landform-elements> ;
.

<https://linked.data.gov.au/def/nrm/196cc8f4-ca9d-5013-b2d0-60d73ea9cb5a>
    a urnc:CategoricalConceptMeta ;
    schema:url "https://github.com/ternaustralia/dawe-rlp-vocabs/tree/main/vocab_files/categorical_collections/luts/landform-element.ttl"^^xsd:anyURI ;
    urnp:categoricalCollection <https://linked.data.gov.au/def/nrm/c1a58967-cb12-4c2c-a7ca-9cee2589919c> ;
    urnp:categoricalConcept <https://linked.data.gov.au/def/nrm/c5274b62-aa6d-5168-a941-37842c6d4791> ;
    urnp:conceptDefinition "Precipitous to gently inclined; typically closed depression of concave contour and profile excavated by ice. The closed part of the depression may be shallow; the larger part being an open depression like an alcove." ;
    urnp:conceptIdentifier 13 ;
    urnp:conceptNotation "CIR" ;
    urnp:conceptSource <https://core.vocabs.paratoo.tern.org.au/api/lut-landform-elements> ;
.

<https://linked.data.gov.au/def/nrm/2283665d-fda9-5f41-932c-a9ecfbcefa9c>
    a urnc:CategoricalConceptMeta ;
    schema:url "https://github.com/ternaustralia/dawe-rlp-vocabs/tree/main/vocab_files/categorical_collections/luts/landform-element.ttl"^^xsd:anyURI ;
    urnp:categoricalCollection <https://linked.data.gov.au/def/nrm/c1a58967-cb12-4c2c-a7ca-9cee2589919c> ;
    urnp:categoricalConcept <https://linked.data.gov.au/def/nrm/45db9fbc-4730-51bb-9329-8818736698cc> ;
    urnp:conceptDefinition "Large; shallow; level-floored closed depression; intermittently water-filled; but mainly dry due to evaporation; bounded as a rule by flats aggraded by sheet flow and channelled stream flow." ;
    urnp:conceptIdentifier 52 ;
    urnp:conceptNotation "PLY" ;
    urnp:conceptSource <https://core.vocabs.paratoo.tern.org.au/api/lut-landform-elements> ;
.

<https://linked.data.gov.au/def/nrm/2321310c-114e-5491-90c2-d0cfff822553>
    a urnc:CategoricalConceptMeta ;
    schema:url "https://github.com/ternaustralia/dawe-rlp-vocabs/tree/main/vocab_files/categorical_collections/luts/landform-element.ttl"^^xsd:anyURI ;
    urnp:categoricalCollection <https://linked.data.gov.au/def/nrm/c1a58967-cb12-4c2c-a7ca-9cee2589919c> ;
    urnp:categoricalConcept <https://linked.data.gov.au/def/nrm/b2025ffe-3999-5c93-a6ef-295bfed37242> ;
    urnp:conceptDefinition "Sand dune with a long; scoop-shaped form; convex in the downwind direction so that its horns point upwind; whose ground plan approximates the form of a parabola. The dunes left behind can be referred to as trailing arms. Where many such dunes have traversed an area; these can give the appearance of linear dunes." ;
    urnp:conceptIdentifier 48 ;
    urnp:conceptNotation "DUP" ;
    urnp:conceptSource <https://core.vocabs.paratoo.tern.org.au/api/lut-landform-elements> ;
.

<https://linked.data.gov.au/def/nrm/25c322d8-61d4-5127-bb2f-0156a5e5607f>
    a urnc:CategoricalConceptMeta ;
    schema:url "https://github.com/ternaustralia/dawe-rlp-vocabs/tree/main/vocab_files/categorical_collections/luts/landform-element.ttl"^^xsd:anyURI ;
    urnp:categoricalCollection <https://linked.data.gov.au/def/nrm/c1a58967-cb12-4c2c-a7ca-9cee2589919c> ;
    urnp:categoricalConcept <https://linked.data.gov.au/def/nrm/bceaebcb-9ab0-54b0-8ea2-b66c3efe9490> ;
    urnp:conceptDefinition "Slope of hillock of very low to extremely low relief (<30 m) (see Residual rise)." ;
    urnp:conceptIdentifier 57 ;
    urnp:conceptNotation "RES" ;
    urnp:conceptSource <https://core.vocabs.paratoo.tern.org.au/api/lut-landform-elements> ;
.

<https://linked.data.gov.au/def/nrm/29b4e0da-94de-58bb-87eb-9754614f2266>
    a urnc:CategoricalConceptMeta ;
    schema:url "https://github.com/ternaustralia/dawe-rlp-vocabs/tree/main/vocab_files/categorical_collections/luts/landform-element.ttl"^^xsd:anyURI ;
    urnp:categoricalCollection <https://linked.data.gov.au/def/nrm/c1a58967-cb12-4c2c-a7ca-9cee2589919c> ;
    urnp:categoricalConcept <https://linked.data.gov.au/def/nrm/85b66cd6-ced2-5176-8338-6cf889145d08> ;
    urnp:conceptDefinition "Hillock with a circular symmetry built up by volcanism. The crest may form a ring around a crater." ;
    urnp:conceptIdentifier 17 ;
    urnp:conceptNotation "CON" ;
    urnp:conceptSource <https://core.vocabs.paratoo.tern.org.au/api/lut-landform-elements> ;
.

<https://linked.data.gov.au/def/nrm/2c37886e-0e46-55b2-9049-9678e2195766>
    a urnc:CategoricalConceptMeta ;
    schema:url "https://github.com/ternaustralia/dawe-rlp-vocabs/tree/main/vocab_files/categorical_collections/luts/landform-element.ttl"^^xsd:anyURI ;
    urnp:categoricalCollection <https://linked.data.gov.au/def/nrm/c1a58967-cb12-4c2c-a7ca-9cee2589919c> ;
    urnp:categoricalConcept <https://linked.data.gov.au/def/nrm/0de17230-6ae6-5c2e-ab07-0bbe262a3501> ;
    urnp:conceptDefinition "Closed depression excavated by human activity." ;
    urnp:conceptIdentifier 50 ;
    urnp:conceptNotation "PIT" ;
    urnp:conceptSource <https://core.vocabs.paratoo.tern.org.au/api/lut-landform-elements> ;
.

<https://linked.data.gov.au/def/nrm/2c3b9fdc-5843-509d-9c5d-fe5c6f0329cb>
    a urnc:CategoricalConceptMeta ;
    schema:url "https://github.com/ternaustralia/dawe-rlp-vocabs/tree/main/vocab_files/categorical_collections/luts/landform-element.ttl"^^xsd:anyURI ;
    urnp:categoricalCollection <https://linked.data.gov.au/def/nrm/c1a58967-cb12-4c2c-a7ca-9cee2589919c> ;
    urnp:categoricalConcept <https://linked.data.gov.au/def/nrm/1248ad7d-fb9c-564f-93c4-0c6bf3fe9088> ;
    urnp:conceptDefinition "Long; curved; commonly water-filled closed depression eroded by channelled stream flow but closed as a result of aggradation by channelled or overbank stream flow during the formation of a meander plain landform pattern. The floor of an ox-bow may be more or less aggraded by overbank stream flow; wind; and biological (peat) accumulation." ;
    urnp:conceptIdentifier 47 ;
    urnp:conceptNotation "OXB" ;
    urnp:conceptSource <https://core.vocabs.paratoo.tern.org.au/api/lut-landform-elements> ;
.

<https://linked.data.gov.au/def/nrm/2d5d3790-186a-5ee7-b41a-efa7df040e3c>
    a urnc:CategoricalConceptMeta ;
    schema:url "https://github.com/ternaustralia/dawe-rlp-vocabs/tree/main/vocab_files/categorical_collections/luts/landform-element.ttl"^^xsd:anyURI ;
    urnp:categoricalCollection <https://linked.data.gov.au/def/nrm/c1a58967-cb12-4c2c-a7ca-9cee2589919c> ;
    urnp:categoricalConcept <https://linked.data.gov.au/def/nrm/1470deb8-2762-5fd9-8c53-fc6cf2f18a4e> ;
    urnp:conceptDefinition "Very long; nearly straight; low ridge; built up by waves and usually modified by wind. A beach ridge is often a relict feature remote from the beach." ;
    urnp:conceptIdentifier 7 ;
    urnp:conceptNotation "BRI" ;
    urnp:conceptSource <https://core.vocabs.paratoo.tern.org.au/api/lut-landform-elements> ;
.

<https://linked.data.gov.au/def/nrm/39716724-eb65-5c47-9562-1007d34c4c5b>
    a urnc:CategoricalConceptMeta ;
    schema:url "https://github.com/ternaustralia/dawe-rlp-vocabs/tree/main/vocab_files/categorical_collections/luts/landform-element.ttl"^^xsd:anyURI ;
    urnp:categoricalCollection <https://linked.data.gov.au/def/nrm/c1a58967-cb12-4c2c-a7ca-9cee2589919c> ;
    urnp:categoricalConcept <https://linked.data.gov.au/def/nrm/987ae37a-02be-5ef7-a4a6-1b13406fa277> ;
    urnp:conceptDefinition "Linear; generally sinuous open depression; in parts eroded; excavated; built up and aggraded by channelled stream flow. This element comprises stream bed and banks." ;
    urnp:conceptIdentifier 67 ;
    urnp:conceptNotation "STC" ;
    urnp:conceptSource <https://core.vocabs.paratoo.tern.org.au/api/lut-landform-elements> ;
.

<https://linked.data.gov.au/def/nrm/3b240bbb-ecac-533e-b103-92707b6b155a>
    a urnc:CategoricalConceptMeta ;
    schema:url "https://github.com/ternaustralia/dawe-rlp-vocabs/tree/main/vocab_files/categorical_collections/luts/landform-element.ttl"^^xsd:anyURI ;
    urnp:categoricalCollection <https://linked.data.gov.au/def/nrm/c1a58967-cb12-4c2c-a7ca-9cee2589919c> ;
    urnp:categoricalConcept <https://linked.data.gov.au/def/nrm/cb894c58-d482-5471-a16d-eabb27d6cc5f> ;
    urnp:conceptDefinition "Large flat subject to inundation by water that is usually salt or brackish; aggradedby tides. An intertidal flat (ITF) is frequently inundated; a supratidal flat (STF) is seldom inundated." ;
    urnp:conceptIdentifier 76 ;
    urnp:conceptNotation "TDF" ;
    urnp:conceptSource <https://core.vocabs.paratoo.tern.org.au/api/lut-landform-elements> ;
.

<https://linked.data.gov.au/def/nrm/3b244d0e-69c3-5d45-b551-ef0d8daabd43>
    a urnc:CategoricalConceptMeta ;
    schema:url "https://github.com/ternaustralia/dawe-rlp-vocabs/tree/main/vocab_files/categorical_collections/luts/landform-element.ttl"^^xsd:anyURI ;
    urnp:categoricalCollection <https://linked.data.gov.au/def/nrm/c1a58967-cb12-4c2c-a7ca-9cee2589919c> ;
    urnp:categoricalConcept <https://linked.data.gov.au/def/nrm/283386fa-c297-5d2a-b453-fca857ddf51d> ;
    urnp:conceptDefinition "(i) Short; very gently inclined to level minimal mid-slope in an embankment or cut face; eroded or aggraded by human activity. (ii) Flat built up by waves above a beach." ;
    urnp:conceptIdentifier 9 ;
    urnp:conceptNotation "BER" ;
    urnp:conceptSource <https://core.vocabs.paratoo.tern.org.au/api/lut-landform-elements> ;
.

<https://linked.data.gov.au/def/nrm/40a5364e-049d-5e96-a5fb-a281372f0d81>
    a urnc:CategoricalConceptMeta ;
    schema:url "https://github.com/ternaustralia/dawe-rlp-vocabs/tree/main/vocab_files/categorical_collections/luts/landform-element.ttl"^^xsd:anyURI ;
    urnp:categoricalCollection <https://linked.data.gov.au/def/nrm/c1a58967-cb12-4c2c-a7ca-9cee2589919c> ;
    urnp:categoricalConcept <https://linked.data.gov.au/def/nrm/a19a72a0-2433-5fd2-8f64-16503637b9ee> ;
    urnp:conceptDefinition "Very gently to moderately inclined rises or hillocks built up or eroded by wind and lacking distinct orientation or regular pattern." ;
    urnp:conceptIdentifier 37 ;
    urnp:conceptNotation "DUH" ;
    urnp:conceptSource <https://core.vocabs.paratoo.tern.org.au/api/lut-landform-elements> ;
.

<https://linked.data.gov.au/def/nrm/435c0396-dbb2-5f3f-8b1a-01b8262901c6>
    a urnc:CategoricalConceptMeta ;
    schema:url "https://github.com/ternaustralia/dawe-rlp-vocabs/tree/main/vocab_files/categorical_collections/luts/landform-element.ttl"^^xsd:anyURI ;
    urnp:categoricalCollection <https://linked.data.gov.au/def/nrm/c1a58967-cb12-4c2c-a7ca-9cee2589919c> ;
    urnp:categoricalConcept <https://linked.data.gov.au/def/nrm/1fc7edc1-8d57-568f-9a98-9ab9ddcf2816> ;
    urnp:conceptDefinition "Large; sharp-crested; elongated; longitudinal (linear) dune or chain of sand dunes; oriented parallel; rather than transverse (perpendicular); to the prevailing wind. Not to be confused with the trailing arms of parabolic dunes." ;
    urnp:conceptIdentifier 43 ;
    urnp:conceptNotation "DUF" ;
    urnp:conceptSource <https://core.vocabs.paratoo.tern.org.au/api/lut-landform-elements> ;
.

<https://linked.data.gov.au/def/nrm/4e7b818a-a4b7-5f47-b638-67ae01575c90>
    a urnc:CategoricalConceptMeta ;
    schema:url "https://github.com/ternaustralia/dawe-rlp-vocabs/tree/main/vocab_files/categorical_collections/luts/landform-element.ttl"^^xsd:anyURI ;
    urnp:categoricalCollection <https://linked.data.gov.au/def/nrm/c1a58967-cb12-4c2c-a7ca-9cee2589919c> ;
    urnp:categoricalConcept <https://linked.data.gov.au/def/nrm/d901256e-66ab-5e26-a806-17a6ab335ae7> ;
    urnp:conceptDefinition "(i) Linear; level-floored open depression excavated by wind; or left relict between ridges built up by wind or waves; or built up to a lesser height than them. (ii) Long; curved open or closed depression left relict between scrolls built up by channelled stream flow." ;
    urnp:conceptIdentifier 70 ;
    urnp:conceptNotation "SWL" ;
    urnp:conceptSource <https://core.vocabs.paratoo.tern.org.au/api/lut-landform-elements> ;
.

<https://linked.data.gov.au/def/nrm/4fd6db54-73f3-5ece-b8a7-a7e56c1afdcc>
    a urnc:CategoricalConceptMeta ;
    schema:url "https://github.com/ternaustralia/dawe-rlp-vocabs/tree/main/vocab_files/categorical_collections/luts/landform-element.ttl"^^xsd:anyURI ;
    urnp:categoricalCollection <https://linked.data.gov.au/def/nrm/c1a58967-cb12-4c2c-a7ca-9cee2589919c> ;
    urnp:categoricalConcept <https://linked.data.gov.au/def/nrm/47eeb3d4-8cd0-50b5-b837-4a54a22e3f31> ;
    urnp:conceptDefinition "Flat eroded by human activity." ;
    urnp:conceptIdentifier 20 ;
    urnp:conceptNotation "COS" ;
    urnp:conceptSource <https://core.vocabs.paratoo.tern.org.au/api/lut-landform-elements> ;
.

<https://linked.data.gov.au/def/nrm/5083d690-4761-555e-a1c0-d6a1cb08ae97>
    a urnc:CategoricalConceptMeta ;
    schema:url "https://github.com/ternaustralia/dawe-rlp-vocabs/tree/main/vocab_files/categorical_collections/luts/landform-element.ttl"^^xsd:anyURI ;
    urnp:categoricalCollection <https://linked.data.gov.au/def/nrm/c1a58967-cb12-4c2c-a7ca-9cee2589919c> ;
    urnp:categoricalConcept <https://linked.data.gov.au/def/nrm/4ee55457-4922-5d00-b13d-ca381ad44f63> ;
    urnp:conceptDefinition "Hillock of very low to extremely low relief (<30 m) and very gentle to steep slopes. This term is used to refer to an isolated rise surrounded by other landforms." ;
    urnp:conceptIdentifier 55 ;
    urnp:conceptNotation "RER" ;
    urnp:conceptSource <https://core.vocabs.paratoo.tern.org.au/api/lut-landform-elements> ;
.

<https://linked.data.gov.au/def/nrm/51183458-2bce-5047-a2a6-17cdea865fc9>
    a urnc:CategoricalConceptMeta ;
    schema:url "https://github.com/ternaustralia/dawe-rlp-vocabs/tree/main/vocab_files/categorical_collections/luts/landform-element.ttl"^^xsd:anyURI ;
    urnp:categoricalCollection <https://linked.data.gov.au/def/nrm/c1a58967-cb12-4c2c-a7ca-9cee2589919c> ;
    urnp:categoricalConcept <https://linked.data.gov.au/def/nrm/41df86fc-66ec-5ef5-a605-edbe1b3c5edc> ;
    urnp:conceptDefinition "Very wide; cliffed (greater than 72 degrees) maximal slope usually eroded by gravitational fall as a result of erosion of the base by various agencies; sometimes built up by marine organisms." ;
    urnp:conceptIdentifier 14 ;
    urnp:conceptNotation "CLI" ;
    urnp:conceptSource <https://core.vocabs.paratoo.tern.org.au/api/lut-landform-elements> ;
.

<https://linked.data.gov.au/def/nrm/5316c0f4-4c8c-583a-bc88-db10c3ca9987>
    a urnc:CategoricalConceptMeta ;
    schema:url "https://github.com/ternaustralia/dawe-rlp-vocabs/tree/main/vocab_files/categorical_collections/luts/landform-element.ttl"^^xsd:anyURI ;
    urnp:categoricalCollection <https://linked.data.gov.au/def/nrm/c1a58967-cb12-4c2c-a7ca-9cee2589919c> ;
    urnp:categoricalConcept <https://linked.data.gov.au/def/nrm/368641eb-467f-570b-9846-e8ebccb10186> ;
    urnp:conceptDefinition "Very wide; level to gently inclined crest with abrupt margins; commonly eroded by water-aided mass movement or sheet wash." ;
    urnp:conceptIdentifier 68 ;
    urnp:conceptNotation "SUS" ;
    urnp:conceptSource <https://core.vocabs.paratoo.tern.org.au/api/lut-landform-elements> ;
.

<https://linked.data.gov.au/def/nrm/584cf753-d739-5040-851d-872add4a2e52>
    a urnc:CategoricalConceptMeta ;
    schema:url "https://github.com/ternaustralia/dawe-rlp-vocabs/tree/main/vocab_files/categorical_collections/luts/landform-element.ttl"^^xsd:anyURI ;
    urnp:categoricalCollection <https://linked.data.gov.au/def/nrm/c1a58967-cb12-4c2c-a7ca-9cee2589919c> ;
    urnp:categoricalConcept <https://linked.data.gov.au/def/nrm/b4c53a4f-3e36-507e-8f29-6468c146cd3c> ;
    urnp:conceptDefinition "Steep-sided; circular or elliptical closed depression; commonly funnel-shaped; characterised by subsurface drainage and formed by collapse of underlying caves within bedrock." ;
    urnp:conceptIdentifier 16 ;
    urnp:conceptNotation "DOC" ;
    urnp:conceptSource <https://core.vocabs.paratoo.tern.org.au/api/lut-landform-elements> ;
.

<https://linked.data.gov.au/def/nrm/5f8d5903-968d-5e8a-bc39-c7fb5d82ee1c>
    a urnc:CategoricalConceptMeta ;
    schema:url "https://github.com/ternaustralia/dawe-rlp-vocabs/tree/main/vocab_files/categorical_collections/luts/landform-element.ttl"^^xsd:anyURI ;
    urnp:categoricalCollection <https://linked.data.gov.au/def/nrm/c1a58967-cb12-4c2c-a7ca-9cee2589919c> ;
    urnp:categoricalConcept <https://linked.data.gov.au/def/nrm/496d5410-d95c-5fe0-9b67-f9364550c4e4> ;
    urnp:conceptDefinition "Large or very large flat aggraded by channelled or overbank stream flow; standing above a scarp and no longer frequently inundated; part of a former flood plain." ;
    urnp:conceptIdentifier 74 ;
    urnp:conceptNotation "TEP" ;
    urnp:conceptSource <https://core.vocabs.paratoo.tern.org.au/api/lut-landform-elements> ;
.

<https://linked.data.gov.au/def/nrm/602d9ed2-71be-56b3-9c68-04a92162a5c0>
    a urnc:CategoricalConceptMeta ;
    schema:url "https://github.com/ternaustralia/dawe-rlp-vocabs/tree/main/vocab_files/categorical_collections/luts/landform-element.ttl"^^xsd:anyURI ;
    urnp:categoricalCollection <https://linked.data.gov.au/def/nrm/c1a58967-cb12-4c2c-a7ca-9cee2589919c> ;
    urnp:categoricalConcept <https://linked.data.gov.au/def/nrm/5de0ce45-d559-57b0-8328-83e133672104> ;
    urnp:conceptDefinition "Level to gently inclined; long; narrow shallow open depression with smoothly concave cross-section rising to moderately inclined side slopes; eroded or aggraded by sheet wash." ;
    urnp:conceptIdentifier 23 ;
    urnp:conceptNotation "DDE" ;
    urnp:conceptSource <https://core.vocabs.paratoo.tern.org.au/api/lut-landform-elements> ;
.

<https://linked.data.gov.au/def/nrm/6587cbb1-a6cf-5bad-bb8d-313607ae1f11>
    a urnc:CategoricalConceptMeta ;
    schema:url "https://github.com/ternaustralia/dawe-rlp-vocabs/tree/main/vocab_files/categorical_collections/luts/landform-element.ttl"^^xsd:anyURI ;
    urnp:categoricalCollection <https://linked.data.gov.au/def/nrm/c1a58967-cb12-4c2c-a7ca-9cee2589919c> ;
    urnp:categoricalConcept <https://linked.data.gov.au/def/nrm/287d64df-98f4-58c3-950e-2356a15687fd> ;
    urnp:conceptDefinition "Crescent shaped dune with tips extending leeward (downwind); making this side concave and the windward (upwind) side convex. Barchan dunes tend to be arranged in chains extending in the dominant wind direction." ;
    urnp:conceptIdentifier 5 ;
    urnp:conceptNotation "DUB" ;
    urnp:conceptSource <https://core.vocabs.paratoo.tern.org.au/api/lut-landform-elements> ;
.

<https://linked.data.gov.au/def/nrm/6945adab-6973-559f-90ce-04f454dcf18b>
    a urnc:CategoricalConceptMeta ;
    schema:url "https://github.com/ternaustralia/dawe-rlp-vocabs/tree/main/vocab_files/categorical_collections/luts/landform-element.ttl"^^xsd:anyURI ;
    urnp:categoricalCollection <https://linked.data.gov.au/def/nrm/c1a58967-cb12-4c2c-a7ca-9cee2589919c> ;
    urnp:categoricalConcept <https://linked.data.gov.au/def/nrm/8e448737-8d60-56a6-94df-9399d5b9e174> ;
    urnp:conceptDefinition "Basin excavated by wind erosion which removes loose material; commonly above a resistant or wet layer." ;
    urnp:conceptIdentifier 22 ;
    urnp:conceptNotation "DBA" ;
    urnp:conceptSource <https://core.vocabs.paratoo.tern.org.au/api/lut-landform-elements> ;
.

<https://linked.data.gov.au/def/nrm/6cd065ab-bc16-5f20-817d-ba9deff03e0d>
    a urnc:CategoricalConceptMeta ;
    schema:url "https://github.com/ternaustralia/dawe-rlp-vocabs/tree/main/vocab_files/categorical_collections/luts/landform-element.ttl"^^xsd:anyURI ;
    urnp:categoricalCollection <https://linked.data.gov.au/def/nrm/c1a58967-cb12-4c2c-a7ca-9cee2589919c> ;
    urnp:categoricalConcept <https://linked.data.gov.au/def/nrm/64008844-d6ff-5fa3-9218-48a3d57ada21> ;
    urnp:conceptDefinition "Small flat aggraded or eroded by channelled or overbank stream flow; standing above a scarp and no longer frequently inundated; a former valley flat or part of a former flood plain." ;
    urnp:conceptIdentifier 73 ;
    urnp:conceptNotation "TEF" ;
    urnp:conceptSource <https://core.vocabs.paratoo.tern.org.au/api/lut-landform-elements> ;
.

<https://linked.data.gov.au/def/nrm/6dc7e12f-cb45-5602-9ac8-83f9e9fbbab7>
    a urnc:CategoricalConceptMeta ;
    schema:url "https://github.com/ternaustralia/dawe-rlp-vocabs/tree/main/vocab_files/categorical_collections/luts/landform-element.ttl"^^xsd:anyURI ;
    urnp:categoricalCollection <https://linked.data.gov.au/def/nrm/c1a58967-cb12-4c2c-a7ca-9cee2589919c> ;
    urnp:categoricalConcept <https://linked.data.gov.au/def/nrm/a749658e-2521-5fe0-8aaf-e352c3639fc1> ;
    urnp:conceptDefinition "Very long; low; narrow; nearly level; sinuous ridge immediately adjacent to a stream channel; built up by overbank flow. Levees are built usually in pairs bounding the two sides of a stream channel; at the level reached by frequent floods. This element is part of a covered plain landform pattern. For an artificial levee; use Embankment. See also Prior stream." ;
    urnp:conceptIdentifier 42 ;
    urnp:conceptNotation "LEV" ;
    urnp:conceptSource <https://core.vocabs.paratoo.tern.org.au/api/lut-landform-elements> ;
.

<https://linked.data.gov.au/def/nrm/6e63d4d1-e472-5c46-b6c8-a8275a01f845>
    a urnc:CategoricalConceptMeta ;
    schema:url "https://github.com/ternaustralia/dawe-rlp-vocabs/tree/main/vocab_files/categorical_collections/luts/landform-element.ttl"^^xsd:anyURI ;
    urnp:categoricalCollection <https://linked.data.gov.au/def/nrm/c1a58967-cb12-4c2c-a7ca-9cee2589919c> ;
    urnp:categoricalConcept <https://linked.data.gov.au/def/nrm/f823af68-b200-57b2-9d6e-c1f15f01b4a4> ;
    urnp:conceptDefinition "Small; gently inclined to level flat; aggraded or sometimes eroded by channelled or overbank stream flow; typically enclosed by hillslopes; a miniature alluvial plain landform pattern." ;
    urnp:conceptIdentifier 80 ;
    urnp:conceptNotation "VLF" ;
    urnp:conceptSource <https://core.vocabs.paratoo.tern.org.au/api/lut-landform-elements> ;
.

<https://linked.data.gov.au/def/nrm/7317acd5-1490-5367-a6df-05e606050ab2>
    a urnc:CategoricalConceptMeta ;
    schema:url "https://github.com/ternaustralia/dawe-rlp-vocabs/tree/main/vocab_files/categorical_collections/luts/landform-element.ttl"^^xsd:anyURI ;
    urnp:categoricalCollection <https://linked.data.gov.au/def/nrm/c1a58967-cb12-4c2c-a7ca-9cee2589919c> ;
    urnp:categoricalConcept <https://linked.data.gov.au/def/nrm/5cd65691-a295-577c-9f94-cd4756337e3f> ;
    urnp:conceptDefinition "Elongated; gently curved; low ridge built up by wind on the margin of a playa; typically with a moderate; wave-modified slope towards the playa and a gentle outer slope." ;
    urnp:conceptIdentifier 44 ;
    urnp:conceptNotation "LUN" ;
    urnp:conceptSource <https://core.vocabs.paratoo.tern.org.au/api/lut-landform-elements> ;
.

<https://linked.data.gov.au/def/nrm/74034049-2f3d-5285-b5de-7b3721d01f3d>
    a urnc:CategoricalConceptMeta ;
    schema:url "https://github.com/ternaustralia/dawe-rlp-vocabs/tree/main/vocab_files/categorical_collections/luts/landform-element.ttl"^^xsd:anyURI ;
    urnp:categoricalCollection <https://linked.data.gov.au/def/nrm/c1a58967-cb12-4c2c-a7ca-9cee2589919c> ;
    urnp:categoricalConcept <https://linked.data.gov.au/def/nrm/130cad8e-0a82-515a-ad75-6b84d165db6c> ;
    urnp:conceptDefinition "Steep-sided; circular or elliptical closed depression; commonly funnel-shaped; characterised by subsurface drainage and formed by dissolution of the surface or underlying within bedrock." ;
    urnp:conceptIdentifier 65 ;
    urnp:conceptNotation "DOL" ;
    urnp:conceptSource <https://core.vocabs.paratoo.tern.org.au/api/lut-landform-elements> ;
.

<https://linked.data.gov.au/def/nrm/75b3cf6d-7625-59de-9d4b-83a2220db206>
    a urnc:CategoricalConceptMeta ;
    schema:url "https://github.com/ternaustralia/dawe-rlp-vocabs/tree/main/vocab_files/categorical_collections/luts/landform-element.ttl"^^xsd:anyURI ;
    urnp:categoricalCollection <https://linked.data.gov.au/def/nrm/c1a58967-cb12-4c2c-a7ca-9cee2589919c> ;
    urnp:categoricalConcept <https://linked.data.gov.au/def/nrm/e13edfb1-b27f-5f73-ac06-bb40b2520684> ;
    urnp:conceptDefinition "Usually small; open or closed depression excavated by the wind." ;
    urnp:conceptIdentifier 10 ;
    urnp:conceptNotation "BOU" ;
    urnp:conceptSource <https://core.vocabs.paratoo.tern.org.au/api/lut-landform-elements> ;
.

<https://linked.data.gov.au/def/nrm/76e33646-90e7-5181-8f19-971161b50bc4>
    a urnc:CategoricalConceptMeta ;
    schema:url "https://github.com/ternaustralia/dawe-rlp-vocabs/tree/main/vocab_files/categorical_collections/luts/landform-element.ttl"^^xsd:anyURI ;
    urnp:categoricalCollection <https://linked.data.gov.au/def/nrm/c1a58967-cb12-4c2c-a7ca-9cee2589919c> ;
    urnp:categoricalConcept <https://linked.data.gov.au/def/nrm/e31ccd59-0ce4-56ad-87a9-4e7a1cda9605> ;
    urnp:conceptDefinition "Open depression excavated by human activity." ;
    urnp:conceptIdentifier 78 ;
    urnp:conceptNotation "TRE" ;
    urnp:conceptSource <https://core.vocabs.paratoo.tern.org.au/api/lut-landform-elements> ;
.

<https://linked.data.gov.au/def/nrm/7987ec07-7798-58e6-ba90-d1eef7ccca57>
    a urnc:CategoricalConceptMeta ;
    schema:url "https://github.com/ternaustralia/dawe-rlp-vocabs/tree/main/vocab_files/categorical_collections/luts/landform-element.ttl"^^xsd:anyURI ;
    urnp:categoricalCollection <https://linked.data.gov.au/def/nrm/c1a58967-cb12-4c2c-a7ca-9cee2589919c> ;
    urnp:categoricalConcept <https://linked.data.gov.au/def/nrm/63960cfe-9e04-52b7-8940-4d6c2ebe0a02> ;
    urnp:conceptDefinition "Short; low; very wide slope; gently or moderately inclined; built up or eroded by waves; forming the shore of a lake or sea." ;
    urnp:conceptIdentifier 6 ;
    urnp:conceptNotation "BEA" ;
    urnp:conceptSource <https://core.vocabs.paratoo.tern.org.au/api/lut-landform-elements> ;
.

<https://linked.data.gov.au/def/nrm/7a751103-0da3-517a-b8fd-6f1d23a11fac>
    a urnc:CategoricalConceptMeta ;
    schema:url "https://github.com/ternaustralia/dawe-rlp-vocabs/tree/main/vocab_files/categorical_collections/luts/landform-element.ttl"^^xsd:anyURI ;
    urnp:categoricalCollection <https://linked.data.gov.au/def/nrm/c1a58967-cb12-4c2c-a7ca-9cee2589919c> ;
    urnp:categoricalConcept <https://linked.data.gov.au/def/nrm/1ed7b887-8971-5d45-8ada-48e18386de45> ;
    urnp:conceptDefinition "Very long; nearly straight moderately inclined to very steep ridge built up by the wind from material from an adjacent beach." ;
    urnp:conceptIdentifier 33 ;
    urnp:conceptNotation "FOR" ;
    urnp:conceptSource <https://core.vocabs.paratoo.tern.org.au/api/lut-landform-elements> ;
.

<https://linked.data.gov.au/def/nrm/7a751c07-1647-5385-9d99-4d4a2ccfee99>
    a urnc:CategoricalConceptMeta ;
    schema:url "https://github.com/ternaustralia/dawe-rlp-vocabs/tree/main/vocab_files/categorical_collections/luts/landform-element.ttl"^^xsd:anyURI ;
    urnp:categoricalCollection <https://linked.data.gov.au/def/nrm/c1a58967-cb12-4c2c-a7ca-9cee2589919c> ;
    urnp:categoricalConcept <https://linked.data.gov.au/def/nrm/c1c77cbf-4251-5437-b8c8-c3e44304f023> ;
    urnp:conceptDefinition "Steep to precipitous hillock; typically convex; with a surface mainly of bare rock; either coherent or comprising subangular to rounded; large boulders (exhumed core-stones; also themselves called tors) separated by open fissures; eroded by sheet wash or water-aided mass movement." ;
    urnp:conceptIdentifier 77 ;
    urnp:conceptNotation "TOR" ;
    urnp:conceptSource <https://core.vocabs.paratoo.tern.org.au/api/lut-landform-elements> ;
.

<https://linked.data.gov.au/def/nrm/82b726cd-c6b3-5653-8e29-522959cb701e>
    a urnc:CategoricalConceptMeta ;
    schema:url "https://github.com/ternaustralia/dawe-rlp-vocabs/tree/main/vocab_files/categorical_collections/luts/landform-element.ttl"^^xsd:anyURI ;
    urnp:categoricalCollection <https://linked.data.gov.au/def/nrm/c1a58967-cb12-4c2c-a7ca-9cee2589919c> ;
    urnp:categoricalConcept <https://linked.data.gov.au/def/nrm/032a1c8b-1048-5c81-bd06-8afce5c12451> ;
    urnp:conceptDefinition "Slope built up or eroded by the wind (see Dune)." ;
    urnp:conceptIdentifier 26 ;
    urnp:conceptNotation "DUS" ;
    urnp:conceptSource <https://core.vocabs.paratoo.tern.org.au/api/lut-landform-elements> ;
.

<https://linked.data.gov.au/def/nrm/869ecf37-5e73-5692-951d-a474f612f466>
    a urnc:CategoricalConceptMeta ;
    schema:url "https://github.com/ternaustralia/dawe-rlp-vocabs/tree/main/vocab_files/categorical_collections/luts/landform-element.ttl"^^xsd:anyURI ;
    urnp:categoricalCollection <https://linked.data.gov.au/def/nrm/c1a58967-cb12-4c2c-a7ca-9cee2589919c> ;
    urnp:categoricalConcept <https://linked.data.gov.au/def/nrm/d85de894-c9f3-545d-a131-906301d4ff91> ;
    urnp:conceptDefinition "Long; curved; very low ridge built up by channelled stream flow and left relict by channel migration. Part of a meander plain landform pattern." ;
    urnp:conceptIdentifier 63 ;
    urnp:conceptNotation "SCR" ;
    urnp:conceptSource <https://core.vocabs.paratoo.tern.org.au/api/lut-landform-elements> ;
.

<https://linked.data.gov.au/def/nrm/8a947829-cd2f-51b7-9165-4d0daf9ce69a>
    a urnc:CategoricalConceptMeta ;
    schema:url "https://github.com/ternaustralia/dawe-rlp-vocabs/tree/main/vocab_files/categorical_collections/luts/landform-element.ttl"^^xsd:anyURI ;
    urnp:categoricalCollection <https://linked.data.gov.au/def/nrm/c1a58967-cb12-4c2c-a7ca-9cee2589919c> ;
    urnp:categoricalConcept <https://linked.data.gov.au/def/nrm/6ff1c19e-cd58-5c14-b39d-6c093ba8b994> ;
    urnp:conceptDefinition "Flat inclined radially away from a point on the margin or at the end of a stream channel; aggraded by overbank stream flow; or by channelled stream flow associated with channels developed within the overbank flow; part of a covered plain landform pattern." ;
    urnp:conceptIdentifier 31 ;
    urnp:conceptNotation "FLD" ;
    urnp:conceptSource <https://core.vocabs.paratoo.tern.org.au/api/lut-landform-elements> ;
.

<https://linked.data.gov.au/def/nrm/8c55054a-3230-5d27-9b48-e380f276bd3c>
    a urnc:CategoricalConceptMeta ;
    schema:url "https://github.com/ternaustralia/dawe-rlp-vocabs/tree/main/vocab_files/categorical_collections/luts/landform-element.ttl"^^xsd:anyURI ;
    urnp:categoricalCollection <https://linked.data.gov.au/def/nrm/c1a58967-cb12-4c2c-a7ca-9cee2589919c> ;
    urnp:categoricalConcept <https://linked.data.gov.au/def/nrm/d110a3b2-a34f-5d94-828d-e539c22ae2b5> ;
    urnp:conceptDefinition "Very short; very wide slope; moderately inclined to precipitous; forming the marginal upper parts of a stream channel and resulting from erosion or aggradation by channelled stream flow." ;
    urnp:conceptIdentifier 3 ;
    urnp:conceptNotation "BAN" ;
    urnp:conceptSource <https://core.vocabs.paratoo.tern.org.au/api/lut-landform-elements> ;
.

<https://linked.data.gov.au/def/nrm/93ec996a-efcc-55eb-9326-df8acb2bc927>
    a urnc:CategoricalConceptMeta ;
    schema:url "https://github.com/ternaustralia/dawe-rlp-vocabs/tree/main/vocab_files/categorical_collections/luts/landform-element.ttl"^^xsd:anyURI ;
    urnp:categoricalCollection <https://linked.data.gov.au/def/nrm/c1a58967-cb12-4c2c-a7ca-9cee2589919c> ;
    urnp:categoricalConcept <https://linked.data.gov.au/def/nrm/141a8baa-89e0-5a55-b9fd-05a3c0b8c79c> ;
    urnp:conceptDefinition "Slope situated below a cliff; with its contours generally parallel to the line of the cliff eroded by sheet wash or water-aided mass movement; and aggraded locally by collapsed material from above." ;
    urnp:conceptIdentifier 15 ;
    urnp:conceptNotation "CFS" ;
    urnp:conceptSource <https://core.vocabs.paratoo.tern.org.au/api/lut-landform-elements> ;
.

<https://linked.data.gov.au/def/nrm/960df542-0451-5092-96a5-6a9dd22b1118>
    a urnc:CategoricalConceptMeta ;
    schema:url "https://github.com/ternaustralia/dawe-rlp-vocabs/tree/main/vocab_files/categorical_collections/luts/landform-element.ttl"^^xsd:anyURI ;
    urnp:categoricalCollection <https://linked.data.gov.au/def/nrm/c1a58967-cb12-4c2c-a7ca-9cee2589919c> ;
    urnp:categoricalConcept <https://linked.data.gov.au/def/nrm/9da5cf89-4487-5f93-b351-0782a42ae362> ;
    urnp:conceptDefinition "Short; gently or very gently inclined minimal mid-slope element eroded or aggraded by any agent." ;
    urnp:conceptIdentifier 8 ;
    urnp:conceptNotation "BEN" ;
    urnp:conceptSource <https://core.vocabs.paratoo.tern.org.au/api/lut-landform-elements> ;
.

<https://linked.data.gov.au/def/nrm/986f781e-5da7-55bc-ae10-8c97d9d54910>
    a urnc:CategoricalConceptMeta ;
    schema:url "https://github.com/ternaustralia/dawe-rlp-vocabs/tree/main/vocab_files/categorical_collections/luts/landform-element.ttl"^^xsd:anyURI ;
    urnp:categoricalCollection <https://linked.data.gov.au/def/nrm/c1a58967-cb12-4c2c-a7ca-9cee2589919c> ;
    urnp:categoricalConcept <https://linked.data.gov.au/def/nrm/d7154911-ea70-5613-9b4d-8fb80b36cda0> ;
    urnp:conceptDefinition "Large; very gently inclined or level element; of unspecified geomorphological agent or mode of activity." ;
    urnp:conceptIdentifier 51 ;
    urnp:conceptNotation "PLA" ;
    urnp:conceptSource <https://core.vocabs.paratoo.tern.org.au/api/lut-landform-elements> ;
.

<https://linked.data.gov.au/def/nrm/98cf6325-95bf-575d-bf79-e4536646e7ff>
    a urnc:CategoricalConceptMeta ;
    schema:url "https://github.com/ternaustralia/dawe-rlp-vocabs/tree/main/vocab_files/categorical_collections/luts/landform-element.ttl"^^xsd:anyURI ;
    urnp:categoricalCollection <https://linked.data.gov.au/def/nrm/c1a58967-cb12-4c2c-a7ca-9cee2589919c> ;
    urnp:categoricalConcept <https://linked.data.gov.au/def/nrm/55911768-52b3-5fff-b4cf-2dd0614583c0> ;
    urnp:conceptDefinition "Hillock built up by human activity." ;
    urnp:conceptIdentifier 46 ;
    urnp:conceptNotation "MOU" ;
    urnp:conceptSource <https://core.vocabs.paratoo.tern.org.au/api/lut-landform-elements> ;
.

<https://linked.data.gov.au/def/nrm/9a9295db-de60-5066-ad35-917678cae36d>
    a urnc:CategoricalConceptMeta ;
    schema:url "https://github.com/ternaustralia/dawe-rlp-vocabs/tree/main/vocab_files/categorical_collections/luts/landform-element.ttl"^^xsd:anyURI ;
    urnp:categoricalCollection <https://linked.data.gov.au/def/nrm/c1a58967-cb12-4c2c-a7ca-9cee2589919c> ;
    urnp:categoricalConcept <https://linked.data.gov.au/def/nrm/9969b531-7f6c-54a6-a23c-123c332d3428> ;
    urnp:conceptDefinition "Crest of hillock of very low to extremely low relief (<30 m) (see Residual rise)." ;
    urnp:conceptIdentifier 56 ;
    urnp:conceptNotation "REC" ;
    urnp:conceptSource <https://core.vocabs.paratoo.tern.org.au/api/lut-landform-elements> ;
.

<https://linked.data.gov.au/def/nrm/9da6a4ed-27a1-5c30-87b6-84e4a56dba99>
    a urnc:CategoricalConceptMeta ;
    schema:url "https://github.com/ternaustralia/dawe-rlp-vocabs/tree/main/vocab_files/categorical_collections/luts/landform-element.ttl"^^xsd:anyURI ;
    urnp:categoricalCollection <https://linked.data.gov.au/def/nrm/c1a58967-cb12-4c2c-a7ca-9cee2589919c> ;
    urnp:categoricalConcept <https://linked.data.gov.au/def/nrm/4524d1f6-1951-502e-b7fe-8439acd3448a> ;
    urnp:conceptDefinition "Large; gently inclined to level element with radial slope lines inclined away from a point; resulting from aggradation; or occasionally from erosion; by channelled; often braided; stream flow; or possibly by sheet flow." ;
    urnp:conceptIdentifier 29 ;
    urnp:conceptNotation "FAN" ;
    urnp:conceptSource <https://core.vocabs.paratoo.tern.org.au/api/lut-landform-elements> ;
.

<https://linked.data.gov.au/def/nrm/9e22fdaf-48e4-5172-bb86-95545f600e7d>
    a urnc:CategoricalConceptMeta ;
    schema:url "https://github.com/ternaustralia/dawe-rlp-vocabs/tree/main/vocab_files/categorical_collections/luts/landform-element.ttl"^^xsd:anyURI ;
    urnp:categoricalCollection <https://linked.data.gov.au/def/nrm/c1a58967-cb12-4c2c-a7ca-9cee2589919c> ;
    urnp:categoricalConcept <https://linked.data.gov.au/def/nrm/1958c732-bbdd-5984-acec-5f56c2b82a06> ;
    urnp:conceptDefinition "Flat aggraded by human activity." ;
    urnp:conceptIdentifier 30 ;
    urnp:conceptNotation "FIL" ;
    urnp:conceptSource <https://core.vocabs.paratoo.tern.org.au/api/lut-landform-elements> ;
.

<https://linked.data.gov.au/def/nrm/a4338ea4-ce49-56df-b773-8c33a9b528b2>
    a urnc:CategoricalConceptMeta ;
    schema:url "https://github.com/ternaustralia/dawe-rlp-vocabs/tree/main/vocab_files/categorical_collections/luts/landform-element.ttl"^^xsd:anyURI ;
    urnp:categoricalCollection <https://linked.data.gov.au/def/nrm/c1a58967-cb12-4c2c-a7ca-9cee2589919c> ;
    urnp:categoricalConcept <https://linked.data.gov.au/def/nrm/b357ae54-1094-5957-bf45-500ceab54a37> ;
    urnp:conceptDefinition "Level-floored; commonly water-filled closed depression with a nearly circular; steep rim; excavated by volcanism." ;
    urnp:conceptIdentifier 45 ;
    urnp:conceptNotation "MAA" ;
    urnp:conceptSource <https://core.vocabs.paratoo.tern.org.au/api/lut-landform-elements> ;
.

<https://linked.data.gov.au/def/nrm/a7b6a6b8-0b0b-5f51-8706-1ad35851a117>
    a urnc:CategoricalConceptMeta ;
    schema:url "https://github.com/ternaustralia/dawe-rlp-vocabs/tree/main/vocab_files/categorical_collections/luts/landform-element.ttl"^^xsd:anyURI ;
    urnp:categoricalCollection <https://linked.data.gov.au/def/nrm/c1a58967-cb12-4c2c-a7ca-9cee2589919c> ;
    urnp:categoricalConcept <https://linked.data.gov.au/def/nrm/7cb2f197-c3e8-5491-b0db-78b839405fd7> ;
    urnp:conceptDefinition "Stream channel close to its junction with a sea or lake; where the action of channelled stream flow is modified by tide and waves. The width typically increases downstream." ;
    urnp:conceptIdentifier 28 ;
    urnp:conceptNotation "EST" ;
    urnp:conceptSource <https://core.vocabs.paratoo.tern.org.au/api/lut-landform-elements> ;
.

<https://linked.data.gov.au/def/nrm/b1887a7f-1df3-5b72-8494-a12009faf955>
    a urnc:CategoricalConceptMeta ;
    schema:url "https://github.com/ternaustralia/dawe-rlp-vocabs/tree/main/vocab_files/categorical_collections/luts/landform-element.ttl"^^xsd:anyURI ;
    urnp:categoricalCollection <https://linked.data.gov.au/def/nrm/c1a58967-cb12-4c2c-a7ca-9cee2589919c> ;
    urnp:categoricalConcept <https://linked.data.gov.au/def/nrm/4b14473a-033a-58f1-b02c-16f47da90265> ;
    urnp:conceptDefinition "Almost level; closed or almost closed depression with a seasonal or permanent watertable at or above the surface; commonly aggraded by overbank stream flow and sometimes biological (peat) accumulation." ;
    urnp:conceptIdentifier 71 ;
    urnp:conceptNotation "SWP" ;
    urnp:conceptSource <https://core.vocabs.paratoo.tern.org.au/api/lut-landform-elements> ;
.

<https://linked.data.gov.au/def/nrm/b2139c18-0220-5fce-98d0-4847e17919cc>
    a urnc:CategoricalConceptMeta ;
    schema:url "https://github.com/ternaustralia/dawe-rlp-vocabs/tree/main/vocab_files/categorical_collections/luts/landform-element.ttl"^^xsd:anyURI ;
    urnp:categoricalCollection <https://linked.data.gov.au/def/nrm/c1a58967-cb12-4c2c-a7ca-9cee2589919c> ;
    urnp:categoricalConcept <https://linked.data.gov.au/def/nrm/115cecfd-35f7-51bf-b884-6267b453f50a> ;
    urnp:conceptDefinition "Very wide; steep to precipitous maximal slope eroded by gravlty; water-aided mass movement or sheet flow." ;
    urnp:conceptIdentifier 61 ;
    urnp:conceptNotation "SCA" ;
    urnp:conceptSource <https://core.vocabs.paratoo.tern.org.au/api/lut-landform-elements> ;
.

<https://linked.data.gov.au/def/nrm/b459407f-82fe-5212-80c0-dfd4e3d49531>
    a urnc:CategoricalConceptMeta ;
    schema:url "https://github.com/ternaustralia/dawe-rlp-vocabs/tree/main/vocab_files/categorical_collections/luts/landform-element.ttl"^^xsd:anyURI ;
    urnp:categoricalCollection <https://linked.data.gov.au/def/nrm/c1a58967-cb12-4c2c-a7ca-9cee2589919c> ;
    urnp:categoricalConcept <https://linked.data.gov.au/def/nrm/30bd2063-582d-5156-8ea0-faab8d16b102> ;
    urnp:conceptDefinition "Very gently inclined to steep crest; smoothly convex; eroded mainly by creep and sheet wash. A typical element of mountains; hills; low hills and rises." ;
    urnp:conceptIdentifier 35 ;
    urnp:conceptNotation "HCR" ;
    urnp:conceptSource <https://core.vocabs.paratoo.tern.org.au/api/lut-landform-elements> ;
.

<https://linked.data.gov.au/def/nrm/b6c1efcd-7bac-5d4d-aca5-f85f5b1e8a8a>
    a urnc:CategoricalConceptMeta ;
    schema:url "https://github.com/ternaustralia/dawe-rlp-vocabs/tree/main/vocab_files/categorical_collections/luts/landform-element.ttl"^^xsd:anyURI ;
    urnp:categoricalCollection <https://linked.data.gov.au/def/nrm/c1a58967-cb12-4c2c-a7ca-9cee2589919c> ;
    urnp:categoricalConcept <https://linked.data.gov.au/def/nrm/f38db675-d185-5bc3-ba02-3c30394b38dc> ;
    urnp:conceptDefinition "Elongated; gently to moderately inclined; low ridge built up by channelled stream flow; part of a stream bed." ;
    urnp:conceptIdentifier 4 ;
    urnp:conceptNotation "BAR" ;
    urnp:conceptSource <https://core.vocabs.paratoo.tern.org.au/api/lut-landform-elements> ;
.

<https://linked.data.gov.au/def/nrm/b87ac878-c02d-50ee-b04c-a82bcb3e02d6>
    a urnc:CategoricalConceptMeta ;
    schema:url "https://github.com/ternaustralia/dawe-rlp-vocabs/tree/main/vocab_files/categorical_collections/luts/landform-element.ttl"^^xsd:anyURI ;
    urnp:categoricalCollection <https://linked.data.gov.au/def/nrm/c1a58967-cb12-4c2c-a7ca-9cee2589919c> ;
    urnp:categoricalConcept <https://linked.data.gov.au/def/nrm/93fed9db-1788-54b3-8731-89430eb8f79a> ;
    urnp:conceptDefinition "Moderately inclined or steep waning lower slope; consisting of rock fragments aggraded by gravlty." ;
    urnp:conceptIdentifier 72 ;
    urnp:conceptNotation "TAL" ;
    urnp:conceptSource <https://core.vocabs.paratoo.tern.org.au/api/lut-landform-elements> ;
.

<https://linked.data.gov.au/def/nrm/bbefbe1f-e0b3-5c10-a425-a179638c5d63>
    a urnc:CategoricalConceptMeta ;
    schema:url "https://github.com/ternaustralia/dawe-rlp-vocabs/tree/main/vocab_files/categorical_collections/luts/landform-element.ttl"^^xsd:anyURI ;
    urnp:categoricalCollection <https://linked.data.gov.au/def/nrm/c1a58967-cb12-4c2c-a7ca-9cee2589919c> ;
    urnp:categoricalConcept <https://linked.data.gov.au/def/nrm/37421601-50ec-5371-b697-e9e18a54ba92> ;
    urnp:conceptDefinition "Open depression with short; precipitous walls and moderately inclined to very gently inclined floor or small stream channel; eroded by channelled stream flow and consequent collapse and water-aided mass movement." ;
    urnp:conceptIdentifier 34 ;
    urnp:conceptNotation "GUL" ;
    urnp:conceptSource <https://core.vocabs.paratoo.tern.org.au/api/lut-landform-elements> ;
.

<https://linked.data.gov.au/def/nrm/be9158a1-5d0c-5558-ab3f-6c7c1e79fb9e>
    a urnc:CategoricalConceptMeta ;
    schema:url "https://github.com/ternaustralia/dawe-rlp-vocabs/tree/main/vocab_files/categorical_collections/luts/landform-element.ttl"^^xsd:anyURI ;
    urnp:categoricalCollection <https://linked.data.gov.au/def/nrm/c1a58967-cb12-4c2c-a7ca-9cee2589919c> ;
    urnp:categoricalConcept <https://linked.data.gov.au/def/nrm/2ac8be18-9aae-56e3-aa07-65929e667648> ;
    urnp:conceptDefinition "Ridge built up by human activity so as to close a depression." ;
    urnp:conceptIdentifier 21 ;
    urnp:conceptNotation "DAM" ;
    urnp:conceptSource <https://core.vocabs.paratoo.tern.org.au/api/lut-landform-elements> ;
.

<https://linked.data.gov.au/def/nrm/bee94ec9-b2b2-5d62-91c3-eb362fcc79e3>
    a urnc:CategoricalConceptMeta ;
    schema:url "https://github.com/ternaustralia/dawe-rlp-vocabs/tree/main/vocab_files/categorical_collections/luts/landform-element.ttl"^^xsd:anyURI ;
    urnp:categoricalCollection <https://linked.data.gov.au/def/nrm/c1a58967-cb12-4c2c-a7ca-9cee2589919c> ;
    urnp:categoricalConcept <https://linked.data.gov.au/def/nrm/c21bb284-7262-5dee-bd5b-8ecfe47961a0> ;
    urnp:conceptDefinition "See Tidal flat." ;
    urnp:conceptIdentifier 38 ;
    urnp:conceptNotation "ITF" ;
    urnp:conceptSource <https://core.vocabs.paratoo.tern.org.au/api/lut-landform-elements> ;
.

<https://linked.data.gov.au/def/nrm/bf8d1824-2df8-59c8-b2e8-eadecb0ef4d2>
    a urnc:CategoricalConceptMeta ;
    schema:url "https://github.com/ternaustralia/dawe-rlp-vocabs/tree/main/vocab_files/categorical_collections/luts/landform-element.ttl"^^xsd:anyURI ;
    urnp:categoricalCollection <https://linked.data.gov.au/def/nrm/c1a58967-cb12-4c2c-a7ca-9cee2589919c> ;
    urnp:categoricalConcept <https://linked.data.gov.au/def/nrm/71bc069c-03d3-53a5-a8d7-ef6a8f039389> ;
    urnp:conceptDefinition "Linear; generally sinuous open depression forming the bottom of a stream channel; eroded and locally excavated; aggraded or built up by channelled stream flow. Parts that are built up include bars." ;
    urnp:conceptIdentifier 66 ;
    urnp:conceptNotation "STB" ;
    urnp:conceptSource <https://core.vocabs.paratoo.tern.org.au/api/lut-landform-elements> ;
.

<https://linked.data.gov.au/def/nrm/c1931b42-0124-51c1-9798-fb1488c9d84e>
    a urnc:CategoricalConceptMeta ;
    schema:url "https://github.com/ternaustralia/dawe-rlp-vocabs/tree/main/vocab_files/categorical_collections/luts/landform-element.ttl"^^xsd:anyURI ;
    urnp:categoricalCollection <https://linked.data.gov.au/def/nrm/c1a58967-cb12-4c2c-a7ca-9cee2589919c> ;
    urnp:categoricalConcept <https://linked.data.gov.au/def/nrm/eecee680-ecd8-5955-8434-dc9e7246f08d> ;
    urnp:conceptDefinition "Moderately inclined to very steep slope; eroded in the upper part and aggraded in the lower part by water-aided mass movement; characterised by irregular hummocks." ;
    urnp:conceptIdentifier 41 ;
    urnp:conceptNotation "LDS" ;
    urnp:conceptSource <https://core.vocabs.paratoo.tern.org.au/api/lut-landform-elements> ;
.

<https://linked.data.gov.au/def/nrm/d024e54c-13e3-5a3c-8617-daa69b0274c7>
    a urnc:CategoricalConceptMeta ;
    schema:url "https://github.com/ternaustralia/dawe-rlp-vocabs/tree/main/vocab_files/categorical_collections/luts/landform-element.ttl"^^xsd:anyURI ;
    urnp:categoricalCollection <https://linked.data.gov.au/def/nrm/c1a58967-cb12-4c2c-a7ca-9cee2589919c> ;
    urnp:categoricalConcept <https://linked.data.gov.au/def/nrm/548c40d1-6c33-511d-be44-0c9f4f1360da> ;
    urnp:conceptDefinition "Hillock heaved up by volcanism (or; elsewhere; built up by human activity at a burial site)." ;
    urnp:conceptIdentifier 79 ;
    urnp:conceptNotation "TUM" ;
    urnp:conceptSource <https://core.vocabs.paratoo.tern.org.au/api/lut-landform-elements> ;
.

<https://linked.data.gov.au/def/nrm/d1732611-cc2f-5e6f-846a-da0adc40a439>
    a urnc:CategoricalConceptMeta ;
    schema:url "https://github.com/ternaustralia/dawe-rlp-vocabs/tree/main/vocab_files/categorical_collections/luts/landform-element.ttl"^^xsd:anyURI ;
    urnp:categoricalCollection <https://linked.data.gov.au/def/nrm/c1a58967-cb12-4c2c-a7ca-9cee2589919c> ;
    urnp:categoricalConcept <https://linked.data.gov.au/def/nrm/a75e7c17-b8c5-50b2-a0ca-74cfc6a65229> ;
    urnp:conceptDefinition "Slope eroded by human activity." ;
    urnp:conceptIdentifier 19 ;
    urnp:conceptNotation "CUT" ;
    urnp:conceptSource <https://core.vocabs.paratoo.tern.org.au/api/lut-landform-elements> ;
.

<https://linked.data.gov.au/def/nrm/d632f875-823d-5fd3-bc6e-9741e735fe4a>
    a urnc:CategoricalConceptMeta ;
    schema:url "https://github.com/ternaustralia/dawe-rlp-vocabs/tree/main/vocab_files/categorical_collections/luts/landform-element.ttl"^^xsd:anyURI ;
    urnp:categoricalCollection <https://linked.data.gov.au/def/nrm/c1a58967-cb12-4c2c-a7ca-9cee2589919c> ;
    urnp:categoricalConcept <https://linked.data.gov.au/def/nrm/54c94292-798f-5a26-8455-d1a302756f4f> ;
    urnp:conceptDefinition "Flat; bare of vegetatiorn; from which soil has been eroded or excavated by surface wash or wind." ;
    urnp:conceptIdentifier 60 ;
    urnp:conceptNotation "SCD" ;
    urnp:conceptSource <https://core.vocabs.paratoo.tern.org.au/api/lut-landform-elements> ;
.

<https://linked.data.gov.au/def/nrm/d7481c8e-dcec-5415-b212-df2326a60bbd>
    a urnc:CategoricalConceptMeta ;
    schema:url "https://github.com/ternaustralia/dawe-rlp-vocabs/tree/main/vocab_files/categorical_collections/luts/landform-element.ttl"^^xsd:anyURI ;
    urnp:categoricalCollection <https://linked.data.gov.au/def/nrm/c1a58967-cb12-4c2c-a7ca-9cee2589919c> ;
    urnp:categoricalConcept <https://linked.data.gov.au/def/nrm/c68c6fca-6465-5607-a2eb-32634881cddf> ;
    urnp:conceptDefinition "Flat at the margin of a stream channel aggraded and partly eroded by overbank and channelled stream flow; an incipient flood plain. Channel benches have been referred to as 'low terraces'; but the term 'terrace' should be restricted to landform patterns above the influence of active stream flow." ;
    urnp:conceptIdentifier 12 ;
    urnp:conceptNotation "CBE" ;
    urnp:conceptSource <https://core.vocabs.paratoo.tern.org.au/api/lut-landform-elements> ;
.

<https://linked.data.gov.au/def/nrm/d7b593d8-badc-562c-940b-352881cbb942>
    a urnc:CategoricalConceptMeta ;
    schema:url "https://github.com/ternaustralia/dawe-rlp-vocabs/tree/main/vocab_files/categorical_collections/luts/landform-element.ttl"^^xsd:anyURI ;
    urnp:categoricalCollection <https://linked.data.gov.au/def/nrm/c1a58967-cb12-4c2c-a7ca-9cee2589919c> ;
    urnp:categoricalConcept <https://linked.data.gov.au/def/nrm/c87e531a-ced5-579b-9c58-befdf3ee53b6> ;
    urnp:conceptDefinition "Moderately to very gently inclined waning lower slope resulting from aggradation or erosion by sheet flow; earth flow or creep." ;
    urnp:conceptIdentifier 32 ;
    urnp:conceptNotation "FOO" ;
    urnp:conceptSource <https://core.vocabs.paratoo.tern.org.au/api/lut-landform-elements> ;
.

<https://linked.data.gov.au/def/nrm/d8c0b7fa-90ad-583d-b0d3-61046094cbb6>
    a urnc:CategoricalConceptMeta ;
    schema:url "https://github.com/ternaustralia/dawe-rlp-vocabs/tree/main/vocab_files/categorical_collections/luts/landform-element.ttl"^^xsd:anyURI ;
    urnp:categoricalCollection <https://linked.data.gov.au/def/nrm/c1a58967-cb12-4c2c-a7ca-9cee2589919c> ;
    urnp:categoricalConcept <https://linked.data.gov.au/def/nrm/5c7e64fc-188c-5d94-b727-c88458bc7f95> ;
    urnp:conceptDefinition "Crest built up or eroded by the wind (see Dune)." ;
    urnp:conceptIdentifier 25 ;
    urnp:conceptNotation "DUC" ;
    urnp:conceptSource <https://core.vocabs.paratoo.tern.org.au/api/lut-landform-elements> ;
.

<https://linked.data.gov.au/def/nrm/dc1f22f5-76c7-512d-86a2-095d911d3829>
    a urnc:CategoricalConceptMeta ;
    schema:url "https://github.com/ternaustralia/dawe-rlp-vocabs/tree/main/vocab_files/categorical_collections/luts/landform-element.ttl"^^xsd:anyURI ;
    urnp:categoricalCollection <https://linked.data.gov.au/def/nrm/c1a58967-cb12-4c2c-a7ca-9cee2589919c> ;
    urnp:categoricalConcept <https://linked.data.gov.au/def/nrm/077edbc4-8980-5e85-a6eb-1f4bd3aa1bbf> ;
    urnp:conceptDefinition "Large; water-filled closed depression." ;
    urnp:conceptIdentifier 40 ;
    urnp:conceptNotation "LAK" ;
    urnp:conceptSource <https://core.vocabs.paratoo.tern.org.au/api/lut-landform-elements> ;
.

<https://linked.data.gov.au/def/nrm/df10c1e5-8fa4-5e36-8357-6fb9d2bd5c75>
    a urnc:CategoricalConceptMeta ;
    schema:url "https://github.com/ternaustralia/dawe-rlp-vocabs/tree/main/vocab_files/categorical_collections/luts/landform-element.ttl"^^xsd:anyURI ;
    urnp:categoricalCollection <https://linked.data.gov.au/def/nrm/c1a58967-cb12-4c2c-a7ca-9cee2589919c> ;
    urnp:categoricalConcept <https://linked.data.gov.au/def/nrm/bc6e0ac3-f1ef-5f6b-bcf9-7e23b620f256> ;
    urnp:conceptDefinition "Flat of bare consolidated rock; usually eroded by sheet wash." ;
    urnp:conceptIdentifier 58 ;
    urnp:conceptNotation "RFL" ;
    urnp:conceptSource <https://core.vocabs.paratoo.tern.org.au/api/lut-landform-elements> ;
.

<https://linked.data.gov.au/def/nrm/e614b305-192b-5122-8702-bd3b0583f644>
    a urnc:CategoricalConceptMeta ;
    schema:url "https://github.com/ternaustralia/dawe-rlp-vocabs/tree/main/vocab_files/categorical_collections/luts/landform-element.ttl"^^xsd:anyURI ;
    urnp:categoricalCollection <https://linked.data.gov.au/def/nrm/c1a58967-cb12-4c2c-a7ca-9cee2589919c> ;
    urnp:categoricalConcept <https://linked.data.gov.au/def/nrm/392c68e8-e681-556d-a1ae-4a7aecf5144d> ;
    urnp:conceptDefinition "Large; gently inclined to level (<1%) waning lower slope; with slope lines inclined in a single direction; or somewhat convergent or divergent; eroded or sometimes slightly aggraded by sheet flow. It is underlain by bedrock." ;
    urnp:conceptIdentifier 49 ;
    urnp:conceptNotation "PED" ;
    urnp:conceptSource <https://core.vocabs.paratoo.tern.org.au/api/lut-landform-elements> ;
.

<https://linked.data.gov.au/def/nrm/ede972cc-963e-57f3-b594-ed4a137ed9dc>
    a urnc:CategoricalConceptMeta ;
    schema:url "https://github.com/ternaustralia/dawe-rlp-vocabs/tree/main/vocab_files/categorical_collections/luts/landform-element.ttl"^^xsd:anyURI ;
    urnp:categoricalCollection <https://linked.data.gov.au/def/nrm/c1a58967-cb12-4c2c-a7ca-9cee2589919c> ;
    urnp:categoricalConcept <https://linked.data.gov.au/def/nrm/d9f167e1-bc10-56b3-8c13-5d6ee1213b10> ;
    urnp:conceptDefinition "Waning or minimal slope situated below a scarp; with its contours generally parallel to the line of the scarp." ;
    urnp:conceptIdentifier 62 ;
    urnp:conceptNotation "SFS" ;
    urnp:conceptSource <https://core.vocabs.paratoo.tern.org.au/api/lut-landform-elements> ;
.

<https://linked.data.gov.au/def/nrm/ef20c946-0016-56a6-b198-50d7fc809686>
    a urnc:CategoricalConceptMeta ;
    schema:url "https://github.com/ternaustralia/dawe-rlp-vocabs/tree/main/vocab_files/categorical_collections/luts/landform-element.ttl"^^xsd:anyURI ;
    urnp:categoricalCollection <https://linked.data.gov.au/def/nrm/c1a58967-cb12-4c2c-a7ca-9cee2589919c> ;
    urnp:categoricalConcept <https://linked.data.gov.au/def/nrm/f1c3145c-ff9d-5303-8281-e2a9866167d7> ;
    urnp:conceptDefinition "Gently inclined to precipitous slope; commonly simple and maximal; eroded by sheet wash; creep or water-aided mass movement. A typical element of mountains; hills; low hills and rises." ;
    urnp:conceptIdentifier 36 ;
    urnp:conceptNotation "HSL" ;
    urnp:conceptSource <https://core.vocabs.paratoo.tern.org.au/api/lut-landform-elements> ;
.

<https://linked.data.gov.au/def/nrm/f29ebd25-4eb7-5619-b8d1-ddd4a1c1214a>
    a urnc:CategoricalConceptMeta ;
    schema:url "https://github.com/ternaustralia/dawe-rlp-vocabs/tree/main/vocab_files/categorical_collections/luts/landform-element.ttl"^^xsd:anyURI ;
    urnp:categoricalCollection <https://linked.data.gov.au/def/nrm/c1a58967-cb12-4c2c-a7ca-9cee2589919c> ;
    urnp:categoricalConcept <https://linked.data.gov.au/def/nrm/e2ca4495-5e11-5f98-9bf1-14ff4bb4bbd5> ;
    urnp:conceptDefinition "Moderately inclined to very steep; short open depression with concave cross-section; eroded by collapse; landslides; creep or surface wash." ;
    urnp:conceptIdentifier 1 ;
    urnp:conceptNotation "ALC" ;
    urnp:conceptSource <https://core.vocabs.paratoo.tern.org.au/api/lut-landform-elements> ;
.

<https://linked.data.gov.au/def/nrm/f29fe987-89e1-597f-881d-1b89ff446c18>
    a urnc:CategoricalConceptMeta ;
    schema:url "https://github.com/ternaustralia/dawe-rlp-vocabs/tree/main/vocab_files/categorical_collections/luts/landform-element.ttl"^^xsd:anyURI ;
    urnp:categoricalCollection <https://linked.data.gov.au/def/nrm/c1a58967-cb12-4c2c-a7ca-9cee2589919c> ;
    urnp:categoricalConcept <https://linked.data.gov.au/def/nrm/5b1e7e84-5a23-5444-91c1-f97a872bc38e> ;
    urnp:conceptDefinition "Closed depression filled with water that is typically salt or brackish; bounded at least in part by forms aggraded or built up by waves or reef-building organisms." ;
    urnp:conceptIdentifier 39 ;
    urnp:conceptNotation "LAG" ;
    urnp:conceptSource <https://core.vocabs.paratoo.tern.org.au/api/lut-landform-elements> ;
.

<https://linked.data.gov.au/def/nrm/f5ee0c0a-6a38-539e-9288-b5b3a5606e27>
    a urnc:CategoricalConceptMeta ;
    schema:url "https://github.com/ternaustralia/dawe-rlp-vocabs/tree/main/vocab_files/categorical_collections/luts/landform-element.ttl"^^xsd:anyURI ;
    urnp:categoricalCollection <https://linked.data.gov.au/def/nrm/c1a58967-cb12-4c2c-a7ca-9cee2589919c> ;
    urnp:categoricalConcept <https://linked.data.gov.au/def/nrm/37480929-9e0f-5ad7-8df9-914920540692> ;
    urnp:conceptDefinition "Steep maximal mid-slope or upper slope; generally comprising both a very short scarp (free face) that is often bare rockland; and a stony scarp-footslope (debris slope); often standing above a pediment" ;
    urnp:conceptIdentifier 11 ;
    urnp:conceptNotation "BRK" ;
    urnp:conceptSource <https://core.vocabs.paratoo.tern.org.au/api/lut-landform-elements> ;
.

<https://linked.data.gov.au/def/nrm/f6f2e07c-dda2-5abd-8a22-2a2ff2e8521a>
    a urnc:CategoricalConceptMeta ;
    schema:url "https://github.com/ternaustralia/dawe-rlp-vocabs/tree/main/vocab_files/categorical_collections/luts/landform-element.ttl"^^xsd:anyURI ;
    urnp:categoricalCollection <https://linked.data.gov.au/def/nrm/c1a58967-cb12-4c2c-a7ca-9cee2589919c> ;
    urnp:categoricalConcept <https://linked.data.gov.au/def/nrm/045be349-f9ed-52d6-89ca-68c7ade53e41> ;
    urnp:conceptDefinition "Ridge or slope built up by human activity." ;
    urnp:conceptIdentifier 27 ;
    urnp:conceptNotation "EMB" ;
    urnp:conceptSource <https://core.vocabs.paratoo.tern.org.au/api/lut-landform-elements> ;
.

<https://linked.data.gov.au/def/nrm/f8726949-6dff-53cd-8b52-996a50eac071>
    a urnc:CategoricalConceptMeta ;
    schema:url "https://github.com/ternaustralia/dawe-rlp-vocabs/tree/main/vocab_files/categorical_collections/luts/landform-element.ttl"^^xsd:anyURI ;
    urnp:categoricalCollection <https://linked.data.gov.au/def/nrm/c1a58967-cb12-4c2c-a7ca-9cee2589919c> ;
    urnp:categoricalConcept <https://linked.data.gov.au/def/nrm/e874a1f0-e788-5a8c-9331-4b8329222759> ;
    urnp:conceptDefinition "Moderately inclined to very steep ridge or hillock built up by the wind. This element may comprise dunecrest and duneslope." ;
    urnp:conceptIdentifier 24 ;
    urnp:conceptNotation "DUN" ;
    urnp:conceptSource <https://core.vocabs.paratoo.tern.org.au/api/lut-landform-elements> ;
.

<https://linked.data.gov.au/def/nrm/032a1c8b-1048-5c81-bd06-8afce5c12451>
    a skos:Concept ;
    dcterms:identifier 26 ;
    dcterms:source <https://core.vocabs.paratoo.tern.org.au/api/lut-landform-elements> ;
    rdfs:isDefinedBy <https://linked.data.gov.au/def/nrm> ;
    skos:definition "Slope built up or eroded by the wind (see Dune)." ;
    skos:notation "DUS" ;
    skos:prefLabel "Dune slope" ;
    schema:url "https://github.com/ternaustralia/dawe-rlp-vocabs/tree/main/vocab_files/categorical_collections/luts/landform-element.ttl"^^xsd:anyURI ;
.

<https://linked.data.gov.au/def/nrm/045be349-f9ed-52d6-89ca-68c7ade53e41>
    a skos:Concept ;
    dcterms:identifier 27 ;
    dcterms:source <https://core.vocabs.paratoo.tern.org.au/api/lut-landform-elements> ;
    rdfs:isDefinedBy <https://linked.data.gov.au/def/nrm> ;
    skos:definition "Ridge or slope built up by human activity." ;
    skos:notation "EMB" ;
    skos:prefLabel "Embankment" ;
    schema:url "https://github.com/ternaustralia/dawe-rlp-vocabs/tree/main/vocab_files/categorical_collections/luts/landform-element.ttl"^^xsd:anyURI ;
.

<https://linked.data.gov.au/def/nrm/077edbc4-8980-5e85-a6eb-1f4bd3aa1bbf>
    a skos:Concept ;
    dcterms:identifier 40 ;
    dcterms:source <https://core.vocabs.paratoo.tern.org.au/api/lut-landform-elements> ;
    rdfs:isDefinedBy <https://linked.data.gov.au/def/nrm> ;
    skos:definition "Large; water-filled closed depression." ;
    skos:notation "LAK" ;
    skos:prefLabel "Lake" ;
    schema:url "https://github.com/ternaustralia/dawe-rlp-vocabs/tree/main/vocab_files/categorical_collections/luts/landform-element.ttl"^^xsd:anyURI ;
.

<https://linked.data.gov.au/def/nrm/0de17230-6ae6-5c2e-ab07-0bbe262a3501>
    a skos:Concept ;
    dcterms:identifier 50 ;
    dcterms:source <https://core.vocabs.paratoo.tern.org.au/api/lut-landform-elements> ;
    rdfs:isDefinedBy <https://linked.data.gov.au/def/nrm> ;
    skos:definition "Closed depression excavated by human activity." ;
    skos:notation "PIT" ;
    skos:prefLabel "Pit" ;
    schema:url "https://github.com/ternaustralia/dawe-rlp-vocabs/tree/main/vocab_files/categorical_collections/luts/landform-element.ttl"^^xsd:anyURI ;
.

<https://linked.data.gov.au/def/nrm/0eec5735-6c35-58bf-9cc7-d129f4c6b8b2>
    a skos:Concept ;
    dcterms:identifier 54 ;
    dcterms:source <https://core.vocabs.paratoo.tern.org.au/api/lut-landform-elements> ;
    rdfs:isDefinedBy <https://linked.data.gov.au/def/nrm> ;
    skos:definition "Flat built up to sea level by marine organisms." ;
    skos:notation "REF" ;
    skos:prefLabel "Reef flat" ;
    schema:url "https://github.com/ternaustralia/dawe-rlp-vocabs/tree/main/vocab_files/categorical_collections/luts/landform-element.ttl"^^xsd:anyURI ;
.

<https://linked.data.gov.au/def/nrm/115cecfd-35f7-51bf-b884-6267b453f50a>
    a skos:Concept ;
    dcterms:identifier 61 ;
    dcterms:source <https://core.vocabs.paratoo.tern.org.au/api/lut-landform-elements> ;
    rdfs:isDefinedBy <https://linked.data.gov.au/def/nrm> ;
    skos:definition "Very wide; steep to precipitous maximal slope eroded by gravlty; water-aided mass movement or sheet flow." ;
    skos:notation "SCA" ;
    skos:prefLabel "Scarp" ;
    schema:url "https://github.com/ternaustralia/dawe-rlp-vocabs/tree/main/vocab_files/categorical_collections/luts/landform-element.ttl"^^xsd:anyURI ;
.

<https://linked.data.gov.au/def/nrm/1248ad7d-fb9c-564f-93c4-0c6bf3fe9088>
    a skos:Concept ;
    dcterms:identifier 47 ;
    dcterms:source <https://core.vocabs.paratoo.tern.org.au/api/lut-landform-elements> ;
    rdfs:isDefinedBy <https://linked.data.gov.au/def/nrm> ;
    skos:definition "Long; curved; commonly water-filled closed depression eroded by channelled stream flow but closed as a result of aggradation by channelled or overbank stream flow during the formation of a meander plain landform pattern. The floor of an ox-bow may be more or less aggraded by overbank stream flow; wind; and biological (peat) accumulation." ;
    skos:notation "OXB" ;
    skos:prefLabel "Ox-bow" ;
    schema:url "https://github.com/ternaustralia/dawe-rlp-vocabs/tree/main/vocab_files/categorical_collections/luts/landform-element.ttl"^^xsd:anyURI ;
.

<https://linked.data.gov.au/def/nrm/130cad8e-0a82-515a-ad75-6b84d165db6c>
    a skos:Concept ;
    dcterms:identifier 65 ;
    dcterms:source <https://core.vocabs.paratoo.tern.org.au/api/lut-landform-elements> ;
    rdfs:isDefinedBy <https://linked.data.gov.au/def/nrm> ;
    skos:definition "Steep-sided; circular or elliptical closed depression; commonly funnel-shaped; characterised by subsurface drainage and formed by dissolution of the surface or underlying within bedrock." ;
    skos:notation "DOL" ;
    skos:prefLabel "Solution doline" ;
    schema:url "https://github.com/ternaustralia/dawe-rlp-vocabs/tree/main/vocab_files/categorical_collections/luts/landform-element.ttl"^^xsd:anyURI ;
.

<https://linked.data.gov.au/def/nrm/141a8baa-89e0-5a55-b9fd-05a3c0b8c79c>
    a skos:Concept ;
    dcterms:identifier 15 ;
    dcterms:source <https://core.vocabs.paratoo.tern.org.au/api/lut-landform-elements> ;
    rdfs:isDefinedBy <https://linked.data.gov.au/def/nrm> ;
    skos:definition "Slope situated below a cliff; with its contours generally parallel to the line of the cliff eroded by sheet wash or water-aided mass movement; and aggraded locally by collapsed material from above." ;
    skos:notation "CFS" ;
    skos:prefLabel "Cliff-footslope" ;
    schema:url "https://github.com/ternaustralia/dawe-rlp-vocabs/tree/main/vocab_files/categorical_collections/luts/landform-element.ttl"^^xsd:anyURI ;
.

<https://linked.data.gov.au/def/nrm/1431e5bb-f41a-56cc-b685-9aeed406fe63>
    a skos:Concept ;
    dcterms:identifier 18 ;
    dcterms:source <https://core.vocabs.paratoo.tern.org.au/api/lut-landform-elements> ;
    rdfs:isDefinedBy <https://linked.data.gov.au/def/nrm> ;
    skos:definition "Steep to precipitous closed depression excavated by explosions due to volcanism; human action; or impact of an extraterrestrial object." ;
    skos:notation "CRA" ;
    skos:prefLabel "Crater" ;
    schema:url "https://github.com/ternaustralia/dawe-rlp-vocabs/tree/main/vocab_files/categorical_collections/luts/landform-element.ttl"^^xsd:anyURI ;
.

<https://linked.data.gov.au/def/nrm/1470deb8-2762-5fd9-8c53-fc6cf2f18a4e>
    a skos:Concept ;
    dcterms:identifier 7 ;
    dcterms:source <https://core.vocabs.paratoo.tern.org.au/api/lut-landform-elements> ;
    rdfs:isDefinedBy <https://linked.data.gov.au/def/nrm> ;
    skos:definition "Very long; nearly straight; low ridge; built up by waves and usually modified by wind. A beach ridge is often a relict feature remote from the beach." ;
    skos:notation "BRI" ;
    skos:prefLabel "Beach ridge" ;
    schema:url "https://github.com/ternaustralia/dawe-rlp-vocabs/tree/main/vocab_files/categorical_collections/luts/landform-element.ttl"^^xsd:anyURI ;
.

<https://linked.data.gov.au/def/nrm/1958c732-bbdd-5984-acec-5f56c2b82a06>
    a skos:Concept ;
    dcterms:identifier 30 ;
    dcterms:source <https://core.vocabs.paratoo.tern.org.au/api/lut-landform-elements> ;
    rdfs:isDefinedBy <https://linked.data.gov.au/def/nrm> ;
    skos:definition "Flat aggraded by human activity." ;
    skos:notation "FIL" ;
    skos:prefLabel "Fil-top" ;
    schema:url "https://github.com/ternaustralia/dawe-rlp-vocabs/tree/main/vocab_files/categorical_collections/luts/landform-element.ttl"^^xsd:anyURI ;
.

<https://linked.data.gov.au/def/nrm/1ed7b887-8971-5d45-8ada-48e18386de45>
    a skos:Concept ;
    dcterms:identifier 33 ;
    dcterms:source <https://core.vocabs.paratoo.tern.org.au/api/lut-landform-elements> ;
    rdfs:isDefinedBy <https://linked.data.gov.au/def/nrm> ;
    skos:definition "Very long; nearly straight moderately inclined to very steep ridge built up by the wind from material from an adjacent beach." ;
    skos:notation "FOR" ;
    skos:prefLabel "Foredune" ;
    schema:url "https://github.com/ternaustralia/dawe-rlp-vocabs/tree/main/vocab_files/categorical_collections/luts/landform-element.ttl"^^xsd:anyURI ;
.

<https://linked.data.gov.au/def/nrm/1fc7edc1-8d57-568f-9a98-9ab9ddcf2816>
    a skos:Concept ;
    dcterms:identifier 43 ;
    dcterms:source <https://core.vocabs.paratoo.tern.org.au/api/lut-landform-elements> ;
    rdfs:isDefinedBy <https://linked.data.gov.au/def/nrm> ;
    skos:definition "Large; sharp-crested; elongated; longitudinal (linear) dune or chain of sand dunes; oriented parallel; rather than transverse (perpendicular); to the prevailing wind. Not to be confused with the trailing arms of parabolic dunes." ;
    skos:notation "DUF" ;
    skos:prefLabel "Linear or longitudinal (seif) dune" ;
    schema:url "https://github.com/ternaustralia/dawe-rlp-vocabs/tree/main/vocab_files/categorical_collections/luts/landform-element.ttl"^^xsd:anyURI ;
.

<https://linked.data.gov.au/def/nrm/283386fa-c297-5d2a-b453-fca857ddf51d>
    a skos:Concept ;
    dcterms:identifier 9 ;
    dcterms:source <https://core.vocabs.paratoo.tern.org.au/api/lut-landform-elements> ;
    rdfs:isDefinedBy <https://linked.data.gov.au/def/nrm> ;
    skos:definition "(i) Short; very gently inclined to level minimal mid-slope in an embankment or cut face; eroded or aggraded by human activity. (ii) Flat built up by waves above a beach." ;
    skos:notation "BER" ;
    skos:prefLabel "Berm" ;
    schema:url "https://github.com/ternaustralia/dawe-rlp-vocabs/tree/main/vocab_files/categorical_collections/luts/landform-element.ttl"^^xsd:anyURI ;
.

<https://linked.data.gov.au/def/nrm/287d64df-98f4-58c3-950e-2356a15687fd>
    a skos:Concept ;
    dcterms:identifier 5 ;
    dcterms:source <https://core.vocabs.paratoo.tern.org.au/api/lut-landform-elements> ;
    rdfs:isDefinedBy <https://linked.data.gov.au/def/nrm> ;
    skos:definition "Crescent shaped dune with tips extending leeward (downwind); making this side concave and the windward (upwind) side convex. Barchan dunes tend to be arranged in chains extending in the dominant wind direction." ;
    skos:notation "DUB" ;
    skos:prefLabel "Barchan dune" ;
    schema:url "https://github.com/ternaustralia/dawe-rlp-vocabs/tree/main/vocab_files/categorical_collections/luts/landform-element.ttl"^^xsd:anyURI ;
.

<https://linked.data.gov.au/def/nrm/2ac8be18-9aae-56e3-aa07-65929e667648>
    a skos:Concept ;
    dcterms:identifier 21 ;
    dcterms:source <https://core.vocabs.paratoo.tern.org.au/api/lut-landform-elements> ;
    rdfs:isDefinedBy <https://linked.data.gov.au/def/nrm> ;
    skos:definition "Ridge built up by human activity so as to close a depression." ;
    skos:notation "DAM" ;
    skos:prefLabel "Dam" ;
    schema:url "https://github.com/ternaustralia/dawe-rlp-vocabs/tree/main/vocab_files/categorical_collections/luts/landform-element.ttl"^^xsd:anyURI ;
.

<https://linked.data.gov.au/def/nrm/30bd2063-582d-5156-8ea0-faab8d16b102>
    a skos:Concept ;
    dcterms:identifier 35 ;
    dcterms:source <https://core.vocabs.paratoo.tern.org.au/api/lut-landform-elements> ;
    rdfs:isDefinedBy <https://linked.data.gov.au/def/nrm> ;
    skos:definition "Very gently inclined to steep crest; smoothly convex; eroded mainly by creep and sheet wash. A typical element of mountains; hills; low hills and rises." ;
    skos:notation "HCR" ;
    skos:prefLabel "Hillcrest" ;
    schema:url "https://github.com/ternaustralia/dawe-rlp-vocabs/tree/main/vocab_files/categorical_collections/luts/landform-element.ttl"^^xsd:anyURI ;
.

<https://linked.data.gov.au/def/nrm/368641eb-467f-570b-9846-e8ebccb10186>
    a skos:Concept ;
    dcterms:identifier 68 ;
    dcterms:source <https://core.vocabs.paratoo.tern.org.au/api/lut-landform-elements> ;
    rdfs:isDefinedBy <https://linked.data.gov.au/def/nrm> ;
    skos:definition "Very wide; level to gently inclined crest with abrupt margins; commonly eroded by water-aided mass movement or sheet wash." ;
    skos:notation "SUS" ;
    skos:prefLabel "Summit surface" ;
    schema:url "https://github.com/ternaustralia/dawe-rlp-vocabs/tree/main/vocab_files/categorical_collections/luts/landform-element.ttl"^^xsd:anyURI ;
.

<https://linked.data.gov.au/def/nrm/37421601-50ec-5371-b697-e9e18a54ba92>
    a skos:Concept ;
    dcterms:identifier 34 ;
    dcterms:source <https://core.vocabs.paratoo.tern.org.au/api/lut-landform-elements> ;
    rdfs:isDefinedBy <https://linked.data.gov.au/def/nrm> ;
    skos:definition "Open depression with short; precipitous walls and moderately inclined to very gently inclined floor or small stream channel; eroded by channelled stream flow and consequent collapse and water-aided mass movement." ;
    skos:notation "GUL" ;
    skos:prefLabel "Gully" ;
    schema:url "https://github.com/ternaustralia/dawe-rlp-vocabs/tree/main/vocab_files/categorical_collections/luts/landform-element.ttl"^^xsd:anyURI ;
.

<https://linked.data.gov.au/def/nrm/37480929-9e0f-5ad7-8df9-914920540692>
    a skos:Concept ;
    dcterms:identifier 11 ;
    dcterms:source <https://core.vocabs.paratoo.tern.org.au/api/lut-landform-elements> ;
    rdfs:isDefinedBy <https://linked.data.gov.au/def/nrm> ;
    skos:definition "Steep maximal mid-slope or upper slope; generally comprising both a very short scarp (free face) that is often bare rockland; and a stony scarp-footslope (debris slope); often standing above a pediment" ;
    skos:notation "BRK" ;
    skos:prefLabel "Breakaway" ;
    schema:url "https://github.com/ternaustralia/dawe-rlp-vocabs/tree/main/vocab_files/categorical_collections/luts/landform-element.ttl"^^xsd:anyURI ;
.

<https://linked.data.gov.au/def/nrm/392c68e8-e681-556d-a1ae-4a7aecf5144d>
    a skos:Concept ;
    dcterms:identifier 49 ;
    dcterms:source <https://core.vocabs.paratoo.tern.org.au/api/lut-landform-elements> ;
    rdfs:isDefinedBy <https://linked.data.gov.au/def/nrm> ;
    skos:definition "Large; gently inclined to level (<1%) waning lower slope; with slope lines inclined in a single direction; or somewhat convergent or divergent; eroded or sometimes slightly aggraded by sheet flow. It is underlain by bedrock." ;
    skos:notation "PED" ;
    skos:prefLabel "Pediment" ;
    schema:url "https://github.com/ternaustralia/dawe-rlp-vocabs/tree/main/vocab_files/categorical_collections/luts/landform-element.ttl"^^xsd:anyURI ;
.

<https://linked.data.gov.au/def/nrm/41df86fc-66ec-5ef5-a605-edbe1b3c5edc>
    a skos:Concept ;
    dcterms:identifier 14 ;
    dcterms:source <https://core.vocabs.paratoo.tern.org.au/api/lut-landform-elements> ;
    rdfs:isDefinedBy <https://linked.data.gov.au/def/nrm> ;
    skos:definition "Very wide; cliffed (greater than 72 degrees) maximal slope usually eroded by gravitational fall as a result of erosion of the base by various agencies; sometimes built up by marine organisms." ;
    skos:notation "CLI" ;
    skos:prefLabel "Cliff" ;
    schema:url "https://github.com/ternaustralia/dawe-rlp-vocabs/tree/main/vocab_files/categorical_collections/luts/landform-element.ttl"^^xsd:anyURI ;
.

<https://linked.data.gov.au/def/nrm/4524d1f6-1951-502e-b7fe-8439acd3448a>
    a skos:Concept ;
    dcterms:identifier 29 ;
    dcterms:source <https://core.vocabs.paratoo.tern.org.au/api/lut-landform-elements> ;
    rdfs:isDefinedBy <https://linked.data.gov.au/def/nrm> ;
    skos:definition "Large; gently inclined to level element with radial slope lines inclined away from a point; resulting from aggradation; or occasionally from erosion; by channelled; often braided; stream flow; or possibly by sheet flow." ;
    skos:notation "FAN" ;
    skos:prefLabel "Fan" ;
    schema:url "https://github.com/ternaustralia/dawe-rlp-vocabs/tree/main/vocab_files/categorical_collections/luts/landform-element.ttl"^^xsd:anyURI ;
.

<https://linked.data.gov.au/def/nrm/45db9fbc-4730-51bb-9329-8818736698cc>
    a skos:Concept ;
    dcterms:identifier 52 ;
    dcterms:source <https://core.vocabs.paratoo.tern.org.au/api/lut-landform-elements> ;
    rdfs:isDefinedBy <https://linked.data.gov.au/def/nrm> ;
    skos:definition "Large; shallow; level-floored closed depression; intermittently water-filled; but mainly dry due to evaporation; bounded as a rule by flats aggraded by sheet flow and channelled stream flow." ;
    skos:notation "PLY" ;
    skos:prefLabel "Playa/pan" ;
    schema:url "https://github.com/ternaustralia/dawe-rlp-vocabs/tree/main/vocab_files/categorical_collections/luts/landform-element.ttl"^^xsd:anyURI ;
.

<https://linked.data.gov.au/def/nrm/47eeb3d4-8cd0-50b5-b837-4a54a22e3f31>
    a skos:Concept ;
    dcterms:identifier 20 ;
    dcterms:source <https://core.vocabs.paratoo.tern.org.au/api/lut-landform-elements> ;
    rdfs:isDefinedBy <https://linked.data.gov.au/def/nrm> ;
    skos:definition "Flat eroded by human activity." ;
    skos:notation "COS" ;
    skos:prefLabel "Cut-over surface" ;
    schema:url "https://github.com/ternaustralia/dawe-rlp-vocabs/tree/main/vocab_files/categorical_collections/luts/landform-element.ttl"^^xsd:anyURI ;
.

<https://linked.data.gov.au/def/nrm/496d5410-d95c-5fe0-9b67-f9364550c4e4>
    a skos:Concept ;
    dcterms:identifier 74 ;
    dcterms:source <https://core.vocabs.paratoo.tern.org.au/api/lut-landform-elements> ;
    rdfs:isDefinedBy <https://linked.data.gov.au/def/nrm> ;
    skos:definition "Large or very large flat aggraded by channelled or overbank stream flow; standing above a scarp and no longer frequently inundated; part of a former flood plain." ;
    skos:notation "TEP" ;
    skos:prefLabel "Terrace plain" ;
    schema:url "https://github.com/ternaustralia/dawe-rlp-vocabs/tree/main/vocab_files/categorical_collections/luts/landform-element.ttl"^^xsd:anyURI ;
.

<https://linked.data.gov.au/def/nrm/4b14473a-033a-58f1-b02c-16f47da90265>
    a skos:Concept ;
    dcterms:identifier 71 ;
    dcterms:source <https://core.vocabs.paratoo.tern.org.au/api/lut-landform-elements> ;
    rdfs:isDefinedBy <https://linked.data.gov.au/def/nrm> ;
    skos:definition "Almost level; closed or almost closed depression with a seasonal or permanent watertable at or above the surface; commonly aggraded by overbank stream flow and sometimes biological (peat) accumulation." ;
    skos:notation "SWP" ;
    skos:prefLabel "Swamp" ;
    schema:url "https://github.com/ternaustralia/dawe-rlp-vocabs/tree/main/vocab_files/categorical_collections/luts/landform-element.ttl"^^xsd:anyURI ;
.

<https://linked.data.gov.au/def/nrm/4ee55457-4922-5d00-b13d-ca381ad44f63>
    a skos:Concept ;
    dcterms:identifier 55 ;
    dcterms:source <https://core.vocabs.paratoo.tern.org.au/api/lut-landform-elements> ;
    rdfs:isDefinedBy <https://linked.data.gov.au/def/nrm> ;
    skos:definition "Hillock of very low to extremely low relief (<30 m) and very gentle to steep slopes. This term is used to refer to an isolated rise surrounded by other landforms." ;
    skos:notation "RER" ;
    skos:prefLabel "Residual rise" ;
    schema:url "https://github.com/ternaustralia/dawe-rlp-vocabs/tree/main/vocab_files/categorical_collections/luts/landform-element.ttl"^^xsd:anyURI ;
.

<https://linked.data.gov.au/def/nrm/548c40d1-6c33-511d-be44-0c9f4f1360da>
    a skos:Concept ;
    dcterms:identifier 79 ;
    dcterms:source <https://core.vocabs.paratoo.tern.org.au/api/lut-landform-elements> ;
    rdfs:isDefinedBy <https://linked.data.gov.au/def/nrm> ;
    skos:definition "Hillock heaved up by volcanism (or; elsewhere; built up by human activity at a burial site)." ;
    skos:notation "TUM" ;
    skos:prefLabel "Tumulus" ;
    schema:url "https://github.com/ternaustralia/dawe-rlp-vocabs/tree/main/vocab_files/categorical_collections/luts/landform-element.ttl"^^xsd:anyURI ;
.

<https://linked.data.gov.au/def/nrm/54c94292-798f-5a26-8455-d1a302756f4f>
    a skos:Concept ;
    dcterms:identifier 60 ;
    dcterms:source <https://core.vocabs.paratoo.tern.org.au/api/lut-landform-elements> ;
    rdfs:isDefinedBy <https://linked.data.gov.au/def/nrm> ;
    skos:definition "Flat; bare of vegetatiorn; from which soil has been eroded or excavated by surface wash or wind." ;
    skos:notation "SCD" ;
    skos:prefLabel "Scald" ;
    schema:url "https://github.com/ternaustralia/dawe-rlp-vocabs/tree/main/vocab_files/categorical_collections/luts/landform-element.ttl"^^xsd:anyURI ;
.

<https://linked.data.gov.au/def/nrm/55911768-52b3-5fff-b4cf-2dd0614583c0>
    a skos:Concept ;
    dcterms:identifier 46 ;
    dcterms:source <https://core.vocabs.paratoo.tern.org.au/api/lut-landform-elements> ;
    rdfs:isDefinedBy <https://linked.data.gov.au/def/nrm> ;
    skos:definition "Hillock built up by human activity." ;
    skos:notation "MOU" ;
    skos:prefLabel "Mound" ;
    schema:url "https://github.com/ternaustralia/dawe-rlp-vocabs/tree/main/vocab_files/categorical_collections/luts/landform-element.ttl"^^xsd:anyURI ;
.

<https://linked.data.gov.au/def/nrm/5b1e7e84-5a23-5444-91c1-f97a872bc38e>
    a skos:Concept ;
    dcterms:identifier 39 ;
    dcterms:source <https://core.vocabs.paratoo.tern.org.au/api/lut-landform-elements> ;
    rdfs:isDefinedBy <https://linked.data.gov.au/def/nrm> ;
    skos:definition "Closed depression filled with water that is typically salt or brackish; bounded at least in part by forms aggraded or built up by waves or reef-building organisms." ;
    skos:notation "LAG" ;
    skos:prefLabel "Lagoon" ;
    schema:url "https://github.com/ternaustralia/dawe-rlp-vocabs/tree/main/vocab_files/categorical_collections/luts/landform-element.ttl"^^xsd:anyURI ;
.

<https://linked.data.gov.au/def/nrm/5c7e64fc-188c-5d94-b727-c88458bc7f95>
    a skos:Concept ;
    dcterms:identifier 25 ;
    dcterms:source <https://core.vocabs.paratoo.tern.org.au/api/lut-landform-elements> ;
    rdfs:isDefinedBy <https://linked.data.gov.au/def/nrm> ;
    skos:definition "Crest built up or eroded by the wind (see Dune)." ;
    skos:notation "DUC" ;
    skos:prefLabel "Dune crest" ;
    schema:url "https://github.com/ternaustralia/dawe-rlp-vocabs/tree/main/vocab_files/categorical_collections/luts/landform-element.ttl"^^xsd:anyURI ;
.

<https://linked.data.gov.au/def/nrm/5cd65691-a295-577c-9f94-cd4756337e3f>
    a skos:Concept ;
    dcterms:identifier 44 ;
    dcterms:source <https://core.vocabs.paratoo.tern.org.au/api/lut-landform-elements> ;
    rdfs:isDefinedBy <https://linked.data.gov.au/def/nrm> ;
    skos:definition "Elongated; gently curved; low ridge built up by wind on the margin of a playa; typically with a moderate; wave-modified slope towards the playa and a gentle outer slope." ;
    skos:notation "LUN" ;
    skos:prefLabel "Lunette" ;
    schema:url "https://github.com/ternaustralia/dawe-rlp-vocabs/tree/main/vocab_files/categorical_collections/luts/landform-element.ttl"^^xsd:anyURI ;
.

<https://linked.data.gov.au/def/nrm/5de0ce45-d559-57b0-8328-83e133672104>
    a skos:Concept ;
    dcterms:identifier 23 ;
    dcterms:source <https://core.vocabs.paratoo.tern.org.au/api/lut-landform-elements> ;
    rdfs:isDefinedBy <https://linked.data.gov.au/def/nrm> ;
    skos:definition "Level to gently inclined; long; narrow shallow open depression with smoothly concave cross-section rising to moderately inclined side slopes; eroded or aggraded by sheet wash." ;
    skos:notation "DDE" ;
    skos:prefLabel "Drainage depression" ;
    schema:url "https://github.com/ternaustralia/dawe-rlp-vocabs/tree/main/vocab_files/categorical_collections/luts/landform-element.ttl"^^xsd:anyURI ;
.

<https://linked.data.gov.au/def/nrm/63960cfe-9e04-52b7-8940-4d6c2ebe0a02>
    a skos:Concept ;
    dcterms:identifier 6 ;
    dcterms:source <https://core.vocabs.paratoo.tern.org.au/api/lut-landform-elements> ;
    rdfs:isDefinedBy <https://linked.data.gov.au/def/nrm> ;
    skos:definition "Short; low; very wide slope; gently or moderately inclined; built up or eroded by waves; forming the shore of a lake or sea." ;
    skos:notation "BEA" ;
    skos:prefLabel "Beach" ;
    schema:url "https://github.com/ternaustralia/dawe-rlp-vocabs/tree/main/vocab_files/categorical_collections/luts/landform-element.ttl"^^xsd:anyURI ;
.

<https://linked.data.gov.au/def/nrm/64008844-d6ff-5fa3-9218-48a3d57ada21>
    a skos:Concept ;
    dcterms:identifier 73 ;
    dcterms:source <https://core.vocabs.paratoo.tern.org.au/api/lut-landform-elements> ;
    rdfs:isDefinedBy <https://linked.data.gov.au/def/nrm> ;
    skos:definition "Small flat aggraded or eroded by channelled or overbank stream flow; standing above a scarp and no longer frequently inundated; a former valley flat or part of a former flood plain." ;
    skos:notation "TEF" ;
    skos:prefLabel "Terrace Flat" ;
    schema:url "https://github.com/ternaustralia/dawe-rlp-vocabs/tree/main/vocab_files/categorical_collections/luts/landform-element.ttl"^^xsd:anyURI ;
.

<https://linked.data.gov.au/def/nrm/69a64f8c-65b5-5185-8e16-39ce4f28a839>
    a skos:Concept ;
    dcterms:identifier 64 ;
    dcterms:source <https://core.vocabs.paratoo.tern.org.au/api/lut-landform-elements> ;
    rdfs:isDefinedBy <https://linked.data.gov.au/def/nrm> ;
    skos:definition "Large flat resulting from aggradation by channelled stream flow as a stream migrates from side to side; the dominant element of a meander plain landform pattern. This landform element may include occurrences of scroll; swale and ox-bow." ;
    skos:notation "SRP" ;
    skos:prefLabel "Scroll plain" ;
    schema:url "https://github.com/ternaustralia/dawe-rlp-vocabs/tree/main/vocab_files/categorical_collections/luts/landform-element.ttl"^^xsd:anyURI ;
.

<https://linked.data.gov.au/def/nrm/6ff1c19e-cd58-5c14-b39d-6c093ba8b994>
    a skos:Concept ;
    dcterms:identifier 31 ;
    dcterms:source <https://core.vocabs.paratoo.tern.org.au/api/lut-landform-elements> ;
    rdfs:isDefinedBy <https://linked.data.gov.au/def/nrm> ;
    skos:definition "Flat inclined radially away from a point on the margin or at the end of a stream channel; aggraded by overbank stream flow; or by channelled stream flow associated with channels developed within the overbank flow; part of a covered plain landform pattern." ;
    skos:notation "FLD" ;
    skos:prefLabel "Floodout" ;
    schema:url "https://github.com/ternaustralia/dawe-rlp-vocabs/tree/main/vocab_files/categorical_collections/luts/landform-element.ttl"^^xsd:anyURI ;
.

<https://linked.data.gov.au/def/nrm/71bc069c-03d3-53a5-a8d7-ef6a8f039389>
    a skos:Concept ;
    dcterms:identifier 66 ;
    dcterms:source <https://core.vocabs.paratoo.tern.org.au/api/lut-landform-elements> ;
    rdfs:isDefinedBy <https://linked.data.gov.au/def/nrm> ;
    skos:definition "Linear; generally sinuous open depression forming the bottom of a stream channel; eroded and locally excavated; aggraded or built up by channelled stream flow. Parts that are built up include bars." ;
    skos:notation "STB" ;
    skos:prefLabel "Stream bed" ;
    schema:url "https://github.com/ternaustralia/dawe-rlp-vocabs/tree/main/vocab_files/categorical_collections/luts/landform-element.ttl"^^xsd:anyURI ;
.

<https://linked.data.gov.au/def/nrm/7cb2f197-c3e8-5491-b0db-78b839405fd7>
    a skos:Concept ;
    dcterms:identifier 28 ;
    dcterms:source <https://core.vocabs.paratoo.tern.org.au/api/lut-landform-elements> ;
    rdfs:isDefinedBy <https://linked.data.gov.au/def/nrm> ;
    skos:definition "Stream channel close to its junction with a sea or lake; where the action of channelled stream flow is modified by tide and waves. The width typically increases downstream." ;
    skos:notation "EST" ;
    skos:prefLabel "Estuary" ;
    schema:url "https://github.com/ternaustralia/dawe-rlp-vocabs/tree/main/vocab_files/categorical_collections/luts/landform-element.ttl"^^xsd:anyURI ;
.

<https://linked.data.gov.au/def/nrm/85b66cd6-ced2-5176-8338-6cf889145d08>
    a skos:Concept ;
    dcterms:identifier 17 ;
    dcterms:source <https://core.vocabs.paratoo.tern.org.au/api/lut-landform-elements> ;
    rdfs:isDefinedBy <https://linked.data.gov.au/def/nrm> ;
    skos:definition "Hillock with a circular symmetry built up by volcanism. The crest may form a ring around a crater." ;
    skos:notation "CON" ;
    skos:prefLabel "Cone (volcanic)" ;
    schema:url "https://github.com/ternaustralia/dawe-rlp-vocabs/tree/main/vocab_files/categorical_collections/luts/landform-element.ttl"^^xsd:anyURI ;
.

<https://linked.data.gov.au/def/nrm/8e448737-8d60-56a6-94df-9399d5b9e174>
    a skos:Concept ;
    dcterms:identifier 22 ;
    dcterms:source <https://core.vocabs.paratoo.tern.org.au/api/lut-landform-elements> ;
    rdfs:isDefinedBy <https://linked.data.gov.au/def/nrm> ;
    skos:definition "Basin excavated by wind erosion which removes loose material; commonly above a resistant or wet layer." ;
    skos:notation "DBA" ;
    skos:prefLabel "Deflation basin" ;
    schema:url "https://github.com/ternaustralia/dawe-rlp-vocabs/tree/main/vocab_files/categorical_collections/luts/landform-element.ttl"^^xsd:anyURI ;
.

<https://linked.data.gov.au/def/nrm/93fed9db-1788-54b3-8731-89430eb8f79a>
    a skos:Concept ;
    dcterms:identifier 72 ;
    dcterms:source <https://core.vocabs.paratoo.tern.org.au/api/lut-landform-elements> ;
    rdfs:isDefinedBy <https://linked.data.gov.au/def/nrm> ;
    skos:definition "Moderately inclined or steep waning lower slope; consisting of rock fragments aggraded by gravlty." ;
    skos:notation "TAL" ;
    skos:prefLabel "Talus" ;
    schema:url "https://github.com/ternaustralia/dawe-rlp-vocabs/tree/main/vocab_files/categorical_collections/luts/landform-element.ttl"^^xsd:anyURI ;
.

<https://linked.data.gov.au/def/nrm/95d1041f-0a82-50d5-9702-f58a95029f95>
    a skos:Concept ;
    dcterms:identifier 2 ;
    dcterms:source <https://core.vocabs.paratoo.tern.org.au/api/lut-landform-elements> ;
    rdfs:isDefinedBy <https://linked.data.gov.au/def/nrm> ;
    skos:definition "Large flat resulting from aggradation by overbank stream flow at some distance from the stream channel and in some cases biological (peat) accumulation; often characterised by a high watertable and the presence of swamps or lakes; part of a covered plain landform pattern." ;
    skos:notation "BKP" ;
    skos:prefLabel "Backplain" ;
    schema:url "https://github.com/ternaustralia/dawe-rlp-vocabs/tree/main/vocab_files/categorical_collections/luts/landform-element.ttl"^^xsd:anyURI ;
.

<https://linked.data.gov.au/def/nrm/987ae37a-02be-5ef7-a4a6-1b13406fa277>
    a skos:Concept ;
    dcterms:identifier 67 ;
    dcterms:source <https://core.vocabs.paratoo.tern.org.au/api/lut-landform-elements> ;
    rdfs:isDefinedBy <https://linked.data.gov.au/def/nrm> ;
    skos:definition "Linear; generally sinuous open depression; in parts eroded; excavated; built up and aggraded by channelled stream flow. This element comprises stream bed and banks." ;
    skos:notation "STC" ;
    skos:prefLabel "Stream channel" ;
    schema:url "https://github.com/ternaustralia/dawe-rlp-vocabs/tree/main/vocab_files/categorical_collections/luts/landform-element.ttl"^^xsd:anyURI ;
.

<https://linked.data.gov.au/def/nrm/9969b531-7f6c-54a6-a23c-123c332d3428>
    a skos:Concept ;
    dcterms:identifier 56 ;
    dcterms:source <https://core.vocabs.paratoo.tern.org.au/api/lut-landform-elements> ;
    rdfs:isDefinedBy <https://linked.data.gov.au/def/nrm> ;
    skos:definition "Crest of hillock of very low to extremely low relief (<30 m) (see Residual rise)." ;
    skos:notation "REC" ;
    skos:prefLabel "Risecrest" ;
    schema:url "https://github.com/ternaustralia/dawe-rlp-vocabs/tree/main/vocab_files/categorical_collections/luts/landform-element.ttl"^^xsd:anyURI ;
.

<https://linked.data.gov.au/def/nrm/9da5cf89-4487-5f93-b351-0782a42ae362>
    a skos:Concept ;
    dcterms:identifier 8 ;
    dcterms:source <https://core.vocabs.paratoo.tern.org.au/api/lut-landform-elements> ;
    rdfs:isDefinedBy <https://linked.data.gov.au/def/nrm> ;
    skos:definition "Short; gently or very gently inclined minimal mid-slope element eroded or aggraded by any agent." ;
    skos:notation "BEN" ;
    skos:prefLabel "Bench" ;
    schema:url "https://github.com/ternaustralia/dawe-rlp-vocabs/tree/main/vocab_files/categorical_collections/luts/landform-element.ttl"^^xsd:anyURI ;
.

<https://linked.data.gov.au/def/nrm/9fcf1019-135e-5fad-9fab-ea6da190eb05>
    a skos:Concept ;
    dcterms:identifier 59 ;
    dcterms:source <https://core.vocabs.paratoo.tern.org.au/api/lut-landform-elements> ;
    rdfs:isDefinedBy <https://linked.data.gov.au/def/nrm> ;
    skos:definition "Flat of consolidated rock eroded by waves." ;
    skos:notation "RPL" ;
    skos:prefLabel "Rock platform" ;
    schema:url "https://github.com/ternaustralia/dawe-rlp-vocabs/tree/main/vocab_files/categorical_collections/luts/landform-element.ttl"^^xsd:anyURI ;
.

<https://linked.data.gov.au/def/nrm/a19a72a0-2433-5fd2-8f64-16503637b9ee>
    a skos:Concept ;
    dcterms:identifier 37 ;
    dcterms:source <https://core.vocabs.paratoo.tern.org.au/api/lut-landform-elements> ;
    rdfs:isDefinedBy <https://linked.data.gov.au/def/nrm> ;
    skos:definition "Very gently to moderately inclined rises or hillocks built up or eroded by wind and lacking distinct orientation or regular pattern." ;
    skos:notation "DUH" ;
    skos:prefLabel "Hummocky (weakly oriented dune)" ;
    schema:url "https://github.com/ternaustralia/dawe-rlp-vocabs/tree/main/vocab_files/categorical_collections/luts/landform-element.ttl"^^xsd:anyURI ;
.

<https://linked.data.gov.au/def/nrm/a749658e-2521-5fe0-8aaf-e352c3639fc1>
    a skos:Concept ;
    dcterms:identifier 42 ;
    dcterms:source <https://core.vocabs.paratoo.tern.org.au/api/lut-landform-elements> ;
    rdfs:isDefinedBy <https://linked.data.gov.au/def/nrm> ;
    skos:definition "Very long; low; narrow; nearly level; sinuous ridge immediately adjacent to a stream channel; built up by overbank flow. Levees are built usually in pairs bounding the two sides of a stream channel; at the level reached by frequent floods. This element is part of a covered plain landform pattern. For an artificial levee; use Embankment. See also Prior stream." ;
    skos:notation "LEV" ;
    skos:prefLabel "Levee" ;
    schema:url "https://github.com/ternaustralia/dawe-rlp-vocabs/tree/main/vocab_files/categorical_collections/luts/landform-element.ttl"^^xsd:anyURI ;
.

<https://linked.data.gov.au/def/nrm/a75e7c17-b8c5-50b2-a0ca-74cfc6a65229>
    a skos:Concept ;
    dcterms:identifier 19 ;
    dcterms:source <https://core.vocabs.paratoo.tern.org.au/api/lut-landform-elements> ;
    rdfs:isDefinedBy <https://linked.data.gov.au/def/nrm> ;
    skos:definition "Slope eroded by human activity." ;
    skos:notation "CUT" ;
    skos:prefLabel "Cut face" ;
    schema:url "https://github.com/ternaustralia/dawe-rlp-vocabs/tree/main/vocab_files/categorical_collections/luts/landform-element.ttl"^^xsd:anyURI ;
.

<https://linked.data.gov.au/def/nrm/b2025ffe-3999-5c93-a6ef-295bfed37242>
    a skos:Concept ;
    dcterms:identifier 48 ;
    dcterms:source <https://core.vocabs.paratoo.tern.org.au/api/lut-landform-elements> ;
    rdfs:isDefinedBy <https://linked.data.gov.au/def/nrm> ;
    skos:definition "Sand dune with a long; scoop-shaped form; convex in the downwind direction so that its horns point upwind; whose ground plan approximates the form of a parabola. The dunes left behind can be referred to as trailing arms. Where many such dunes have traversed an area; these can give the appearance of linear dunes." ;
    skos:notation "DUP" ;
    skos:prefLabel "Parabolic dune" ;
    schema:url "https://github.com/ternaustralia/dawe-rlp-vocabs/tree/main/vocab_files/categorical_collections/luts/landform-element.ttl"^^xsd:anyURI ;
.

<https://linked.data.gov.au/def/nrm/b357ae54-1094-5957-bf45-500ceab54a37>
    a skos:Concept ;
    dcterms:identifier 45 ;
    dcterms:source <https://core.vocabs.paratoo.tern.org.au/api/lut-landform-elements> ;
    rdfs:isDefinedBy <https://linked.data.gov.au/def/nrm> ;
    skos:definition "Level-floored; commonly water-filled closed depression with a nearly circular; steep rim; excavated by volcanism." ;
    skos:notation "MAA" ;
    skos:prefLabel "Maar" ;
    schema:url "https://github.com/ternaustralia/dawe-rlp-vocabs/tree/main/vocab_files/categorical_collections/luts/landform-element.ttl"^^xsd:anyURI ;
.

<https://linked.data.gov.au/def/nrm/b4c53a4f-3e36-507e-8f29-6468c146cd3c>
    a skos:Concept ;
    dcterms:identifier 16 ;
    dcterms:source <https://core.vocabs.paratoo.tern.org.au/api/lut-landform-elements> ;
    rdfs:isDefinedBy <https://linked.data.gov.au/def/nrm> ;
    skos:definition "Steep-sided; circular or elliptical closed depression; commonly funnel-shaped; characterised by subsurface drainage and formed by collapse of underlying caves within bedrock." ;
    skos:notation "DOC" ;
    skos:prefLabel "Collapse doline" ;
    schema:url "https://github.com/ternaustralia/dawe-rlp-vocabs/tree/main/vocab_files/categorical_collections/luts/landform-element.ttl"^^xsd:anyURI ;
.

<https://linked.data.gov.au/def/nrm/b82cfeb6-1194-513a-ba81-5010cb9eb38b>
    a skos:Concept ;
    dcterms:identifier 75 ;
    dcterms:source <https://core.vocabs.paratoo.tern.org.au/api/lut-landform-elements> ;
    rdfs:isDefinedBy <https://linked.data.gov.au/def/nrm> ;
    skos:definition "Intermittently water-filled open depression in parts eroded; excavated; built up and aggraded by channelled tide-water flow; type of stream channel characterised by a rapid increase in width downstream." ;
    skos:notation "TDC" ;
    skos:prefLabel "Tidal creek" ;
    schema:url "https://github.com/ternaustralia/dawe-rlp-vocabs/tree/main/vocab_files/categorical_collections/luts/landform-element.ttl"^^xsd:anyURI ;
.

<https://linked.data.gov.au/def/nrm/bc6e0ac3-f1ef-5f6b-bcf9-7e23b620f256>
    a skos:Concept ;
    dcterms:identifier 58 ;
    dcterms:source <https://core.vocabs.paratoo.tern.org.au/api/lut-landform-elements> ;
    rdfs:isDefinedBy <https://linked.data.gov.au/def/nrm> ;
    skos:definition "Flat of bare consolidated rock; usually eroded by sheet wash." ;
    skos:notation "RFL" ;
    skos:prefLabel "Rock flat" ;
    schema:url "https://github.com/ternaustralia/dawe-rlp-vocabs/tree/main/vocab_files/categorical_collections/luts/landform-element.ttl"^^xsd:anyURI ;
.

<https://linked.data.gov.au/def/nrm/bceaebcb-9ab0-54b0-8ea2-b66c3efe9490>
    a skos:Concept ;
    dcterms:identifier 57 ;
    dcterms:source <https://core.vocabs.paratoo.tern.org.au/api/lut-landform-elements> ;
    rdfs:isDefinedBy <https://linked.data.gov.au/def/nrm> ;
    skos:definition "Slope of hillock of very low to extremely low relief (<30 m) (see Residual rise)." ;
    skos:notation "RES" ;
    skos:prefLabel "Riseslope" ;
    schema:url "https://github.com/ternaustralia/dawe-rlp-vocabs/tree/main/vocab_files/categorical_collections/luts/landform-element.ttl"^^xsd:anyURI ;
.

<https://linked.data.gov.au/def/nrm/c1c77cbf-4251-5437-b8c8-c3e44304f023>
    a skos:Concept ;
    dcterms:identifier 77 ;
    dcterms:source <https://core.vocabs.paratoo.tern.org.au/api/lut-landform-elements> ;
    rdfs:isDefinedBy <https://linked.data.gov.au/def/nrm> ;
    skos:definition "Steep to precipitous hillock; typically convex; with a surface mainly of bare rock; either coherent or comprising subangular to rounded; large boulders (exhumed core-stones; also themselves called tors) separated by open fissures; eroded by sheet wash or water-aided mass movement." ;
    skos:notation "TOR" ;
    skos:prefLabel "Tor" ;
    schema:url "https://github.com/ternaustralia/dawe-rlp-vocabs/tree/main/vocab_files/categorical_collections/luts/landform-element.ttl"^^xsd:anyURI ;
.

<https://linked.data.gov.au/def/nrm/c21bb284-7262-5dee-bd5b-8ecfe47961a0>
    a skos:Concept ;
    dcterms:identifier 38 ;
    dcterms:source <https://core.vocabs.paratoo.tern.org.au/api/lut-landform-elements> ;
    rdfs:isDefinedBy <https://linked.data.gov.au/def/nrm> ;
    skos:definition "See Tidal flat." ;
    skos:notation "ITF" ;
    skos:prefLabel "Intertidal flat" ;
    schema:url "https://github.com/ternaustralia/dawe-rlp-vocabs/tree/main/vocab_files/categorical_collections/luts/landform-element.ttl"^^xsd:anyURI ;
.

<https://linked.data.gov.au/def/nrm/c5274b62-aa6d-5168-a941-37842c6d4791>
    a skos:Concept ;
    dcterms:identifier 13 ;
    dcterms:source <https://core.vocabs.paratoo.tern.org.au/api/lut-landform-elements> ;
    rdfs:isDefinedBy <https://linked.data.gov.au/def/nrm> ;
    skos:definition "Precipitous to gently inclined; typically closed depression of concave contour and profile excavated by ice. The closed part of the depression may be shallow; the larger part being an open depression like an alcove." ;
    skos:notation "CIR" ;
    skos:prefLabel "Cirque" ;
    schema:url "https://github.com/ternaustralia/dawe-rlp-vocabs/tree/main/vocab_files/categorical_collections/luts/landform-element.ttl"^^xsd:anyURI ;
.

<https://linked.data.gov.au/def/nrm/c68c6fca-6465-5607-a2eb-32634881cddf>
    a skos:Concept ;
    dcterms:identifier 12 ;
    dcterms:source <https://core.vocabs.paratoo.tern.org.au/api/lut-landform-elements> ;
    rdfs:isDefinedBy <https://linked.data.gov.au/def/nrm> ;
    skos:definition "Flat at the margin of a stream channel aggraded and partly eroded by overbank and channelled stream flow; an incipient flood plain. Channel benches have been referred to as 'low terraces'; but the term 'terrace' should be restricted to landform patterns above the influence of active stream flow." ;
    skos:notation "CBE" ;
    skos:prefLabel "Channel bench" ;
    schema:url "https://github.com/ternaustralia/dawe-rlp-vocabs/tree/main/vocab_files/categorical_collections/luts/landform-element.ttl"^^xsd:anyURI ;
.

<https://linked.data.gov.au/def/nrm/c87e531a-ced5-579b-9c58-befdf3ee53b6>
    a skos:Concept ;
    dcterms:identifier 32 ;
    dcterms:source <https://core.vocabs.paratoo.tern.org.au/api/lut-landform-elements> ;
    rdfs:isDefinedBy <https://linked.data.gov.au/def/nrm> ;
    skos:definition "Moderately to very gently inclined waning lower slope resulting from aggradation or erosion by sheet flow; earth flow or creep." ;
    skos:notation "FOO" ;
    skos:prefLabel "Footslope" ;
    schema:url "https://github.com/ternaustralia/dawe-rlp-vocabs/tree/main/vocab_files/categorical_collections/luts/landform-element.ttl"^^xsd:anyURI ;
.

<https://linked.data.gov.au/def/nrm/cb894c58-d482-5471-a16d-eabb27d6cc5f>
    a skos:Concept ;
    dcterms:identifier 76 ;
    dcterms:source <https://core.vocabs.paratoo.tern.org.au/api/lut-landform-elements> ;
    rdfs:isDefinedBy <https://linked.data.gov.au/def/nrm> ;
    skos:definition "Large flat subject to inundation by water that is usually salt or brackish; aggradedby tides. An intertidal flat (ITF) is frequently inundated; a supratidal flat (STF) is seldom inundated." ;
    skos:notation "TDF" ;
    skos:prefLabel "Tidal flat" ;
    schema:url "https://github.com/ternaustralia/dawe-rlp-vocabs/tree/main/vocab_files/categorical_collections/luts/landform-element.ttl"^^xsd:anyURI ;
.

<https://linked.data.gov.au/def/nrm/d110a3b2-a34f-5d94-828d-e539c22ae2b5>
    a skos:Concept ;
    dcterms:identifier 3 ;
    dcterms:source <https://core.vocabs.paratoo.tern.org.au/api/lut-landform-elements> ;
    rdfs:isDefinedBy <https://linked.data.gov.au/def/nrm> ;
    skos:definition "Very short; very wide slope; moderately inclined to precipitous; forming the marginal upper parts of a stream channel and resulting from erosion or aggradation by channelled stream flow." ;
    skos:notation "BAN" ;
    skos:prefLabel "Bank (stream bank)" ;
    schema:url "https://github.com/ternaustralia/dawe-rlp-vocabs/tree/main/vocab_files/categorical_collections/luts/landform-element.ttl"^^xsd:anyURI ;
.

<https://linked.data.gov.au/def/nrm/d7154911-ea70-5613-9b4d-8fb80b36cda0>
    a skos:Concept ;
    dcterms:identifier 51 ;
    dcterms:source <https://core.vocabs.paratoo.tern.org.au/api/lut-landform-elements> ;
    rdfs:isDefinedBy <https://linked.data.gov.au/def/nrm> ;
    skos:definition "Large; very gently inclined or level element; of unspecified geomorphological agent or mode of activity." ;
    skos:notation "PLA" ;
    skos:prefLabel "Plain" ;
    schema:url "https://github.com/ternaustralia/dawe-rlp-vocabs/tree/main/vocab_files/categorical_collections/luts/landform-element.ttl"^^xsd:anyURI ;
.

<https://linked.data.gov.au/def/nrm/d85de894-c9f3-545d-a131-906301d4ff91>
    a skos:Concept ;
    dcterms:identifier 63 ;
    dcterms:source <https://core.vocabs.paratoo.tern.org.au/api/lut-landform-elements> ;
    rdfs:isDefinedBy <https://linked.data.gov.au/def/nrm> ;
    skos:definition "Long; curved; very low ridge built up by channelled stream flow and left relict by channel migration. Part of a meander plain landform pattern." ;
    skos:notation "SCR" ;
    skos:prefLabel "Scroll" ;
    schema:url "https://github.com/ternaustralia/dawe-rlp-vocabs/tree/main/vocab_files/categorical_collections/luts/landform-element.ttl"^^xsd:anyURI ;
.

<https://linked.data.gov.au/def/nrm/d901256e-66ab-5e26-a806-17a6ab335ae7>
    a skos:Concept ;
    dcterms:identifier 70 ;
    dcterms:source <https://core.vocabs.paratoo.tern.org.au/api/lut-landform-elements> ;
    rdfs:isDefinedBy <https://linked.data.gov.au/def/nrm> ;
    skos:definition "(i) Linear; level-floored open depression excavated by wind; or left relict between ridges built up by wind or waves; or built up to a lesser height than them. (ii) Long; curved open or closed depression left relict between scrolls built up by channelled stream flow." ;
    skos:notation "SWL" ;
    skos:prefLabel "Swale" ;
    schema:url "https://github.com/ternaustralia/dawe-rlp-vocabs/tree/main/vocab_files/categorical_collections/luts/landform-element.ttl"^^xsd:anyURI ;
.

<https://linked.data.gov.au/def/nrm/d9f167e1-bc10-56b3-8c13-5d6ee1213b10>
    a skos:Concept ;
    dcterms:identifier 62 ;
    dcterms:source <https://core.vocabs.paratoo.tern.org.au/api/lut-landform-elements> ;
    rdfs:isDefinedBy <https://linked.data.gov.au/def/nrm> ;
    skos:definition "Waning or minimal slope situated below a scarp; with its contours generally parallel to the line of the scarp." ;
    skos:notation "SFS" ;
    skos:prefLabel "Scarp-footslope" ;
    schema:url "https://github.com/ternaustralia/dawe-rlp-vocabs/tree/main/vocab_files/categorical_collections/luts/landform-element.ttl"^^xsd:anyURI ;
.

<https://linked.data.gov.au/def/nrm/dd2d43e4-2a30-509f-817a-407b271e8204>
    a skos:Concept ;
    dcterms:identifier 69 ;
    dcterms:source <https://core.vocabs.paratoo.tern.org.au/api/lut-landform-elements> ;
    rdfs:isDefinedBy <https://linked.data.gov.au/def/nrm> ;
    skos:definition "See Tidal flat." ;
    skos:notation "STF" ;
    skos:prefLabel "Supratidal flat" ;
    schema:url "https://github.com/ternaustralia/dawe-rlp-vocabs/tree/main/vocab_files/categorical_collections/luts/landform-element.ttl"^^xsd:anyURI ;
.

<https://linked.data.gov.au/def/nrm/e13edfb1-b27f-5f73-ac06-bb40b2520684>
    a skos:Concept ;
    dcterms:identifier 10 ;
    dcterms:source <https://core.vocabs.paratoo.tern.org.au/api/lut-landform-elements> ;
    rdfs:isDefinedBy <https://linked.data.gov.au/def/nrm> ;
    skos:definition "Usually small; open or closed depression excavated by the wind." ;
    skos:notation "BOU" ;
    skos:prefLabel "Blow-out" ;
    schema:url "https://github.com/ternaustralia/dawe-rlp-vocabs/tree/main/vocab_files/categorical_collections/luts/landform-element.ttl"^^xsd:anyURI ;
.

<https://linked.data.gov.au/def/nrm/e2ca4495-5e11-5f98-9bf1-14ff4bb4bbd5>
    a skos:Concept ;
    dcterms:identifier 1 ;
    dcterms:source <https://core.vocabs.paratoo.tern.org.au/api/lut-landform-elements> ;
    rdfs:isDefinedBy <https://linked.data.gov.au/def/nrm> ;
    skos:definition "Moderately inclined to very steep; short open depression with concave cross-section; eroded by collapse; landslides; creep or surface wash." ;
    skos:notation "ALC" ;
    skos:prefLabel "Alcove" ;
    schema:url "https://github.com/ternaustralia/dawe-rlp-vocabs/tree/main/vocab_files/categorical_collections/luts/landform-element.ttl"^^xsd:anyURI ;
.

<https://linked.data.gov.au/def/nrm/e31ccd59-0ce4-56ad-87a9-4e7a1cda9605>
    a skos:Concept ;
    dcterms:identifier 78 ;
    dcterms:source <https://core.vocabs.paratoo.tern.org.au/api/lut-landform-elements> ;
    rdfs:isDefinedBy <https://linked.data.gov.au/def/nrm> ;
    skos:definition "Open depression excavated by human activity." ;
    skos:notation "TRE" ;
    skos:prefLabel "Trench" ;
    schema:url "https://github.com/ternaustralia/dawe-rlp-vocabs/tree/main/vocab_files/categorical_collections/luts/landform-element.ttl"^^xsd:anyURI ;
.

<https://linked.data.gov.au/def/nrm/e705f231-3807-5f0b-9afd-59a1c9093a36>
    a skos:Concept ;
    dcterms:identifier 53 ;
    dcterms:source <https://core.vocabs.paratoo.tern.org.au/api/lut-landform-elements> ;
    rdfs:isDefinedBy <https://linked.data.gov.au/def/nrm> ;
    skos:definition "Long; generally sinuous; low ridge built up from materials originally deposited by stream flow along the line of a former stream channel. The landform element may include a depression marking the old stream bed; and relict levees." ;
    skos:notation "PST" ;
    skos:prefLabel "Prior stream" ;
    schema:url "https://github.com/ternaustralia/dawe-rlp-vocabs/tree/main/vocab_files/categorical_collections/luts/landform-element.ttl"^^xsd:anyURI ;
.

<https://linked.data.gov.au/def/nrm/e874a1f0-e788-5a8c-9331-4b8329222759>
    a skos:Concept ;
    dcterms:identifier 24 ;
    dcterms:source <https://core.vocabs.paratoo.tern.org.au/api/lut-landform-elements> ;
    rdfs:isDefinedBy <https://linked.data.gov.au/def/nrm> ;
    skos:definition "Moderately inclined to very steep ridge or hillock built up by the wind. This element may comprise dunecrest and duneslope." ;
    skos:notation "DUN" ;
    skos:prefLabel "Dune" ;
    schema:url "https://github.com/ternaustralia/dawe-rlp-vocabs/tree/main/vocab_files/categorical_collections/luts/landform-element.ttl"^^xsd:anyURI ;
.

<https://linked.data.gov.au/def/nrm/eecee680-ecd8-5955-8434-dc9e7246f08d>
    a skos:Concept ;
    dcterms:identifier 41 ;
    dcterms:source <https://core.vocabs.paratoo.tern.org.au/api/lut-landform-elements> ;
    rdfs:isDefinedBy <https://linked.data.gov.au/def/nrm> ;
    skos:definition "Moderately inclined to very steep slope; eroded in the upper part and aggraded in the lower part by water-aided mass movement; characterised by irregular hummocks." ;
    skos:notation "LDS" ;
    skos:prefLabel "Landslide" ;
    schema:url "https://github.com/ternaustralia/dawe-rlp-vocabs/tree/main/vocab_files/categorical_collections/luts/landform-element.ttl"^^xsd:anyURI ;
.

<https://linked.data.gov.au/def/nrm/f1c3145c-ff9d-5303-8281-e2a9866167d7>
    a skos:Concept ;
    dcterms:identifier 36 ;
    dcterms:source <https://core.vocabs.paratoo.tern.org.au/api/lut-landform-elements> ;
    rdfs:isDefinedBy <https://linked.data.gov.au/def/nrm> ;
    skos:definition "Gently inclined to precipitous slope; commonly simple and maximal; eroded by sheet wash; creep or water-aided mass movement. A typical element of mountains; hills; low hills and rises." ;
    skos:notation "HSL" ;
    skos:prefLabel "Hillslope" ;
    schema:url "https://github.com/ternaustralia/dawe-rlp-vocabs/tree/main/vocab_files/categorical_collections/luts/landform-element.ttl"^^xsd:anyURI ;
.

<https://linked.data.gov.au/def/nrm/f38db675-d185-5bc3-ba02-3c30394b38dc>
    a skos:Concept ;
    dcterms:identifier 4 ;
    dcterms:source <https://core.vocabs.paratoo.tern.org.au/api/lut-landform-elements> ;
    rdfs:isDefinedBy <https://linked.data.gov.au/def/nrm> ;
    skos:definition "Elongated; gently to moderately inclined; low ridge built up by channelled stream flow; part of a stream bed." ;
    skos:notation "BAR" ;
    skos:prefLabel "Bar (stream bar)" ;
    schema:url "https://github.com/ternaustralia/dawe-rlp-vocabs/tree/main/vocab_files/categorical_collections/luts/landform-element.ttl"^^xsd:anyURI ;
.

<https://linked.data.gov.au/def/nrm/f823af68-b200-57b2-9d6e-c1f15f01b4a4>
    a skos:Concept ;
    dcterms:identifier 80 ;
    dcterms:source <https://core.vocabs.paratoo.tern.org.au/api/lut-landform-elements> ;
    rdfs:isDefinedBy <https://linked.data.gov.au/def/nrm> ;
    skos:definition "Small; gently inclined to level flat; aggraded or sometimes eroded by channelled or overbank stream flow; typically enclosed by hillslopes; a miniature alluvial plain landform pattern." ;
    skos:notation "VLF" ;
    skos:prefLabel "Valley flat" ;
    schema:url "https://github.com/ternaustralia/dawe-rlp-vocabs/tree/main/vocab_files/categorical_collections/luts/landform-element.ttl"^^xsd:anyURI ;
.

<https://linked.data.gov.au/def/nrm/c1a58967-cb12-4c2c-a7ca-9cee2589919c>
    a skos:Collection ;
    dcterms:description "A collection of landform element types and its codes." ;
    dcterms:source <https://core.vocabs.paratoo.tern.org.au/api/lut-landform-elements> ;
    rdfs:isDefinedBy <https://linked.data.gov.au/def/nrm> ;
    skos:member
        <https://linked.data.gov.au/def/nrm/032a1c8b-1048-5c81-bd06-8afce5c12451> ,
        <https://linked.data.gov.au/def/nrm/045be349-f9ed-52d6-89ca-68c7ade53e41> ,
        <https://linked.data.gov.au/def/nrm/077edbc4-8980-5e85-a6eb-1f4bd3aa1bbf> ,
        <https://linked.data.gov.au/def/nrm/0de17230-6ae6-5c2e-ab07-0bbe262a3501> ,
        <https://linked.data.gov.au/def/nrm/0eec5735-6c35-58bf-9cc7-d129f4c6b8b2> ,
        <https://linked.data.gov.au/def/nrm/115cecfd-35f7-51bf-b884-6267b453f50a> ,
        <https://linked.data.gov.au/def/nrm/1248ad7d-fb9c-564f-93c4-0c6bf3fe9088> ,
        <https://linked.data.gov.au/def/nrm/130cad8e-0a82-515a-ad75-6b84d165db6c> ,
        <https://linked.data.gov.au/def/nrm/141a8baa-89e0-5a55-b9fd-05a3c0b8c79c> ,
        <https://linked.data.gov.au/def/nrm/1431e5bb-f41a-56cc-b685-9aeed406fe63> ,
        <https://linked.data.gov.au/def/nrm/1470deb8-2762-5fd9-8c53-fc6cf2f18a4e> ,
        <https://linked.data.gov.au/def/nrm/1958c732-bbdd-5984-acec-5f56c2b82a06> ,
        <https://linked.data.gov.au/def/nrm/1ed7b887-8971-5d45-8ada-48e18386de45> ,
        <https://linked.data.gov.au/def/nrm/1fc7edc1-8d57-568f-9a98-9ab9ddcf2816> ,
        <https://linked.data.gov.au/def/nrm/283386fa-c297-5d2a-b453-fca857ddf51d> ,
        <https://linked.data.gov.au/def/nrm/287d64df-98f4-58c3-950e-2356a15687fd> ,
        <https://linked.data.gov.au/def/nrm/2ac8be18-9aae-56e3-aa07-65929e667648> ,
        <https://linked.data.gov.au/def/nrm/30bd2063-582d-5156-8ea0-faab8d16b102> ,
        <https://linked.data.gov.au/def/nrm/368641eb-467f-570b-9846-e8ebccb10186> ,
        <https://linked.data.gov.au/def/nrm/37421601-50ec-5371-b697-e9e18a54ba92> ,
        <https://linked.data.gov.au/def/nrm/37480929-9e0f-5ad7-8df9-914920540692> ,
        <https://linked.data.gov.au/def/nrm/392c68e8-e681-556d-a1ae-4a7aecf5144d> ,
        <https://linked.data.gov.au/def/nrm/41df86fc-66ec-5ef5-a605-edbe1b3c5edc> ,
        <https://linked.data.gov.au/def/nrm/4524d1f6-1951-502e-b7fe-8439acd3448a> ,
        <https://linked.data.gov.au/def/nrm/45db9fbc-4730-51bb-9329-8818736698cc> ,
        <https://linked.data.gov.au/def/nrm/47eeb3d4-8cd0-50b5-b837-4a54a22e3f31> ,
        <https://linked.data.gov.au/def/nrm/496d5410-d95c-5fe0-9b67-f9364550c4e4> ,
        <https://linked.data.gov.au/def/nrm/4b14473a-033a-58f1-b02c-16f47da90265> ,
        <https://linked.data.gov.au/def/nrm/4ee55457-4922-5d00-b13d-ca381ad44f63> ,
        <https://linked.data.gov.au/def/nrm/548c40d1-6c33-511d-be44-0c9f4f1360da> ,
        <https://linked.data.gov.au/def/nrm/54c94292-798f-5a26-8455-d1a302756f4f> ,
        <https://linked.data.gov.au/def/nrm/55911768-52b3-5fff-b4cf-2dd0614583c0> ,
        <https://linked.data.gov.au/def/nrm/5b1e7e84-5a23-5444-91c1-f97a872bc38e> ,
        <https://linked.data.gov.au/def/nrm/5c7e64fc-188c-5d94-b727-c88458bc7f95> ,
        <https://linked.data.gov.au/def/nrm/5cd65691-a295-577c-9f94-cd4756337e3f> ,
        <https://linked.data.gov.au/def/nrm/5de0ce45-d559-57b0-8328-83e133672104> ,
        <https://linked.data.gov.au/def/nrm/63960cfe-9e04-52b7-8940-4d6c2ebe0a02> ,
        <https://linked.data.gov.au/def/nrm/64008844-d6ff-5fa3-9218-48a3d57ada21> ,
        <https://linked.data.gov.au/def/nrm/69a64f8c-65b5-5185-8e16-39ce4f28a839> ,
        <https://linked.data.gov.au/def/nrm/6ff1c19e-cd58-5c14-b39d-6c093ba8b994> ,
        <https://linked.data.gov.au/def/nrm/71bc069c-03d3-53a5-a8d7-ef6a8f039389> ,
        <https://linked.data.gov.au/def/nrm/7cb2f197-c3e8-5491-b0db-78b839405fd7> ,
        <https://linked.data.gov.au/def/nrm/85b66cd6-ced2-5176-8338-6cf889145d08> ,
        <https://linked.data.gov.au/def/nrm/8e448737-8d60-56a6-94df-9399d5b9e174> ,
        <https://linked.data.gov.au/def/nrm/93fed9db-1788-54b3-8731-89430eb8f79a> ,
        <https://linked.data.gov.au/def/nrm/95d1041f-0a82-50d5-9702-f58a95029f95> ,
        <https://linked.data.gov.au/def/nrm/987ae37a-02be-5ef7-a4a6-1b13406fa277> ,
        <https://linked.data.gov.au/def/nrm/9969b531-7f6c-54a6-a23c-123c332d3428> ,
        <https://linked.data.gov.au/def/nrm/9da5cf89-4487-5f93-b351-0782a42ae362> ,
        <https://linked.data.gov.au/def/nrm/9fcf1019-135e-5fad-9fab-ea6da190eb05> ,
        <https://linked.data.gov.au/def/nrm/a19a72a0-2433-5fd2-8f64-16503637b9ee> ,
        <https://linked.data.gov.au/def/nrm/a749658e-2521-5fe0-8aaf-e352c3639fc1> ,
        <https://linked.data.gov.au/def/nrm/a75e7c17-b8c5-50b2-a0ca-74cfc6a65229> ,
        <https://linked.data.gov.au/def/nrm/b2025ffe-3999-5c93-a6ef-295bfed37242> ,
        <https://linked.data.gov.au/def/nrm/b357ae54-1094-5957-bf45-500ceab54a37> ,
        <https://linked.data.gov.au/def/nrm/b4c53a4f-3e36-507e-8f29-6468c146cd3c> ,
        <https://linked.data.gov.au/def/nrm/b82cfeb6-1194-513a-ba81-5010cb9eb38b> ,
        <https://linked.data.gov.au/def/nrm/bc6e0ac3-f1ef-5f6b-bcf9-7e23b620f256> ,
        <https://linked.data.gov.au/def/nrm/bceaebcb-9ab0-54b0-8ea2-b66c3efe9490> ,
        <https://linked.data.gov.au/def/nrm/c1c77cbf-4251-5437-b8c8-c3e44304f023> ,
        <https://linked.data.gov.au/def/nrm/c21bb284-7262-5dee-bd5b-8ecfe47961a0> ,
        <https://linked.data.gov.au/def/nrm/c5274b62-aa6d-5168-a941-37842c6d4791> ,
        <https://linked.data.gov.au/def/nrm/c68c6fca-6465-5607-a2eb-32634881cddf> ,
        <https://linked.data.gov.au/def/nrm/c87e531a-ced5-579b-9c58-befdf3ee53b6> ,
        <https://linked.data.gov.au/def/nrm/cb894c58-d482-5471-a16d-eabb27d6cc5f> ,
        <https://linked.data.gov.au/def/nrm/d110a3b2-a34f-5d94-828d-e539c22ae2b5> ,
        <https://linked.data.gov.au/def/nrm/d7154911-ea70-5613-9b4d-8fb80b36cda0> ,
        <https://linked.data.gov.au/def/nrm/d85de894-c9f3-545d-a131-906301d4ff91> ,
        <https://linked.data.gov.au/def/nrm/d901256e-66ab-5e26-a806-17a6ab335ae7> ,
        <https://linked.data.gov.au/def/nrm/d9f167e1-bc10-56b3-8c13-5d6ee1213b10> ,
        <https://linked.data.gov.au/def/nrm/dd2d43e4-2a30-509f-817a-407b271e8204> ,
        <https://linked.data.gov.au/def/nrm/e13edfb1-b27f-5f73-ac06-bb40b2520684> ,
        <https://linked.data.gov.au/def/nrm/e2ca4495-5e11-5f98-9bf1-14ff4bb4bbd5> ,
        <https://linked.data.gov.au/def/nrm/e31ccd59-0ce4-56ad-87a9-4e7a1cda9605> ,
        <https://linked.data.gov.au/def/nrm/e705f231-3807-5f0b-9afd-59a1c9093a36> ,
        <https://linked.data.gov.au/def/nrm/e874a1f0-e788-5a8c-9331-4b8329222759> ,
        <https://linked.data.gov.au/def/nrm/eecee680-ecd8-5955-8434-dc9e7246f08d> ,
        <https://linked.data.gov.au/def/nrm/f1c3145c-ff9d-5303-8281-e2a9866167d7> ,
        <https://linked.data.gov.au/def/nrm/f38db675-d185-5bc3-ba02-3c30394b38dc> ,
        <https://linked.data.gov.au/def/nrm/f823af68-b200-57b2-9d6e-c1f15f01b4a4> ;
    skos:prefLabel "Landform element codes" ;
    schema:url "https://github.com/ternaustralia/dawe-rlp-vocabs/tree/main/vocab_files/categorical_collections/luts/landform-element.ttl"^^xsd:anyURI ;
.

