PREFIX dcterms: <http://purl.org/dc/terms/>
PREFIX rdfs: <http://www.w3.org/2000/01/rdf-schema#>
PREFIX schema: <https://schema.org/>
PREFIX skos: <http://www.w3.org/2004/02/skos/core#>
PREFIX xsd: <http://www.w3.org/2001/XMLSchema#>

<https://linked.data.gov.au/def/test/dawe-cv/c1a58967-cb12-4c2c-a7ca-9cee2589919c>
    a skos:Collection ;
    dcterms:description "A collection of landform element types and its codes." ;
    dcterms:source <http://vocabs.paratoo.tern.org.au:1337/api/lut-landform-elements> ;
    rdfs:isDefinedBy <https://linked.data.gov.au/def/nrm> ;
    skos:member
        <https://linked.data.gov.au/def/test/dawe-cv/090ab00d-476e-5b85-afb6-7cca342b3ebc> ,
        <https://linked.data.gov.au/def/test/dawe-cv/091d7ea0-3ff7-5bc4-a2ad-c899d79f1997> ,
        <https://linked.data.gov.au/def/test/dawe-cv/0984ff0a-ae49-5a2a-907d-431be99f9f2a> ,
        <https://linked.data.gov.au/def/test/dawe-cv/0a8fd92c-b8d0-5fba-a4d4-0d4c5d540f34> ,
        <https://linked.data.gov.au/def/test/dawe-cv/0be7b164-3f5b-53d7-a526-d8a97f8a7814> ,
        <https://linked.data.gov.au/def/test/dawe-cv/0c5ea218-0495-5aaf-bc9b-ea7316799ac8> ,
        <https://linked.data.gov.au/def/test/dawe-cv/0d181003-328e-5ef8-bcdc-707a72b36149> ,
        <https://linked.data.gov.au/def/test/dawe-cv/160d44e9-4010-50df-949b-b2353546d176> ,
        <https://linked.data.gov.au/def/test/dawe-cv/196cc8f4-ca9d-5013-b2d0-60d73ea9cb5a> ,
        <https://linked.data.gov.au/def/test/dawe-cv/2283665d-fda9-5f41-932c-a9ecfbcefa9c> ,
        <https://linked.data.gov.au/def/test/dawe-cv/2321310c-114e-5491-90c2-d0cfff822553> ,
        <https://linked.data.gov.au/def/test/dawe-cv/25c322d8-61d4-5127-bb2f-0156a5e5607f> ,
        <https://linked.data.gov.au/def/test/dawe-cv/29b4e0da-94de-58bb-87eb-9754614f2266> ,
        <https://linked.data.gov.au/def/test/dawe-cv/2c37886e-0e46-55b2-9049-9678e2195766> ,
        <https://linked.data.gov.au/def/test/dawe-cv/2c3b9fdc-5843-509d-9c5d-fe5c6f0329cb> ,
        <https://linked.data.gov.au/def/test/dawe-cv/2d5d3790-186a-5ee7-b41a-efa7df040e3c> ,
        <https://linked.data.gov.au/def/test/dawe-cv/39716724-eb65-5c47-9562-1007d34c4c5b> ,
        <https://linked.data.gov.au/def/test/dawe-cv/3b240bbb-ecac-533e-b103-92707b6b155a> ,
        <https://linked.data.gov.au/def/test/dawe-cv/3b244d0e-69c3-5d45-b551-ef0d8daabd43> ,
        <https://linked.data.gov.au/def/test/dawe-cv/40a5364e-049d-5e96-a5fb-a281372f0d81> ,
        <https://linked.data.gov.au/def/test/dawe-cv/435c0396-dbb2-5f3f-8b1a-01b8262901c6> ,
        <https://linked.data.gov.au/def/test/dawe-cv/4e7b818a-a4b7-5f47-b638-67ae01575c90> ,
        <https://linked.data.gov.au/def/test/dawe-cv/4fd6db54-73f3-5ece-b8a7-a7e56c1afdcc> ,
        <https://linked.data.gov.au/def/test/dawe-cv/5083d690-4761-555e-a1c0-d6a1cb08ae97> ,
        <https://linked.data.gov.au/def/test/dawe-cv/51183458-2bce-5047-a2a6-17cdea865fc9> ,
        <https://linked.data.gov.au/def/test/dawe-cv/5316c0f4-4c8c-583a-bc88-db10c3ca9987> ,
        <https://linked.data.gov.au/def/test/dawe-cv/584cf753-d739-5040-851d-872add4a2e52> ,
        <https://linked.data.gov.au/def/test/dawe-cv/5f8d5903-968d-5e8a-bc39-c7fb5d82ee1c> ,
        <https://linked.data.gov.au/def/test/dawe-cv/602d9ed2-71be-56b3-9c68-04a92162a5c0> ,
        <https://linked.data.gov.au/def/test/dawe-cv/6587cbb1-a6cf-5bad-bb8d-313607ae1f11> ,
        <https://linked.data.gov.au/def/test/dawe-cv/6945adab-6973-559f-90ce-04f454dcf18b> ,
        <https://linked.data.gov.au/def/test/dawe-cv/6cd065ab-bc16-5f20-817d-ba9deff03e0d> ,
        <https://linked.data.gov.au/def/test/dawe-cv/6dc7e12f-cb45-5602-9ac8-83f9e9fbbab7> ,
        <https://linked.data.gov.au/def/test/dawe-cv/6e63d4d1-e472-5c46-b6c8-a8275a01f845> ,
        <https://linked.data.gov.au/def/test/dawe-cv/7317acd5-1490-5367-a6df-05e606050ab2> ,
        <https://linked.data.gov.au/def/test/dawe-cv/74034049-2f3d-5285-b5de-7b3721d01f3d> ,
        <https://linked.data.gov.au/def/test/dawe-cv/75b3cf6d-7625-59de-9d4b-83a2220db206> ,
        <https://linked.data.gov.au/def/test/dawe-cv/76e33646-90e7-5181-8f19-971161b50bc4> ,
        <https://linked.data.gov.au/def/test/dawe-cv/7987ec07-7798-58e6-ba90-d1eef7ccca57> ,
        <https://linked.data.gov.au/def/test/dawe-cv/7a751103-0da3-517a-b8fd-6f1d23a11fac> ,
        <https://linked.data.gov.au/def/test/dawe-cv/7a751c07-1647-5385-9d99-4d4a2ccfee99> ,
        <https://linked.data.gov.au/def/test/dawe-cv/82b726cd-c6b3-5653-8e29-522959cb701e> ,
        <https://linked.data.gov.au/def/test/dawe-cv/869ecf37-5e73-5692-951d-a474f612f466> ,
        <https://linked.data.gov.au/def/test/dawe-cv/8a947829-cd2f-51b7-9165-4d0daf9ce69a> ,
        <https://linked.data.gov.au/def/test/dawe-cv/8c55054a-3230-5d27-9b48-e380f276bd3c> ,
        <https://linked.data.gov.au/def/test/dawe-cv/93ec996a-efcc-55eb-9326-df8acb2bc927> ,
        <https://linked.data.gov.au/def/test/dawe-cv/960df542-0451-5092-96a5-6a9dd22b1118> ,
        <https://linked.data.gov.au/def/test/dawe-cv/986f781e-5da7-55bc-ae10-8c97d9d54910> ,
        <https://linked.data.gov.au/def/test/dawe-cv/98cf6325-95bf-575d-bf79-e4536646e7ff> ,
        <https://linked.data.gov.au/def/test/dawe-cv/9a9295db-de60-5066-ad35-917678cae36d> ,
        <https://linked.data.gov.au/def/test/dawe-cv/9da6a4ed-27a1-5c30-87b6-84e4a56dba99> ,
        <https://linked.data.gov.au/def/test/dawe-cv/9e22fdaf-48e4-5172-bb86-95545f600e7d> ,
        <https://linked.data.gov.au/def/test/dawe-cv/a4338ea4-ce49-56df-b773-8c33a9b528b2> ,
        <https://linked.data.gov.au/def/test/dawe-cv/a7b6a6b8-0b0b-5f51-8706-1ad35851a117> ,
        <https://linked.data.gov.au/def/test/dawe-cv/b1887a7f-1df3-5b72-8494-a12009faf955> ,
        <https://linked.data.gov.au/def/test/dawe-cv/b2139c18-0220-5fce-98d0-4847e17919cc> ,
        <https://linked.data.gov.au/def/test/dawe-cv/b459407f-82fe-5212-80c0-dfd4e3d49531> ,
        <https://linked.data.gov.au/def/test/dawe-cv/b6c1efcd-7bac-5d4d-aca5-f85f5b1e8a8a> ,
        <https://linked.data.gov.au/def/test/dawe-cv/b87ac878-c02d-50ee-b04c-a82bcb3e02d6> ,
        <https://linked.data.gov.au/def/test/dawe-cv/bbefbe1f-e0b3-5c10-a425-a179638c5d63> ,
        <https://linked.data.gov.au/def/test/dawe-cv/be9158a1-5d0c-5558-ab3f-6c7c1e79fb9e> ,
        <https://linked.data.gov.au/def/test/dawe-cv/bee94ec9-b2b2-5d62-91c3-eb362fcc79e3> ,
        <https://linked.data.gov.au/def/test/dawe-cv/bf8d1824-2df8-59c8-b2e8-eadecb0ef4d2> ,
        <https://linked.data.gov.au/def/test/dawe-cv/c1931b42-0124-51c1-9798-fb1488c9d84e> ,
        <https://linked.data.gov.au/def/test/dawe-cv/d024e54c-13e3-5a3c-8617-daa69b0274c7> ,
        <https://linked.data.gov.au/def/test/dawe-cv/d1732611-cc2f-5e6f-846a-da0adc40a439> ,
        <https://linked.data.gov.au/def/test/dawe-cv/d632f875-823d-5fd3-bc6e-9741e735fe4a> ,
        <https://linked.data.gov.au/def/test/dawe-cv/d7481c8e-dcec-5415-b212-df2326a60bbd> ,
        <https://linked.data.gov.au/def/test/dawe-cv/d7b593d8-badc-562c-940b-352881cbb942> ,
        <https://linked.data.gov.au/def/test/dawe-cv/d8c0b7fa-90ad-583d-b0d3-61046094cbb6> ,
        <https://linked.data.gov.au/def/test/dawe-cv/dc1f22f5-76c7-512d-86a2-095d911d3829> ,
        <https://linked.data.gov.au/def/test/dawe-cv/df10c1e5-8fa4-5e36-8357-6fb9d2bd5c75> ,
        <https://linked.data.gov.au/def/test/dawe-cv/e614b305-192b-5122-8702-bd3b0583f644> ,
        <https://linked.data.gov.au/def/test/dawe-cv/ede972cc-963e-57f3-b594-ed4a137ed9dc> ,
        <https://linked.data.gov.au/def/test/dawe-cv/ef20c946-0016-56a6-b198-50d7fc809686> ,
        <https://linked.data.gov.au/def/test/dawe-cv/f29ebd25-4eb7-5619-b8d1-ddd4a1c1214a> ,
        <https://linked.data.gov.au/def/test/dawe-cv/f29fe987-89e1-597f-881d-1b89ff446c18> ,
        <https://linked.data.gov.au/def/test/dawe-cv/f5ee0c0a-6a38-539e-9288-b5b3a5606e27> ,
        <https://linked.data.gov.au/def/test/dawe-cv/f6f2e07c-dda2-5abd-8a22-2a2ff2e8521a> ,
        <https://linked.data.gov.au/def/test/dawe-cv/f8726949-6dff-53cd-8b52-996a50eac071> ;
    skos:prefLabel "Landform element codes" ;
    schema:url "https://github.com/ternaustralia/dawe-rlp-vocabs/tree/main/vocab_files/categorical_collections/luts/landform-element.ttl"^^xsd:anyURI ;
.

<https://linked.data.gov.au/def/test/dawe-cv/090ab00d-476e-5b85-afb6-7cca342b3ebc>
    a skos:Concept ;
    dcterms:identifier 53 ;
    dcterms:source <http://vocabs.paratoo.tern.org.au:1337/api/lut-landform-elements> ;
    rdfs:isDefinedBy <https://linked.data.gov.au/def/nrm> ;
    skos:definition "Long; generally sinuous; low ridge built up from materials originally deposited by stream flow along the line of a former stream channel. The landform element may include a depression marking the old stream bed; and relict levees." ;
    skos:notation "PST" ;
    skos:prefLabel "Prior stream" ;
    schema:url "https://github.com/ternaustralia/dawe-rlp-vocabs/tree/main/vocab_files/categorical_collections/luts/landform-element.ttl"^^xsd:anyURI ;
.

<https://linked.data.gov.au/def/test/dawe-cv/091d7ea0-3ff7-5bc4-a2ad-c899d79f1997>
    a skos:Concept ;
    dcterms:identifier 59 ;
    dcterms:source <http://vocabs.paratoo.tern.org.au:1337/api/lut-landform-elements> ;
    rdfs:isDefinedBy <https://linked.data.gov.au/def/nrm> ;
    skos:definition "Flat of consolidated rock eroded by waves." ;
    skos:notation "RPL" ;
    skos:prefLabel "Rock platform" ;
    schema:url "https://github.com/ternaustralia/dawe-rlp-vocabs/tree/main/vocab_files/categorical_collections/luts/landform-element.ttl"^^xsd:anyURI ;
.

<https://linked.data.gov.au/def/test/dawe-cv/0984ff0a-ae49-5a2a-907d-431be99f9f2a>
    a skos:Concept ;
    dcterms:identifier 69 ;
    dcterms:source <http://vocabs.paratoo.tern.org.au:1337/api/lut-landform-elements> ;
    rdfs:isDefinedBy <https://linked.data.gov.au/def/nrm> ;
    skos:definition "See Tidal flat." ;
    skos:notation "STF" ;
    skos:prefLabel "Supratidal flat" ;
    schema:url "https://github.com/ternaustralia/dawe-rlp-vocabs/tree/main/vocab_files/categorical_collections/luts/landform-element.ttl"^^xsd:anyURI ;
.

<https://linked.data.gov.au/def/test/dawe-cv/0a8fd92c-b8d0-5fba-a4d4-0d4c5d540f34>
    a skos:Concept ;
    dcterms:identifier 54 ;
    dcterms:source <http://vocabs.paratoo.tern.org.au:1337/api/lut-landform-elements> ;
    rdfs:isDefinedBy <https://linked.data.gov.au/def/nrm> ;
    skos:definition "Flat built up to sea level by marine organisms." ;
    skos:notation "REF" ;
    skos:prefLabel "Reef flat" ;
    schema:url "https://github.com/ternaustralia/dawe-rlp-vocabs/tree/main/vocab_files/categorical_collections/luts/landform-element.ttl"^^xsd:anyURI ;
.

<https://linked.data.gov.au/def/test/dawe-cv/0be7b164-3f5b-53d7-a526-d8a97f8a7814>
    a skos:Concept ;
    dcterms:identifier 2 ;
    dcterms:source <http://vocabs.paratoo.tern.org.au:1337/api/lut-landform-elements> ;
    rdfs:isDefinedBy <https://linked.data.gov.au/def/nrm> ;
    skos:definition "Large flat resulting from aggradation by overbank stream flow at some distance from the stream channel and in some cases biological (peat) accumulation; often characterised by a high watertable and the presence of swamps or lakes; part of a covered plain landform pattern." ;
    skos:notation "BKP" ;
    skos:prefLabel "Backplain" ;
    schema:url "https://github.com/ternaustralia/dawe-rlp-vocabs/tree/main/vocab_files/categorical_collections/luts/landform-element.ttl"^^xsd:anyURI ;
.

<https://linked.data.gov.au/def/test/dawe-cv/0c5ea218-0495-5aaf-bc9b-ea7316799ac8>
    a skos:Concept ;
    dcterms:identifier 75 ;
    dcterms:source <http://vocabs.paratoo.tern.org.au:1337/api/lut-landform-elements> ;
    rdfs:isDefinedBy <https://linked.data.gov.au/def/nrm> ;
    skos:definition "Intermittently water-filled open depression in parts eroded; excavated; built up and aggraded by channelled tide-water flow; type of stream channel characterised by a rapid increase in width downstream." ;
    skos:notation "TDC" ;
    skos:prefLabel "Tidal creek" ;
    schema:url "https://github.com/ternaustralia/dawe-rlp-vocabs/tree/main/vocab_files/categorical_collections/luts/landform-element.ttl"^^xsd:anyURI ;
.

<https://linked.data.gov.au/def/test/dawe-cv/0d181003-328e-5ef8-bcdc-707a72b36149>
    a skos:Concept ;
    dcterms:identifier 64 ;
    dcterms:source <http://vocabs.paratoo.tern.org.au:1337/api/lut-landform-elements> ;
    rdfs:isDefinedBy <https://linked.data.gov.au/def/nrm> ;
    skos:definition "Large flat resulting from aggradation by channelled stream flow as a stream migrates from side to side; the dominant element of a meander plain landform pattern. This landform element may include occurrences of scroll; swale and ox-bow." ;
    skos:notation "SRP" ;
    skos:prefLabel "Scroll plain" ;
    schema:url "https://github.com/ternaustralia/dawe-rlp-vocabs/tree/main/vocab_files/categorical_collections/luts/landform-element.ttl"^^xsd:anyURI ;
.

<https://linked.data.gov.au/def/test/dawe-cv/160d44e9-4010-50df-949b-b2353546d176>
    a skos:Concept ;
    dcterms:identifier 18 ;
    dcterms:source <http://vocabs.paratoo.tern.org.au:1337/api/lut-landform-elements> ;
    rdfs:isDefinedBy <https://linked.data.gov.au/def/nrm> ;
    skos:definition "Steep to precipitous closed depression excavated by explosions due to volcanism; human action; or impact of an extraterrestrial object." ;
    skos:notation "CRA" ;
    skos:prefLabel "Crater" ;
    schema:url "https://github.com/ternaustralia/dawe-rlp-vocabs/tree/main/vocab_files/categorical_collections/luts/landform-element.ttl"^^xsd:anyURI ;
.

<https://linked.data.gov.au/def/test/dawe-cv/196cc8f4-ca9d-5013-b2d0-60d73ea9cb5a>
    a skos:Concept ;
    dcterms:identifier 13 ;
    dcterms:source <http://vocabs.paratoo.tern.org.au:1337/api/lut-landform-elements> ;
    rdfs:isDefinedBy <https://linked.data.gov.au/def/nrm> ;
    skos:definition "Precipitous to gently inclined; typically closed depression of concave contour and profile excavated by ice. The closed part of the depression may be shallow; the larger part being an open depression like an alcove." ;
    skos:notation "CIR" ;
    skos:prefLabel "Cirque" ;
    schema:url "https://github.com/ternaustralia/dawe-rlp-vocabs/tree/main/vocab_files/categorical_collections/luts/landform-element.ttl"^^xsd:anyURI ;
.

<https://linked.data.gov.au/def/test/dawe-cv/2283665d-fda9-5f41-932c-a9ecfbcefa9c>
    a skos:Concept ;
    dcterms:identifier 52 ;
    dcterms:source <http://vocabs.paratoo.tern.org.au:1337/api/lut-landform-elements> ;
    rdfs:isDefinedBy <https://linked.data.gov.au/def/nrm> ;
    skos:definition "Large; shallow; level-floored closed depression; intermittently water-filled; but mainly dry due to evaporation; bounded as a rule by flats aggraded by sheet flow and channelled stream flow." ;
    skos:notation "PLY" ;
    skos:prefLabel "Playa/pan" ;
    schema:url "https://github.com/ternaustralia/dawe-rlp-vocabs/tree/main/vocab_files/categorical_collections/luts/landform-element.ttl"^^xsd:anyURI ;
.

<https://linked.data.gov.au/def/test/dawe-cv/2321310c-114e-5491-90c2-d0cfff822553>
    a skos:Concept ;
    dcterms:identifier 48 ;
    dcterms:source <http://vocabs.paratoo.tern.org.au:1337/api/lut-landform-elements> ;
    rdfs:isDefinedBy <https://linked.data.gov.au/def/nrm> ;
    skos:definition "Sand dune with a long; scoop-shaped form; convex in the downwind direction so that its horns point upwind; whose ground plan approximates the form of a parabola. The dunes left behind can be referred to as trailing arms. Where many such dunes have traversed an area; these can give the appearance of linear dunes." ;
    skos:notation "DUP" ;
    skos:prefLabel "Parabolic dune" ;
    schema:url "https://github.com/ternaustralia/dawe-rlp-vocabs/tree/main/vocab_files/categorical_collections/luts/landform-element.ttl"^^xsd:anyURI ;
.

<https://linked.data.gov.au/def/test/dawe-cv/25c322d8-61d4-5127-bb2f-0156a5e5607f>
    a skos:Concept ;
    dcterms:identifier 57 ;
    dcterms:source <http://vocabs.paratoo.tern.org.au:1337/api/lut-landform-elements> ;
    rdfs:isDefinedBy <https://linked.data.gov.au/def/nrm> ;
    skos:definition "Slope of hillock of very low to extremely low relief (<30 m) (see Residual rise)." ;
    skos:notation "RES" ;
    skos:prefLabel "Riseslope" ;
    schema:url "https://github.com/ternaustralia/dawe-rlp-vocabs/tree/main/vocab_files/categorical_collections/luts/landform-element.ttl"^^xsd:anyURI ;
.

<https://linked.data.gov.au/def/test/dawe-cv/29b4e0da-94de-58bb-87eb-9754614f2266>
    a skos:Concept ;
    dcterms:identifier 17 ;
    dcterms:source <http://vocabs.paratoo.tern.org.au:1337/api/lut-landform-elements> ;
    rdfs:isDefinedBy <https://linked.data.gov.au/def/nrm> ;
    skos:definition "Hillock with a circular symmetry built up by volcanism. The crest may form a ring around a crater." ;
    skos:notation "CON" ;
    skos:prefLabel "Cone (volcanic)" ;
    schema:url "https://github.com/ternaustralia/dawe-rlp-vocabs/tree/main/vocab_files/categorical_collections/luts/landform-element.ttl"^^xsd:anyURI ;
.

<https://linked.data.gov.au/def/test/dawe-cv/2c37886e-0e46-55b2-9049-9678e2195766>
    a skos:Concept ;
    dcterms:identifier 50 ;
    dcterms:source <http://vocabs.paratoo.tern.org.au:1337/api/lut-landform-elements> ;
    rdfs:isDefinedBy <https://linked.data.gov.au/def/nrm> ;
    skos:definition "Closed depression excavated by human activity." ;
    skos:notation "PIT" ;
    skos:prefLabel "Pit" ;
    schema:url "https://github.com/ternaustralia/dawe-rlp-vocabs/tree/main/vocab_files/categorical_collections/luts/landform-element.ttl"^^xsd:anyURI ;
.

<https://linked.data.gov.au/def/test/dawe-cv/2c3b9fdc-5843-509d-9c5d-fe5c6f0329cb>
    a skos:Concept ;
    dcterms:identifier 47 ;
    dcterms:source <http://vocabs.paratoo.tern.org.au:1337/api/lut-landform-elements> ;
    rdfs:isDefinedBy <https://linked.data.gov.au/def/nrm> ;
    skos:definition "Long; curved; commonly water-filled closed depression eroded by channelled stream flow but closed as a result of aggradation by channelled or overbank stream flow during the formation of a meander plain landform pattern. The floor of an ox-bow may be more or less aggraded by overbank stream flow; wind; and biological (peat) accumulation." ;
    skos:notation "OXB" ;
    skos:prefLabel "Ox-bow" ;
    schema:url "https://github.com/ternaustralia/dawe-rlp-vocabs/tree/main/vocab_files/categorical_collections/luts/landform-element.ttl"^^xsd:anyURI ;
.

<https://linked.data.gov.au/def/test/dawe-cv/2d5d3790-186a-5ee7-b41a-efa7df040e3c>
    a skos:Concept ;
    dcterms:identifier 7 ;
    dcterms:source <http://vocabs.paratoo.tern.org.au:1337/api/lut-landform-elements> ;
    rdfs:isDefinedBy <https://linked.data.gov.au/def/nrm> ;
    skos:definition "Very long; nearly straight; low ridge; built up by waves and usually modified by wind. A beach ridge is often a relict feature remote from the beach." ;
    skos:notation "BRI" ;
    skos:prefLabel "Beach ridge" ;
    schema:url "https://github.com/ternaustralia/dawe-rlp-vocabs/tree/main/vocab_files/categorical_collections/luts/landform-element.ttl"^^xsd:anyURI ;
.

<https://linked.data.gov.au/def/test/dawe-cv/39716724-eb65-5c47-9562-1007d34c4c5b>
    a skos:Concept ;
    dcterms:identifier 67 ;
    dcterms:source <http://vocabs.paratoo.tern.org.au:1337/api/lut-landform-elements> ;
    rdfs:isDefinedBy <https://linked.data.gov.au/def/nrm> ;
    skos:definition "Linear; generally sinuous open depression; in parts eroded; excavated; built up and aggraded by channelled stream flow. This element comprises stream bed and banks." ;
    skos:notation "STC" ;
    skos:prefLabel "Stream channel" ;
    schema:url "https://github.com/ternaustralia/dawe-rlp-vocabs/tree/main/vocab_files/categorical_collections/luts/landform-element.ttl"^^xsd:anyURI ;
.

<https://linked.data.gov.au/def/test/dawe-cv/3b240bbb-ecac-533e-b103-92707b6b155a>
    a skos:Concept ;
    dcterms:identifier 76 ;
    dcterms:source <http://vocabs.paratoo.tern.org.au:1337/api/lut-landform-elements> ;
    rdfs:isDefinedBy <https://linked.data.gov.au/def/nrm> ;
    skos:definition "Large flat subject to inundation by water that is usually salt or brackish; aggradedby tides. An intertidal flat (ITF) is frequently inundated; a supratidal flat (STF) is seldom inundated." ;
    skos:notation "TDF" ;
    skos:prefLabel "Tidal flat" ;
    schema:url "https://github.com/ternaustralia/dawe-rlp-vocabs/tree/main/vocab_files/categorical_collections/luts/landform-element.ttl"^^xsd:anyURI ;
.

<https://linked.data.gov.au/def/test/dawe-cv/3b244d0e-69c3-5d45-b551-ef0d8daabd43>
    a skos:Concept ;
    dcterms:identifier 9 ;
    dcterms:source <http://vocabs.paratoo.tern.org.au:1337/api/lut-landform-elements> ;
    rdfs:isDefinedBy <https://linked.data.gov.au/def/nrm> ;
    skos:definition "(i) Short; very gently inclined to level minimal mid-slope in an embankment or cut face; eroded or aggraded by human activity. (ii) Flat built up by waves above a beach." ;
    skos:notation "BER" ;
    skos:prefLabel "Berm" ;
    schema:url "https://github.com/ternaustralia/dawe-rlp-vocabs/tree/main/vocab_files/categorical_collections/luts/landform-element.ttl"^^xsd:anyURI ;
.

<https://linked.data.gov.au/def/test/dawe-cv/40a5364e-049d-5e96-a5fb-a281372f0d81>
    a skos:Concept ;
    dcterms:identifier 37 ;
    dcterms:source <http://vocabs.paratoo.tern.org.au:1337/api/lut-landform-elements> ;
    rdfs:isDefinedBy <https://linked.data.gov.au/def/nrm> ;
    skos:definition "Very gently to moderately inclined rises or hillocks built up or eroded by wind and lacking distinct orientation or regular pattern." ;
    skos:notation "DUH" ;
    skos:prefLabel "Hummocky (weakly oriented dune)" ;
    schema:url "https://github.com/ternaustralia/dawe-rlp-vocabs/tree/main/vocab_files/categorical_collections/luts/landform-element.ttl"^^xsd:anyURI ;
.

<https://linked.data.gov.au/def/test/dawe-cv/435c0396-dbb2-5f3f-8b1a-01b8262901c6>
    a skos:Concept ;
    dcterms:identifier 43 ;
    dcterms:source <http://vocabs.paratoo.tern.org.au:1337/api/lut-landform-elements> ;
    rdfs:isDefinedBy <https://linked.data.gov.au/def/nrm> ;
    skos:definition "Large; sharp-crested; elongated; longitudinal (linear) dune or chain of sand dunes; oriented parallel; rather than transverse (perpendicular); to the prevailing wind. Not to be confused with the trailing arms of parabolic dunes." ;
    skos:notation "DUF" ;
    skos:prefLabel "Linear or longitudinal (seif) dune" ;
    schema:url "https://github.com/ternaustralia/dawe-rlp-vocabs/tree/main/vocab_files/categorical_collections/luts/landform-element.ttl"^^xsd:anyURI ;
.

<https://linked.data.gov.au/def/test/dawe-cv/4e7b818a-a4b7-5f47-b638-67ae01575c90>
    a skos:Concept ;
    dcterms:identifier 70 ;
    dcterms:source <http://vocabs.paratoo.tern.org.au:1337/api/lut-landform-elements> ;
    rdfs:isDefinedBy <https://linked.data.gov.au/def/nrm> ;
    skos:definition "(i) Linear; level-floored open depression excavated by wind; or left relict between ridges built up by wind or waves; or built up to a lesser height than them. (ii) Long; curved open or closed depression left relict between scrolls built up by channelled stream flow." ;
    skos:notation "SWL" ;
    skos:prefLabel "Swale" ;
    schema:url "https://github.com/ternaustralia/dawe-rlp-vocabs/tree/main/vocab_files/categorical_collections/luts/landform-element.ttl"^^xsd:anyURI ;
.

<https://linked.data.gov.au/def/test/dawe-cv/4fd6db54-73f3-5ece-b8a7-a7e56c1afdcc>
    a skos:Concept ;
    dcterms:identifier 20 ;
    dcterms:source <http://vocabs.paratoo.tern.org.au:1337/api/lut-landform-elements> ;
    rdfs:isDefinedBy <https://linked.data.gov.au/def/nrm> ;
    skos:definition "Flat eroded by human activity." ;
    skos:notation "COS" ;
    skos:prefLabel "Cut-over surface" ;
    schema:url "https://github.com/ternaustralia/dawe-rlp-vocabs/tree/main/vocab_files/categorical_collections/luts/landform-element.ttl"^^xsd:anyURI ;
.

<https://linked.data.gov.au/def/test/dawe-cv/5083d690-4761-555e-a1c0-d6a1cb08ae97>
    a skos:Concept ;
    dcterms:identifier 55 ;
    dcterms:source <http://vocabs.paratoo.tern.org.au:1337/api/lut-landform-elements> ;
    rdfs:isDefinedBy <https://linked.data.gov.au/def/nrm> ;
    skos:definition "Hillock of very low to extremely low relief (<30 m) and very gentle to steep slopes. This term is used to refer to an isolated rise surrounded by other landforms." ;
    skos:notation "RER" ;
    skos:prefLabel "Residual rise" ;
    schema:url "https://github.com/ternaustralia/dawe-rlp-vocabs/tree/main/vocab_files/categorical_collections/luts/landform-element.ttl"^^xsd:anyURI ;
.

<https://linked.data.gov.au/def/test/dawe-cv/51183458-2bce-5047-a2a6-17cdea865fc9>
    a skos:Concept ;
    dcterms:identifier 14 ;
    dcterms:source <http://vocabs.paratoo.tern.org.au:1337/api/lut-landform-elements> ;
    rdfs:isDefinedBy <https://linked.data.gov.au/def/nrm> ;
    skos:definition "Very wide; cliffed (greater than 72 degrees) maximal slope usually eroded by gravitational fall as a result of erosion of the base by various agencies; sometimes built up by marine organisms." ;
    skos:notation "CLI" ;
    skos:prefLabel "Cliff" ;
    schema:url "https://github.com/ternaustralia/dawe-rlp-vocabs/tree/main/vocab_files/categorical_collections/luts/landform-element.ttl"^^xsd:anyURI ;
.

<https://linked.data.gov.au/def/test/dawe-cv/5316c0f4-4c8c-583a-bc88-db10c3ca9987>
    a skos:Concept ;
    dcterms:identifier 68 ;
    dcterms:source <http://vocabs.paratoo.tern.org.au:1337/api/lut-landform-elements> ;
    rdfs:isDefinedBy <https://linked.data.gov.au/def/nrm> ;
    skos:definition "Very wide; level to gently inclined crest with abrupt margins; commonly eroded by water-aided mass movement or sheet wash." ;
    skos:notation "SUS" ;
    skos:prefLabel "Summit surface" ;
    schema:url "https://github.com/ternaustralia/dawe-rlp-vocabs/tree/main/vocab_files/categorical_collections/luts/landform-element.ttl"^^xsd:anyURI ;
.

<https://linked.data.gov.au/def/test/dawe-cv/584cf753-d739-5040-851d-872add4a2e52>
    a skos:Concept ;
    dcterms:identifier 16 ;
    dcterms:source <http://vocabs.paratoo.tern.org.au:1337/api/lut-landform-elements> ;
    rdfs:isDefinedBy <https://linked.data.gov.au/def/nrm> ;
    skos:definition "Steep-sided; circular or elliptical closed depression; commonly funnel-shaped; characterised by subsurface drainage and formed by collapse of underlying caves within bedrock." ;
    skos:notation "DOC" ;
    skos:prefLabel "Collapse doline" ;
    schema:url "https://github.com/ternaustralia/dawe-rlp-vocabs/tree/main/vocab_files/categorical_collections/luts/landform-element.ttl"^^xsd:anyURI ;
.

<https://linked.data.gov.au/def/test/dawe-cv/5f8d5903-968d-5e8a-bc39-c7fb5d82ee1c>
    a skos:Concept ;
    dcterms:identifier 74 ;
    dcterms:source <http://vocabs.paratoo.tern.org.au:1337/api/lut-landform-elements> ;
    rdfs:isDefinedBy <https://linked.data.gov.au/def/nrm> ;
    skos:definition "Large or very large flat aggraded by channelled or overbank stream flow; standing above a scarp and no longer frequently inundated; part of a former flood plain." ;
    skos:notation "TEP" ;
    skos:prefLabel "Terrace plain" ;
    schema:url "https://github.com/ternaustralia/dawe-rlp-vocabs/tree/main/vocab_files/categorical_collections/luts/landform-element.ttl"^^xsd:anyURI ;
.

<https://linked.data.gov.au/def/test/dawe-cv/602d9ed2-71be-56b3-9c68-04a92162a5c0>
    a skos:Concept ;
    dcterms:identifier 23 ;
    dcterms:source <http://vocabs.paratoo.tern.org.au:1337/api/lut-landform-elements> ;
    rdfs:isDefinedBy <https://linked.data.gov.au/def/nrm> ;
    skos:definition "Level to gently inclined; long; narrow shallow open depression with smoothly concave cross-section rising to moderately inclined side slopes; eroded or aggraded by sheet wash." ;
    skos:notation "DDE" ;
    skos:prefLabel "Drainage depression" ;
    schema:url "https://github.com/ternaustralia/dawe-rlp-vocabs/tree/main/vocab_files/categorical_collections/luts/landform-element.ttl"^^xsd:anyURI ;
.

<https://linked.data.gov.au/def/test/dawe-cv/6587cbb1-a6cf-5bad-bb8d-313607ae1f11>
    a skos:Concept ;
    dcterms:identifier 5 ;
    dcterms:source <http://vocabs.paratoo.tern.org.au:1337/api/lut-landform-elements> ;
    rdfs:isDefinedBy <https://linked.data.gov.au/def/nrm> ;
    skos:definition "Crescent shaped dune with tips extending leeward (downwind); making this side concave and the windward (upwind) side convex. Barchan dunes tend to be arranged in chains extending in the dominant wind direction." ;
    skos:notation "DUB" ;
    skos:prefLabel "Barchan dune" ;
    schema:url "https://github.com/ternaustralia/dawe-rlp-vocabs/tree/main/vocab_files/categorical_collections/luts/landform-element.ttl"^^xsd:anyURI ;
.

<https://linked.data.gov.au/def/test/dawe-cv/6945adab-6973-559f-90ce-04f454dcf18b>
    a skos:Concept ;
    dcterms:identifier 22 ;
    dcterms:source <http://vocabs.paratoo.tern.org.au:1337/api/lut-landform-elements> ;
    rdfs:isDefinedBy <https://linked.data.gov.au/def/nrm> ;
    skos:definition "Basin excavated by wind erosion which removes loose material; commonly above a resistant or wet layer." ;
    skos:notation "DBA" ;
    skos:prefLabel "Deflation basin" ;
    schema:url "https://github.com/ternaustralia/dawe-rlp-vocabs/tree/main/vocab_files/categorical_collections/luts/landform-element.ttl"^^xsd:anyURI ;
.

<https://linked.data.gov.au/def/test/dawe-cv/6cd065ab-bc16-5f20-817d-ba9deff03e0d>
    a skos:Concept ;
    dcterms:identifier 73 ;
    dcterms:source <http://vocabs.paratoo.tern.org.au:1337/api/lut-landform-elements> ;
    rdfs:isDefinedBy <https://linked.data.gov.au/def/nrm> ;
    skos:definition "Small flat aggraded or eroded by channelled or overbank stream flow; standing above a scarp and no longer frequently inundated; a former valley flat or part of a former flood plain." ;
    skos:notation "TEF" ;
    skos:prefLabel "Terrace Flat" ;
    schema:url "https://github.com/ternaustralia/dawe-rlp-vocabs/tree/main/vocab_files/categorical_collections/luts/landform-element.ttl"^^xsd:anyURI ;
.

<https://linked.data.gov.au/def/test/dawe-cv/6dc7e12f-cb45-5602-9ac8-83f9e9fbbab7>
    a skos:Concept ;
    dcterms:identifier 42 ;
    dcterms:source <http://vocabs.paratoo.tern.org.au:1337/api/lut-landform-elements> ;
    rdfs:isDefinedBy <https://linked.data.gov.au/def/nrm> ;
    skos:definition "Very long; low; narrow; nearly level; sinuous ridge immediately adjacent to a stream channel; built up by overbank flow. Levees are built usually in pairs bounding the two sides of a stream channel; at the level reached by frequent floods. This element is part of a covered plain landform pattern. For an artificial levee; use Embankment. See also Prior stream." ;
    skos:notation "LEV" ;
    skos:prefLabel "Levee" ;
    schema:url "https://github.com/ternaustralia/dawe-rlp-vocabs/tree/main/vocab_files/categorical_collections/luts/landform-element.ttl"^^xsd:anyURI ;
.

<https://linked.data.gov.au/def/test/dawe-cv/6e63d4d1-e472-5c46-b6c8-a8275a01f845>
    a skos:Concept ;
    dcterms:identifier 80 ;
    dcterms:source <http://vocabs.paratoo.tern.org.au:1337/api/lut-landform-elements> ;
    rdfs:isDefinedBy <https://linked.data.gov.au/def/nrm> ;
    skos:definition "Small; gently inclined to level flat; aggraded or sometimes eroded by channelled or overbank stream flow; typically enclosed by hillslopes; a miniature alluvial plain landform pattern." ;
    skos:notation "VLF" ;
    skos:prefLabel "Valley flat" ;
    schema:url "https://github.com/ternaustralia/dawe-rlp-vocabs/tree/main/vocab_files/categorical_collections/luts/landform-element.ttl"^^xsd:anyURI ;
.

<https://linked.data.gov.au/def/test/dawe-cv/7317acd5-1490-5367-a6df-05e606050ab2>
    a skos:Concept ;
    dcterms:identifier 44 ;
    dcterms:source <http://vocabs.paratoo.tern.org.au:1337/api/lut-landform-elements> ;
    rdfs:isDefinedBy <https://linked.data.gov.au/def/nrm> ;
    skos:definition "Elongated; gently curved; low ridge built up by wind on the margin of a playa; typically with a moderate; wave-modified slope towards the playa and a gentle outer slope." ;
    skos:notation "LUN" ;
    skos:prefLabel "Lunette" ;
    schema:url "https://github.com/ternaustralia/dawe-rlp-vocabs/tree/main/vocab_files/categorical_collections/luts/landform-element.ttl"^^xsd:anyURI ;
.

<https://linked.data.gov.au/def/test/dawe-cv/74034049-2f3d-5285-b5de-7b3721d01f3d>
    a skos:Concept ;
    dcterms:identifier 65 ;
    dcterms:source <http://vocabs.paratoo.tern.org.au:1337/api/lut-landform-elements> ;
    rdfs:isDefinedBy <https://linked.data.gov.au/def/nrm> ;
    skos:definition "Steep-sided; circular or elliptical closed depression; commonly funnel-shaped; characterised by subsurface drainage and formed by dissolution of the surface or underlying within bedrock." ;
    skos:notation "DOL" ;
    skos:prefLabel "Solution doline" ;
    schema:url "https://github.com/ternaustralia/dawe-rlp-vocabs/tree/main/vocab_files/categorical_collections/luts/landform-element.ttl"^^xsd:anyURI ;
.

<https://linked.data.gov.au/def/test/dawe-cv/75b3cf6d-7625-59de-9d4b-83a2220db206>
    a skos:Concept ;
    dcterms:identifier 10 ;
    dcterms:source <http://vocabs.paratoo.tern.org.au:1337/api/lut-landform-elements> ;
    rdfs:isDefinedBy <https://linked.data.gov.au/def/nrm> ;
    skos:definition "Usually small; open or closed depression excavated by the wind." ;
    skos:notation "BOU" ;
    skos:prefLabel "Blow-out" ;
    schema:url "https://github.com/ternaustralia/dawe-rlp-vocabs/tree/main/vocab_files/categorical_collections/luts/landform-element.ttl"^^xsd:anyURI ;
.

<https://linked.data.gov.au/def/test/dawe-cv/76e33646-90e7-5181-8f19-971161b50bc4>
    a skos:Concept ;
    dcterms:identifier 78 ;
    dcterms:source <http://vocabs.paratoo.tern.org.au:1337/api/lut-landform-elements> ;
    rdfs:isDefinedBy <https://linked.data.gov.au/def/nrm> ;
    skos:definition "Open depression excavated by human activity." ;
    skos:notation "TRE" ;
    skos:prefLabel "Trench" ;
    schema:url "https://github.com/ternaustralia/dawe-rlp-vocabs/tree/main/vocab_files/categorical_collections/luts/landform-element.ttl"^^xsd:anyURI ;
.

<https://linked.data.gov.au/def/test/dawe-cv/7987ec07-7798-58e6-ba90-d1eef7ccca57>
    a skos:Concept ;
    dcterms:identifier 6 ;
    dcterms:source <http://vocabs.paratoo.tern.org.au:1337/api/lut-landform-elements> ;
    rdfs:isDefinedBy <https://linked.data.gov.au/def/nrm> ;
    skos:definition "Short; low; very wide slope; gently or moderately inclined; built up or eroded by waves; forming the shore of a lake or sea." ;
    skos:notation "BEA" ;
    skos:prefLabel "Beach" ;
    schema:url "https://github.com/ternaustralia/dawe-rlp-vocabs/tree/main/vocab_files/categorical_collections/luts/landform-element.ttl"^^xsd:anyURI ;
.

<https://linked.data.gov.au/def/test/dawe-cv/7a751103-0da3-517a-b8fd-6f1d23a11fac>
    a skos:Concept ;
    dcterms:identifier 33 ;
    dcterms:source <http://vocabs.paratoo.tern.org.au:1337/api/lut-landform-elements> ;
    rdfs:isDefinedBy <https://linked.data.gov.au/def/nrm> ;
    skos:definition "Very long; nearly straight moderately inclined to very steep ridge built up by the wind from material from an adjacent beach." ;
    skos:notation "FOR" ;
    skos:prefLabel "Foredune" ;
    schema:url "https://github.com/ternaustralia/dawe-rlp-vocabs/tree/main/vocab_files/categorical_collections/luts/landform-element.ttl"^^xsd:anyURI ;
.

<https://linked.data.gov.au/def/test/dawe-cv/7a751c07-1647-5385-9d99-4d4a2ccfee99>
    a skos:Concept ;
    dcterms:identifier 77 ;
    dcterms:source <http://vocabs.paratoo.tern.org.au:1337/api/lut-landform-elements> ;
    rdfs:isDefinedBy <https://linked.data.gov.au/def/nrm> ;
    skos:definition "Steep to precipitous hillock; typically convex; with a surface mainly of bare rock; either coherent or comprising subangular to rounded; large boulders (exhumed core-stones; also themselves called tors) separated by open fissures; eroded by sheet wash or water-aided mass movement." ;
    skos:notation "TOR" ;
    skos:prefLabel "Tor" ;
    schema:url "https://github.com/ternaustralia/dawe-rlp-vocabs/tree/main/vocab_files/categorical_collections/luts/landform-element.ttl"^^xsd:anyURI ;
.

<https://linked.data.gov.au/def/test/dawe-cv/82b726cd-c6b3-5653-8e29-522959cb701e>
    a skos:Concept ;
    dcterms:identifier 26 ;
    dcterms:source <http://vocabs.paratoo.tern.org.au:1337/api/lut-landform-elements> ;
    rdfs:isDefinedBy <https://linked.data.gov.au/def/nrm> ;
    skos:definition "Slope built up or eroded by the wind (see Dune)." ;
    skos:notation "DUS" ;
    skos:prefLabel "Dune slope" ;
    schema:url "https://github.com/ternaustralia/dawe-rlp-vocabs/tree/main/vocab_files/categorical_collections/luts/landform-element.ttl"^^xsd:anyURI ;
.

<https://linked.data.gov.au/def/test/dawe-cv/869ecf37-5e73-5692-951d-a474f612f466>
    a skos:Concept ;
    dcterms:identifier 63 ;
    dcterms:source <http://vocabs.paratoo.tern.org.au:1337/api/lut-landform-elements> ;
    rdfs:isDefinedBy <https://linked.data.gov.au/def/nrm> ;
    skos:definition "Long; curved; very low ridge built up by channelled stream flow and left relict by channel migration. Part of a meander plain landform pattern." ;
    skos:notation "SCR" ;
    skos:prefLabel "Scroll" ;
    schema:url "https://github.com/ternaustralia/dawe-rlp-vocabs/tree/main/vocab_files/categorical_collections/luts/landform-element.ttl"^^xsd:anyURI ;
.

<https://linked.data.gov.au/def/test/dawe-cv/8a947829-cd2f-51b7-9165-4d0daf9ce69a>
    a skos:Concept ;
    dcterms:identifier 31 ;
    dcterms:source <http://vocabs.paratoo.tern.org.au:1337/api/lut-landform-elements> ;
    rdfs:isDefinedBy <https://linked.data.gov.au/def/nrm> ;
    skos:definition "Flat inclined radially away from a point on the margin or at the end of a stream channel; aggraded by overbank stream flow; or by channelled stream flow associated with channels developed within the overbank flow; part of a covered plain landform pattern." ;
    skos:notation "FLD" ;
    skos:prefLabel "Floodout" ;
    schema:url "https://github.com/ternaustralia/dawe-rlp-vocabs/tree/main/vocab_files/categorical_collections/luts/landform-element.ttl"^^xsd:anyURI ;
.

<https://linked.data.gov.au/def/test/dawe-cv/8c55054a-3230-5d27-9b48-e380f276bd3c>
    a skos:Concept ;
    dcterms:identifier 3 ;
    dcterms:source <http://vocabs.paratoo.tern.org.au:1337/api/lut-landform-elements> ;
    rdfs:isDefinedBy <https://linked.data.gov.au/def/nrm> ;
    skos:definition "Very short; very wide slope; moderately inclined to precipitous; forming the marginal upper parts of a stream channel and resulting from erosion or aggradation by channelled stream flow." ;
    skos:notation "BAN" ;
    skos:prefLabel "Bank (stream bank)" ;
    schema:url "https://github.com/ternaustralia/dawe-rlp-vocabs/tree/main/vocab_files/categorical_collections/luts/landform-element.ttl"^^xsd:anyURI ;
.

<https://linked.data.gov.au/def/test/dawe-cv/93ec996a-efcc-55eb-9326-df8acb2bc927>
    a skos:Concept ;
    dcterms:identifier 15 ;
    dcterms:source <http://vocabs.paratoo.tern.org.au:1337/api/lut-landform-elements> ;
    rdfs:isDefinedBy <https://linked.data.gov.au/def/nrm> ;
    skos:definition "Slope situated below a cliff; with its contours generally parallel to the line of the cliff eroded by sheet wash or water-aided mass movement; and aggraded locally by collapsed material from above." ;
    skos:notation "CFS" ;
    skos:prefLabel "Cliff-footslope" ;
    schema:url "https://github.com/ternaustralia/dawe-rlp-vocabs/tree/main/vocab_files/categorical_collections/luts/landform-element.ttl"^^xsd:anyURI ;
.

<https://linked.data.gov.au/def/test/dawe-cv/960df542-0451-5092-96a5-6a9dd22b1118>
    a skos:Concept ;
    dcterms:identifier 8 ;
    dcterms:source <http://vocabs.paratoo.tern.org.au:1337/api/lut-landform-elements> ;
    rdfs:isDefinedBy <https://linked.data.gov.au/def/nrm> ;
    skos:definition "Short; gently or very gently inclined minimal mid-slope element eroded or aggraded by any agent." ;
    skos:notation "BEN" ;
    skos:prefLabel "Bench" ;
    schema:url "https://github.com/ternaustralia/dawe-rlp-vocabs/tree/main/vocab_files/categorical_collections/luts/landform-element.ttl"^^xsd:anyURI ;
.

<https://linked.data.gov.au/def/test/dawe-cv/986f781e-5da7-55bc-ae10-8c97d9d54910>
    a skos:Concept ;
    dcterms:identifier 51 ;
    dcterms:source <http://vocabs.paratoo.tern.org.au:1337/api/lut-landform-elements> ;
    rdfs:isDefinedBy <https://linked.data.gov.au/def/nrm> ;
    skos:definition "Large; very gently inclined or level element; of unspecified geomorphological agent or mode of activity." ;
    skos:notation "PLA" ;
    skos:prefLabel "Plain" ;
    schema:url "https://github.com/ternaustralia/dawe-rlp-vocabs/tree/main/vocab_files/categorical_collections/luts/landform-element.ttl"^^xsd:anyURI ;
.

<https://linked.data.gov.au/def/test/dawe-cv/98cf6325-95bf-575d-bf79-e4536646e7ff>
    a skos:Concept ;
    dcterms:identifier 46 ;
    dcterms:source <http://vocabs.paratoo.tern.org.au:1337/api/lut-landform-elements> ;
    rdfs:isDefinedBy <https://linked.data.gov.au/def/nrm> ;
    skos:definition "Hillock built up by human activity." ;
    skos:notation "MOU" ;
    skos:prefLabel "Mound" ;
    schema:url "https://github.com/ternaustralia/dawe-rlp-vocabs/tree/main/vocab_files/categorical_collections/luts/landform-element.ttl"^^xsd:anyURI ;
.

<https://linked.data.gov.au/def/test/dawe-cv/9a9295db-de60-5066-ad35-917678cae36d>
    a skos:Concept ;
    dcterms:identifier 56 ;
    dcterms:source <http://vocabs.paratoo.tern.org.au:1337/api/lut-landform-elements> ;
    rdfs:isDefinedBy <https://linked.data.gov.au/def/nrm> ;
    skos:definition "Crest of hillock of very low to extremely low relief (<30 m) (see Residual rise)." ;
    skos:notation "REC" ;
    skos:prefLabel "Risecrest" ;
    schema:url "https://github.com/ternaustralia/dawe-rlp-vocabs/tree/main/vocab_files/categorical_collections/luts/landform-element.ttl"^^xsd:anyURI ;
.

<https://linked.data.gov.au/def/test/dawe-cv/9da6a4ed-27a1-5c30-87b6-84e4a56dba99>
    a skos:Concept ;
    dcterms:identifier 29 ;
    dcterms:source <http://vocabs.paratoo.tern.org.au:1337/api/lut-landform-elements> ;
    rdfs:isDefinedBy <https://linked.data.gov.au/def/nrm> ;
    skos:definition "Large; gently inclined to level element with radial slope lines inclined away from a point; resulting from aggradation; or occasionally from erosion; by channelled; often braided; stream flow; or possibly by sheet flow." ;
    skos:notation "FAN" ;
    skos:prefLabel "Fan" ;
    schema:url "https://github.com/ternaustralia/dawe-rlp-vocabs/tree/main/vocab_files/categorical_collections/luts/landform-element.ttl"^^xsd:anyURI ;
.

<https://linked.data.gov.au/def/test/dawe-cv/9e22fdaf-48e4-5172-bb86-95545f600e7d>
    a skos:Concept ;
    dcterms:identifier 30 ;
    dcterms:source <http://vocabs.paratoo.tern.org.au:1337/api/lut-landform-elements> ;
    rdfs:isDefinedBy <https://linked.data.gov.au/def/nrm> ;
    skos:definition "Flat aggraded by human activity." ;
    skos:notation "FIL" ;
    skos:prefLabel "Fil-top" ;
    schema:url "https://github.com/ternaustralia/dawe-rlp-vocabs/tree/main/vocab_files/categorical_collections/luts/landform-element.ttl"^^xsd:anyURI ;
.

<https://linked.data.gov.au/def/test/dawe-cv/a4338ea4-ce49-56df-b773-8c33a9b528b2>
    a skos:Concept ;
    dcterms:identifier 45 ;
    dcterms:source <http://vocabs.paratoo.tern.org.au:1337/api/lut-landform-elements> ;
    rdfs:isDefinedBy <https://linked.data.gov.au/def/nrm> ;
    skos:definition "Level-floored; commonly water-filled closed depression with a nearly circular; steep rim; excavated by volcanism." ;
    skos:notation "MAA" ;
    skos:prefLabel "Maar" ;
    schema:url "https://github.com/ternaustralia/dawe-rlp-vocabs/tree/main/vocab_files/categorical_collections/luts/landform-element.ttl"^^xsd:anyURI ;
.

<https://linked.data.gov.au/def/test/dawe-cv/a7b6a6b8-0b0b-5f51-8706-1ad35851a117>
    a skos:Concept ;
    dcterms:identifier 28 ;
    dcterms:source <http://vocabs.paratoo.tern.org.au:1337/api/lut-landform-elements> ;
    rdfs:isDefinedBy <https://linked.data.gov.au/def/nrm> ;
    skos:definition "Stream channel close to its junction with a sea or lake; where the action of channelled stream flow is modified by tide and waves. The width typically increases downstream." ;
    skos:notation "EST" ;
    skos:prefLabel "Estuary" ;
    schema:url "https://github.com/ternaustralia/dawe-rlp-vocabs/tree/main/vocab_files/categorical_collections/luts/landform-element.ttl"^^xsd:anyURI ;
.

<https://linked.data.gov.au/def/test/dawe-cv/b1887a7f-1df3-5b72-8494-a12009faf955>
    a skos:Concept ;
    dcterms:identifier 71 ;
    dcterms:source <http://vocabs.paratoo.tern.org.au:1337/api/lut-landform-elements> ;
    rdfs:isDefinedBy <https://linked.data.gov.au/def/nrm> ;
    skos:definition "Almost level; closed or almost closed depression with a seasonal or permanent watertable at or above the surface; commonly aggraded by overbank stream flow and sometimes biological (peat) accumulation." ;
    skos:notation "SWP" ;
    skos:prefLabel "Swamp" ;
    schema:url "https://github.com/ternaustralia/dawe-rlp-vocabs/tree/main/vocab_files/categorical_collections/luts/landform-element.ttl"^^xsd:anyURI ;
.

<https://linked.data.gov.au/def/test/dawe-cv/b2139c18-0220-5fce-98d0-4847e17919cc>
    a skos:Concept ;
    dcterms:identifier 61 ;
    dcterms:source <http://vocabs.paratoo.tern.org.au:1337/api/lut-landform-elements> ;
    rdfs:isDefinedBy <https://linked.data.gov.au/def/nrm> ;
    skos:definition "Very wide; steep to precipitous maximal slope eroded by gravlty; water-aided mass movement or sheet flow." ;
    skos:notation "SCA" ;
    skos:prefLabel "Scarp" ;
    schema:url "https://github.com/ternaustralia/dawe-rlp-vocabs/tree/main/vocab_files/categorical_collections/luts/landform-element.ttl"^^xsd:anyURI ;
.

<https://linked.data.gov.au/def/test/dawe-cv/b459407f-82fe-5212-80c0-dfd4e3d49531>
    a skos:Concept ;
    dcterms:identifier 35 ;
    dcterms:source <http://vocabs.paratoo.tern.org.au:1337/api/lut-landform-elements> ;
    rdfs:isDefinedBy <https://linked.data.gov.au/def/nrm> ;
    skos:definition "Very gently inclined to steep crest; smoothly convex; eroded mainly by creep and sheet wash. A typical element of mountains; hills; low hills and rises." ;
    skos:notation "HCR" ;
    skos:prefLabel "Hillcrest" ;
    schema:url "https://github.com/ternaustralia/dawe-rlp-vocabs/tree/main/vocab_files/categorical_collections/luts/landform-element.ttl"^^xsd:anyURI ;
.

<https://linked.data.gov.au/def/test/dawe-cv/b6c1efcd-7bac-5d4d-aca5-f85f5b1e8a8a>
    a skos:Concept ;
    dcterms:identifier 4 ;
    dcterms:source <http://vocabs.paratoo.tern.org.au:1337/api/lut-landform-elements> ;
    rdfs:isDefinedBy <https://linked.data.gov.au/def/nrm> ;
    skos:definition "Elongated; gently to moderately inclined; low ridge built up by channelled stream flow; part of a stream bed." ;
    skos:notation "BAR" ;
    skos:prefLabel "Bar (stream bar)" ;
    schema:url "https://github.com/ternaustralia/dawe-rlp-vocabs/tree/main/vocab_files/categorical_collections/luts/landform-element.ttl"^^xsd:anyURI ;
.

<https://linked.data.gov.au/def/test/dawe-cv/b87ac878-c02d-50ee-b04c-a82bcb3e02d6>
    a skos:Concept ;
    dcterms:identifier 72 ;
    dcterms:source <http://vocabs.paratoo.tern.org.au:1337/api/lut-landform-elements> ;
    rdfs:isDefinedBy <https://linked.data.gov.au/def/nrm> ;
    skos:definition "Moderately inclined or steep waning lower slope; consisting of rock fragments aggraded by gravlty." ;
    skos:notation "TAL" ;
    skos:prefLabel "Talus" ;
    schema:url "https://github.com/ternaustralia/dawe-rlp-vocabs/tree/main/vocab_files/categorical_collections/luts/landform-element.ttl"^^xsd:anyURI ;
.

<https://linked.data.gov.au/def/test/dawe-cv/bbefbe1f-e0b3-5c10-a425-a179638c5d63>
    a skos:Concept ;
    dcterms:identifier 34 ;
    dcterms:source <http://vocabs.paratoo.tern.org.au:1337/api/lut-landform-elements> ;
    rdfs:isDefinedBy <https://linked.data.gov.au/def/nrm> ;
    skos:definition "Open depression with short; precipitous walls and moderately inclined to very gently inclined floor or small stream channel; eroded by channelled stream flow and consequent collapse and water-aided mass movement." ;
    skos:notation "GUL" ;
    skos:prefLabel "Gully" ;
    schema:url "https://github.com/ternaustralia/dawe-rlp-vocabs/tree/main/vocab_files/categorical_collections/luts/landform-element.ttl"^^xsd:anyURI ;
.

<https://linked.data.gov.au/def/test/dawe-cv/be9158a1-5d0c-5558-ab3f-6c7c1e79fb9e>
    a skos:Concept ;
    dcterms:identifier 21 ;
    dcterms:source <http://vocabs.paratoo.tern.org.au:1337/api/lut-landform-elements> ;
    rdfs:isDefinedBy <https://linked.data.gov.au/def/nrm> ;
    skos:definition "Ridge built up by human activity so as to close a depression." ;
    skos:notation "DAM" ;
    skos:prefLabel "Dam" ;
    schema:url "https://github.com/ternaustralia/dawe-rlp-vocabs/tree/main/vocab_files/categorical_collections/luts/landform-element.ttl"^^xsd:anyURI ;
.

<https://linked.data.gov.au/def/test/dawe-cv/bee94ec9-b2b2-5d62-91c3-eb362fcc79e3>
    a skos:Concept ;
    dcterms:identifier 38 ;
    dcterms:source <http://vocabs.paratoo.tern.org.au:1337/api/lut-landform-elements> ;
    rdfs:isDefinedBy <https://linked.data.gov.au/def/nrm> ;
    skos:definition "See Tidal flat." ;
    skos:notation "ITF" ;
    skos:prefLabel "Intertidal flat" ;
    schema:url "https://github.com/ternaustralia/dawe-rlp-vocabs/tree/main/vocab_files/categorical_collections/luts/landform-element.ttl"^^xsd:anyURI ;
.

<https://linked.data.gov.au/def/test/dawe-cv/bf8d1824-2df8-59c8-b2e8-eadecb0ef4d2>
    a skos:Concept ;
    dcterms:identifier 66 ;
    dcterms:source <http://vocabs.paratoo.tern.org.au:1337/api/lut-landform-elements> ;
    rdfs:isDefinedBy <https://linked.data.gov.au/def/nrm> ;
    skos:definition "Linear; generally sinuous open depression forming the bottom of a stream channel; eroded and locally excavated; aggraded or built up by channelled stream flow. Parts that are built up include bars." ;
    skos:notation "STB" ;
    skos:prefLabel "Stream bed" ;
    schema:url "https://github.com/ternaustralia/dawe-rlp-vocabs/tree/main/vocab_files/categorical_collections/luts/landform-element.ttl"^^xsd:anyURI ;
.

<https://linked.data.gov.au/def/test/dawe-cv/c1931b42-0124-51c1-9798-fb1488c9d84e>
    a skos:Concept ;
    dcterms:identifier 41 ;
    dcterms:source <http://vocabs.paratoo.tern.org.au:1337/api/lut-landform-elements> ;
    rdfs:isDefinedBy <https://linked.data.gov.au/def/nrm> ;
    skos:definition "Moderately inclined to very steep slope; eroded in the upper part and aggraded in the lower part by water-aided mass movement; characterised by irregular hummocks." ;
    skos:notation "LDS" ;
    skos:prefLabel "Landslide" ;
    schema:url "https://github.com/ternaustralia/dawe-rlp-vocabs/tree/main/vocab_files/categorical_collections/luts/landform-element.ttl"^^xsd:anyURI ;
.

<https://linked.data.gov.au/def/test/dawe-cv/d024e54c-13e3-5a3c-8617-daa69b0274c7>
    a skos:Concept ;
    dcterms:identifier 79 ;
    dcterms:source <http://vocabs.paratoo.tern.org.au:1337/api/lut-landform-elements> ;
    rdfs:isDefinedBy <https://linked.data.gov.au/def/nrm> ;
    skos:definition "Hillock heaved up by volcanism (or; elsewhere; built up by human activity at a burial site)." ;
    skos:notation "TUM" ;
    skos:prefLabel "Tumulus" ;
    schema:url "https://github.com/ternaustralia/dawe-rlp-vocabs/tree/main/vocab_files/categorical_collections/luts/landform-element.ttl"^^xsd:anyURI ;
.

<https://linked.data.gov.au/def/test/dawe-cv/d1732611-cc2f-5e6f-846a-da0adc40a439>
    a skos:Concept ;
    dcterms:identifier 19 ;
    dcterms:source <http://vocabs.paratoo.tern.org.au:1337/api/lut-landform-elements> ;
    rdfs:isDefinedBy <https://linked.data.gov.au/def/nrm> ;
    skos:definition "Slope eroded by human activity." ;
    skos:notation "CUT" ;
    skos:prefLabel "Cut face" ;
    schema:url "https://github.com/ternaustralia/dawe-rlp-vocabs/tree/main/vocab_files/categorical_collections/luts/landform-element.ttl"^^xsd:anyURI ;
.

<https://linked.data.gov.au/def/test/dawe-cv/d632f875-823d-5fd3-bc6e-9741e735fe4a>
    a skos:Concept ;
    dcterms:identifier 60 ;
    dcterms:source <http://vocabs.paratoo.tern.org.au:1337/api/lut-landform-elements> ;
    rdfs:isDefinedBy <https://linked.data.gov.au/def/nrm> ;
    skos:definition "Flat; bare of vegetatiorn; from which soil has been eroded or excavated by surface wash or wind." ;
    skos:notation "SCD" ;
    skos:prefLabel "Scald" ;
    schema:url "https://github.com/ternaustralia/dawe-rlp-vocabs/tree/main/vocab_files/categorical_collections/luts/landform-element.ttl"^^xsd:anyURI ;
.

<https://linked.data.gov.au/def/test/dawe-cv/d7481c8e-dcec-5415-b212-df2326a60bbd>
    a skos:Concept ;
    dcterms:identifier 12 ;
    dcterms:source <http://vocabs.paratoo.tern.org.au:1337/api/lut-landform-elements> ;
    rdfs:isDefinedBy <https://linked.data.gov.au/def/nrm> ;
    skos:definition "Flat at the margin of a stream channel aggraded and partly eroded by overbank and channelled stream flow; an incipient flood plain. Channel benches have been referred to as 'low terraces'; but the term 'terrace' should be restricted to landform patterns above the influence of active stream flow." ;
    skos:notation "CBE" ;
    skos:prefLabel "Channel bench" ;
    schema:url "https://github.com/ternaustralia/dawe-rlp-vocabs/tree/main/vocab_files/categorical_collections/luts/landform-element.ttl"^^xsd:anyURI ;
.

<https://linked.data.gov.au/def/test/dawe-cv/d7b593d8-badc-562c-940b-352881cbb942>
    a skos:Concept ;
    dcterms:identifier 32 ;
    dcterms:source <http://vocabs.paratoo.tern.org.au:1337/api/lut-landform-elements> ;
    rdfs:isDefinedBy <https://linked.data.gov.au/def/nrm> ;
    skos:definition "Moderately to very gently inclined waning lower slope resulting from aggradation or erosion by sheet flow; earth flow or creep." ;
    skos:notation "FOO" ;
    skos:prefLabel "Footslope" ;
    schema:url "https://github.com/ternaustralia/dawe-rlp-vocabs/tree/main/vocab_files/categorical_collections/luts/landform-element.ttl"^^xsd:anyURI ;
.

<https://linked.data.gov.au/def/test/dawe-cv/d8c0b7fa-90ad-583d-b0d3-61046094cbb6>
    a skos:Concept ;
    dcterms:identifier 25 ;
    dcterms:source <http://vocabs.paratoo.tern.org.au:1337/api/lut-landform-elements> ;
    rdfs:isDefinedBy <https://linked.data.gov.au/def/nrm> ;
    skos:definition "Crest built up or eroded by the wind (see Dune)." ;
    skos:notation "DUC" ;
    skos:prefLabel "Dune crest" ;
    schema:url "https://github.com/ternaustralia/dawe-rlp-vocabs/tree/main/vocab_files/categorical_collections/luts/landform-element.ttl"^^xsd:anyURI ;
.

<https://linked.data.gov.au/def/test/dawe-cv/dc1f22f5-76c7-512d-86a2-095d911d3829>
    a skos:Concept ;
    dcterms:identifier 40 ;
    dcterms:source <http://vocabs.paratoo.tern.org.au:1337/api/lut-landform-elements> ;
    rdfs:isDefinedBy <https://linked.data.gov.au/def/nrm> ;
    skos:definition "Large; water-filled closed depression." ;
    skos:notation "LAK" ;
    skos:prefLabel "Lake" ;
    schema:url "https://github.com/ternaustralia/dawe-rlp-vocabs/tree/main/vocab_files/categorical_collections/luts/landform-element.ttl"^^xsd:anyURI ;
.

<https://linked.data.gov.au/def/test/dawe-cv/df10c1e5-8fa4-5e36-8357-6fb9d2bd5c75>
    a skos:Concept ;
    dcterms:identifier 58 ;
    dcterms:source <http://vocabs.paratoo.tern.org.au:1337/api/lut-landform-elements> ;
    rdfs:isDefinedBy <https://linked.data.gov.au/def/nrm> ;
    skos:definition "Flat of bare consolidated rock; usually eroded by sheet wash." ;
    skos:notation "RFL" ;
    skos:prefLabel "Rock flat" ;
    schema:url "https://github.com/ternaustralia/dawe-rlp-vocabs/tree/main/vocab_files/categorical_collections/luts/landform-element.ttl"^^xsd:anyURI ;
.

<https://linked.data.gov.au/def/test/dawe-cv/e614b305-192b-5122-8702-bd3b0583f644>
    a skos:Concept ;
    dcterms:identifier 49 ;
    dcterms:source <http://vocabs.paratoo.tern.org.au:1337/api/lut-landform-elements> ;
    rdfs:isDefinedBy <https://linked.data.gov.au/def/nrm> ;
    skos:definition "Large; gently inclined to level (<1%) waning lower slope; with slope lines inclined in a single direction; or somewhat convergent or divergent; eroded or sometimes slightly aggraded by sheet flow. It is underlain by bedrock." ;
    skos:notation "PED" ;
    skos:prefLabel "Pediment" ;
    schema:url "https://github.com/ternaustralia/dawe-rlp-vocabs/tree/main/vocab_files/categorical_collections/luts/landform-element.ttl"^^xsd:anyURI ;
.

<https://linked.data.gov.au/def/test/dawe-cv/ede972cc-963e-57f3-b594-ed4a137ed9dc>
    a skos:Concept ;
    dcterms:identifier 62 ;
    dcterms:source <http://vocabs.paratoo.tern.org.au:1337/api/lut-landform-elements> ;
    rdfs:isDefinedBy <https://linked.data.gov.au/def/nrm> ;
    skos:definition "Waning or minimal slope situated below a scarp; with its contours generally parallel to the line of the scarp." ;
    skos:notation "SFS" ;
    skos:prefLabel "Scarp-footslope" ;
    schema:url "https://github.com/ternaustralia/dawe-rlp-vocabs/tree/main/vocab_files/categorical_collections/luts/landform-element.ttl"^^xsd:anyURI ;
.

<https://linked.data.gov.au/def/test/dawe-cv/ef20c946-0016-56a6-b198-50d7fc809686>
    a skos:Concept ;
    dcterms:identifier 36 ;
    dcterms:source <http://vocabs.paratoo.tern.org.au:1337/api/lut-landform-elements> ;
    rdfs:isDefinedBy <https://linked.data.gov.au/def/nrm> ;
    skos:definition "Gently inclined to precipitous slope; commonly simple and maximal; eroded by sheet wash; creep or water-aided mass movement. A typical element of mountains; hills; low hills and rises." ;
    skos:notation "HSL" ;
    skos:prefLabel "Hillslope" ;
    schema:url "https://github.com/ternaustralia/dawe-rlp-vocabs/tree/main/vocab_files/categorical_collections/luts/landform-element.ttl"^^xsd:anyURI ;
.

<https://linked.data.gov.au/def/test/dawe-cv/f29ebd25-4eb7-5619-b8d1-ddd4a1c1214a>
    a skos:Concept ;
    dcterms:identifier 1 ;
    dcterms:source <http://vocabs.paratoo.tern.org.au:1337/api/lut-landform-elements> ;
    rdfs:isDefinedBy <https://linked.data.gov.au/def/nrm> ;
    skos:definition "Moderately inclined to very steep; short open depression with concave cross-section; eroded by collapse; landslides; creep or surface wash." ;
    skos:notation "ALC" ;
    skos:prefLabel "Alcove" ;
    schema:url "https://github.com/ternaustralia/dawe-rlp-vocabs/tree/main/vocab_files/categorical_collections/luts/landform-element.ttl"^^xsd:anyURI ;
.

<https://linked.data.gov.au/def/test/dawe-cv/f29fe987-89e1-597f-881d-1b89ff446c18>
    a skos:Concept ;
    dcterms:identifier 39 ;
    dcterms:source <http://vocabs.paratoo.tern.org.au:1337/api/lut-landform-elements> ;
    rdfs:isDefinedBy <https://linked.data.gov.au/def/nrm> ;
    skos:definition "Closed depression filled with water that is typically salt or brackish; bounded at least in part by forms aggraded or built up by waves or reef-building organisms." ;
    skos:notation "LAG" ;
    skos:prefLabel "Lagoon" ;
    schema:url "https://github.com/ternaustralia/dawe-rlp-vocabs/tree/main/vocab_files/categorical_collections/luts/landform-element.ttl"^^xsd:anyURI ;
.

<https://linked.data.gov.au/def/test/dawe-cv/f5ee0c0a-6a38-539e-9288-b5b3a5606e27>
    a skos:Concept ;
    dcterms:identifier 11 ;
    dcterms:source <http://vocabs.paratoo.tern.org.au:1337/api/lut-landform-elements> ;
    rdfs:isDefinedBy <https://linked.data.gov.au/def/nrm> ;
    skos:definition "Steep maximal mid-slope or upper slope; generally comprising both a very short scarp (free face) that is often bare rockland; and a stony scarp-footslope (debris slope); often standing above a pediment" ;
    skos:notation "BRK" ;
    skos:prefLabel "Breakaway" ;
    schema:url "https://github.com/ternaustralia/dawe-rlp-vocabs/tree/main/vocab_files/categorical_collections/luts/landform-element.ttl"^^xsd:anyURI ;
.

<https://linked.data.gov.au/def/test/dawe-cv/f6f2e07c-dda2-5abd-8a22-2a2ff2e8521a>
    a skos:Concept ;
    dcterms:identifier 27 ;
    dcterms:source <http://vocabs.paratoo.tern.org.au:1337/api/lut-landform-elements> ;
    rdfs:isDefinedBy <https://linked.data.gov.au/def/nrm> ;
    skos:definition "Ridge or slope built up by human activity." ;
    skos:notation "EMB" ;
    skos:prefLabel "Embankment" ;
    schema:url "https://github.com/ternaustralia/dawe-rlp-vocabs/tree/main/vocab_files/categorical_collections/luts/landform-element.ttl"^^xsd:anyURI ;
.

<https://linked.data.gov.au/def/test/dawe-cv/f8726949-6dff-53cd-8b52-996a50eac071>
    a skos:Concept ;
    dcterms:identifier 24 ;
    dcterms:source <http://vocabs.paratoo.tern.org.au:1337/api/lut-landform-elements> ;
    rdfs:isDefinedBy <https://linked.data.gov.au/def/nrm> ;
    skos:definition "Moderately inclined to very steep ridge or hillock built up by the wind. This element may comprise dunecrest and duneslope." ;
    skos:notation "DUN" ;
    skos:prefLabel "Dune" ;
    schema:url "https://github.com/ternaustralia/dawe-rlp-vocabs/tree/main/vocab_files/categorical_collections/luts/landform-element.ttl"^^xsd:anyURI ;
.

