# Do not edit this file directly. This file is generated by `make luts` with endpoints from src/dawe_nrm/api/categorical_values/endpoints.py
PREFIX dcterms: <http://purl.org/dc/terms/>
PREFIX rdfs: <http://www.w3.org/2000/01/rdf-schema#>
PREFIX schema: <https://schema.org/>
PREFIX skos: <http://www.w3.org/2004/02/skos/core#>
PREFIX urnc: <urn:class:>
PREFIX urnp: <urn:property:>
PREFIX xsd: <http://www.w3.org/2001/XMLSchema#>

<https://linked.data.gov.au/def/nrm/40d8bc62-466c-5de3-bf7d-52f425580694>
    a urnc:CategoricalConceptMeta ;
    schema:url "https://github.com/ternaustralia/dawe-rlp-vocabs/tree/main/vocab_files/categorical_collections/luts/soils-confidence-levels.ttl"^^xsd:anyURI ;
    urnp:categoricalCollection <https://linked.data.gov.au/def/nrm/7bd6fc9b-2e65-4cdd-acda-8cab19f2cefe> ;
    urnp:categoricalConcept <https://linked.data.gov.au/def/nrm/334b6b31-12a2-5bfc-bf4f-870c0954b343> ;
    urnp:conceptDefinition "Necessary analytical and/or morphological data for the profile are incomplete but are sufficient to classify the soil with a reasonable degree of confidence." ;
    urnp:conceptIdentifier 2 ;
    urnp:conceptNotation "2" ;
    urnp:conceptSource <https://core.vocabs.paratoo.tern.org.au/api/lut-soils-confidence-levels> ;
.

<https://linked.data.gov.au/def/nrm/4cc5ac2a-5fcd-5a9c-b8d5-9c9af994e59e>
    a urnc:CategoricalConceptMeta ;
    schema:url "https://github.com/ternaustralia/dawe-rlp-vocabs/tree/main/vocab_files/categorical_collections/luts/soils-confidence-levels.ttl"^^xsd:anyURI ;
    urnp:categoricalCollection <https://linked.data.gov.au/def/nrm/7bd6fc9b-2e65-4cdd-acda-8cab19f2cefe> ;
    urnp:categoricalConcept <https://linked.data.gov.au/def/nrm/ff6c5a08-b2fa-56b6-ac00-6830f4074b6a> ;
    urnp:conceptDefinition "No necessary analytical or limited morphological data are available for the profile and the classifier has little knowledge or experience with this kind of soil, hence the classification is provisional." ;
    urnp:conceptIdentifier 4 ;
    urnp:conceptNotation "4" ;
    urnp:conceptSource <https://core.vocabs.paratoo.tern.org.au/api/lut-soils-confidence-levels> ;
.

<https://linked.data.gov.au/def/nrm/5a2b7b22-b263-59dd-922e-71e0cf882135>
    a urnc:CategoricalConceptMeta ;
    schema:url "https://github.com/ternaustralia/dawe-rlp-vocabs/tree/main/vocab_files/categorical_collections/luts/soils-confidence-levels.ttl"^^xsd:anyURI ;
    urnp:categoricalCollection <https://linked.data.gov.au/def/nrm/7bd6fc9b-2e65-4cdd-acda-8cab19f2cefe> ;
    urnp:categoricalConcept <https://linked.data.gov.au/def/nrm/c093c7f6-6edf-595e-9539-70de788efbaa> ;
    urnp:conceptDefinition "No necessary analytical or limited morphological data are available for the profile but confidence is fair, based on knowledge of similar soils in similar environments." ;
    urnp:conceptIdentifier 3 ;
    urnp:conceptNotation "3" ;
    urnp:conceptSource <https://core.vocabs.paratoo.tern.org.au/api/lut-soils-confidence-levels> ;
.

<https://linked.data.gov.au/def/nrm/fe6067f3-a3cc-57e0-93aa-07fd49c875c8>
    a urnc:CategoricalConceptMeta ;
    schema:url "https://github.com/ternaustralia/dawe-rlp-vocabs/tree/main/vocab_files/categorical_collections/luts/soils-confidence-levels.ttl"^^xsd:anyURI ;
    urnp:categoricalCollection <https://linked.data.gov.au/def/nrm/7bd6fc9b-2e65-4cdd-acda-8cab19f2cefe> ;
    urnp:categoricalConcept <https://linked.data.gov.au/def/nrm/b80c8fef-a677-5340-85fb-2c162d75df03> ;
    urnp:conceptDefinition "All necessary analytical and/or morphological data are available for the profile being classified." ;
    urnp:conceptIdentifier 1 ;
    urnp:conceptNotation "1" ;
    urnp:conceptSource <https://core.vocabs.paratoo.tern.org.au/api/lut-soils-confidence-levels> ;
.

<https://linked.data.gov.au/def/nrm/334b6b31-12a2-5bfc-bf4f-870c0954b343>
    a skos:Concept ;
    dcterms:identifier 2 ;
    dcterms:source <https://core.vocabs.paratoo.tern.org.au/api/lut-soils-confidence-levels> ;
    rdfs:isDefinedBy <https://linked.data.gov.au/def/nrm> ;
    skos:definition "Necessary analytical and/or morphological data for the profile are incomplete but are sufficient to classify the soil with a reasonable degree of confidence." ;
    skos:notation "2" ;
    skos:prefLabel "2" ;
    schema:url "https://github.com/ternaustralia/dawe-rlp-vocabs/tree/main/vocab_files/categorical_collections/luts/soils-confidence-levels.ttl"^^xsd:anyURI ;
.

<https://linked.data.gov.au/def/nrm/b80c8fef-a677-5340-85fb-2c162d75df03>
    a skos:Concept ;
    dcterms:identifier 1 ;
    dcterms:source <https://core.vocabs.paratoo.tern.org.au/api/lut-soils-confidence-levels> ;
    rdfs:isDefinedBy <https://linked.data.gov.au/def/nrm> ;
    skos:definition "All necessary analytical and/or morphological data are available for the profile being classified." ;
    skos:notation "1" ;
    skos:prefLabel "1" ;
    schema:url "https://github.com/ternaustralia/dawe-rlp-vocabs/tree/main/vocab_files/categorical_collections/luts/soils-confidence-levels.ttl"^^xsd:anyURI ;
.

<https://linked.data.gov.au/def/nrm/c093c7f6-6edf-595e-9539-70de788efbaa>
    a skos:Concept ;
    dcterms:identifier 3 ;
    dcterms:source <https://core.vocabs.paratoo.tern.org.au/api/lut-soils-confidence-levels> ;
    rdfs:isDefinedBy <https://linked.data.gov.au/def/nrm> ;
    skos:definition "No necessary analytical or limited morphological data are available for the profile but confidence is fair, based on knowledge of similar soils in similar environments." ;
    skos:notation "3" ;
    skos:prefLabel "3" ;
    schema:url "https://github.com/ternaustralia/dawe-rlp-vocabs/tree/main/vocab_files/categorical_collections/luts/soils-confidence-levels.ttl"^^xsd:anyURI ;
.

<https://linked.data.gov.au/def/nrm/ff6c5a08-b2fa-56b6-ac00-6830f4074b6a>
    a skos:Concept ;
    dcterms:identifier 4 ;
    dcterms:source <https://core.vocabs.paratoo.tern.org.au/api/lut-soils-confidence-levels> ;
    rdfs:isDefinedBy <https://linked.data.gov.au/def/nrm> ;
    skos:definition "No necessary analytical or limited morphological data are available for the profile and the classifier has little knowledge or experience with this kind of soil, hence the classification is provisional." ;
    skos:notation "4" ;
    skos:prefLabel "4" ;
    schema:url "https://github.com/ternaustralia/dawe-rlp-vocabs/tree/main/vocab_files/categorical_collections/luts/soils-confidence-levels.ttl"^^xsd:anyURI ;
.

<https://linked.data.gov.au/def/nrm/7bd6fc9b-2e65-4cdd-acda-8cab19f2cefe>
    a skos:Collection ;
    dcterms:description "A collection of soils confidence levels and its codes." ;
    dcterms:source <https://core.vocabs.paratoo.tern.org.au/api/lut-soils-confidence-levels> ;
    rdfs:isDefinedBy <https://linked.data.gov.au/def/nrm> ;
    skos:member
        <https://linked.data.gov.au/def/nrm/334b6b31-12a2-5bfc-bf4f-870c0954b343> ,
        <https://linked.data.gov.au/def/nrm/b80c8fef-a677-5340-85fb-2c162d75df03> ,
        <https://linked.data.gov.au/def/nrm/c093c7f6-6edf-595e-9539-70de788efbaa> ,
        <https://linked.data.gov.au/def/nrm/ff6c5a08-b2fa-56b6-ac00-6830f4074b6a> ;
    skos:prefLabel "Soils confidence levels codes" ;
    schema:url "https://github.com/ternaustralia/dawe-rlp-vocabs/tree/main/vocab_files/categorical_collections/luts/soils-confidence-levels.ttl"^^xsd:anyURI ;
.

