# Do not edit this file directly. This file is generated by `make luts` with endpoints from src/dawe_nrm/api/categorical_values/endpoints.py
PREFIX dcterms: <http://purl.org/dc/terms/>
PREFIX rdfs: <http://www.w3.org/2000/01/rdf-schema#>
PREFIX schema: <https://schema.org/>
PREFIX skos: <http://www.w3.org/2004/02/skos/core#>
PREFIX xsd: <http://www.w3.org/2001/XMLSchema#>

<https://linked.data.gov.au/def/test/dawe-cv/457faa4f-74e8-4b8a-9e4b-541bb7c50441>
    a skos:Collection ;
    dcterms:description "A collection of soils microrelief types and its codes." ;
    dcterms:source <http://vocabs.paratoo.tern.org.au:1337/api/lut-soils-microrelief-types> ;
    rdfs:isDefinedBy <https://linked.data.gov.au/def/nrm> ;
    skos:member
        <https://linked.data.gov.au/def/test/dawe-cv/1652b8df-f21d-55c2-bd0d-9cd6014fe01d> ,
        <https://linked.data.gov.au/def/test/dawe-cv/32856323-668d-58ed-b4ff-ff5e35e5f2d4> ,
        <https://linked.data.gov.au/def/test/dawe-cv/46ab5b7b-0c5e-5e59-868d-355e8f38d74d> ,
        <https://linked.data.gov.au/def/test/dawe-cv/573b16d1-aa69-5707-8449-fecd540facae> ,
        <https://linked.data.gov.au/def/test/dawe-cv/5ace7c87-8130-5208-9356-94b0699b34a5> ,
        <https://linked.data.gov.au/def/test/dawe-cv/6adae5c9-17eb-5809-b089-3a02778f0bb2> ,
        <https://linked.data.gov.au/def/test/dawe-cv/6ec7f9f8-b467-59ff-876e-1f6bb4d5444f> ,
        <https://linked.data.gov.au/def/test/dawe-cv/8c5506a1-f661-521c-97ce-438d032be97f> ,
        <https://linked.data.gov.au/def/test/dawe-cv/9d791a95-eeaa-5650-b7a0-82bae8d5120e> ,
        <https://linked.data.gov.au/def/test/dawe-cv/9f400fbf-84c2-5be9-a69f-bc293cf23a67> ,
        <https://linked.data.gov.au/def/test/dawe-cv/a5ad416b-30ee-53d4-af0b-1166c1e13110> ,
        <https://linked.data.gov.au/def/test/dawe-cv/a848bd11-d330-500d-8cfe-80a44a871d00> ,
        <https://linked.data.gov.au/def/test/dawe-cv/a8bf19d8-dc8c-5bfa-9198-100444fb9c6a> ,
        <https://linked.data.gov.au/def/test/dawe-cv/abc10ed6-bc34-5188-80b9-4c8767740609> ,
        <https://linked.data.gov.au/def/test/dawe-cv/ba6428ab-7e7d-54f4-8a1c-c97749febddb> ,
        <https://linked.data.gov.au/def/test/dawe-cv/bb7102b7-aaec-54c9-bc85-bc9d5dc1b2c4> ,
        <https://linked.data.gov.au/def/test/dawe-cv/dd620811-2995-57da-88a0-e113212b07d1> ,
        <https://linked.data.gov.au/def/test/dawe-cv/deba9223-29d2-5330-a5a8-a7667a4520aa> ,
        <https://linked.data.gov.au/def/test/dawe-cv/ee59db14-2399-51cd-bfd0-6746f12f02de> ;
    skos:prefLabel "Soils microrelief types codes" ;
    schema:url "https://github.com/ternaustralia/dawe-rlp-vocabs/tree/main/vocab_files/categorical_collections/luts/soils-microrelief-types.ttl"^^xsd:anyURI ;
.

<https://linked.data.gov.au/def/test/dawe-cv/1652b8df-f21d-55c2-bd0d-9cd6014fe01d>
    a skos:Concept ;
    dcterms:identifier 10 ;
    dcterms:source <http://vocabs.paratoo.tern.org.au:1337/api/lut-soils-microrelief-types> ;
    rdfs:isDefinedBy <https://linked.data.gov.au/def/nrm> ;
    skos:definition "" ;
    skos:notation "B" ;
    skos:prefLabel "Biotic" ;
    schema:url "https://github.com/ternaustralia/dawe-rlp-vocabs/tree/main/vocab_files/categorical_collections/luts/soils-microrelief-types.ttl"^^xsd:anyURI ;
.

<https://linked.data.gov.au/def/test/dawe-cv/32856323-668d-58ed-b4ff-ff5e35e5f2d4>
    a skos:Concept ;
    dcterms:identifier 1 ;
    dcterms:source <http://vocabs.paratoo.tern.org.au:1337/api/lut-soils-microrelief-types> ;
    rdfs:isDefinedBy <https://linked.data.gov.au/def/nrm> ;
    skos:definition "" ;
    skos:notation "Z" ;
    skos:prefLabel "Zero or no microrelief" ;
    schema:url "https://github.com/ternaustralia/dawe-rlp-vocabs/tree/main/vocab_files/categorical_collections/luts/soils-microrelief-types.ttl"^^xsd:anyURI ;
.

<https://linked.data.gov.au/def/test/dawe-cv/46ab5b7b-0c5e-5e59-868d-355e8f38d74d>
    a skos:Concept ;
    dcterms:identifier 16 ;
    dcterms:source <http://vocabs.paratoo.tern.org.au:1337/api/lut-soils-microrelief-types> ;
    rdfs:isDefinedBy <https://linked.data.gov.au/def/nrm> ;
    skos:definition "Trenches typically 0.2 m deep and 0.6 m wide; with near vertical walls; alternating with flat-crested ridges about 1.3 m wide; which extend along the contour for several metres or tens of metres. Contour trenches are known in areas in south-eastern Australia above 350 m altitude with a high effective rainfall; where they are associated with a grassland or heathland vegetation on undulating rises." ;
    skos:notation "T" ;
    skos:prefLabel "Contour trench" ;
    schema:url "https://github.com/ternaustralia/dawe-rlp-vocabs/tree/main/vocab_files/categorical_collections/luts/soils-microrelief-types.ttl"^^xsd:anyURI ;
.

<https://linked.data.gov.au/def/test/dawe-cv/573b16d1-aa69-5707-8449-fecd540facae>
    a skos:Concept ;
    dcterms:identifier 12 ;
    dcterms:source <http://vocabs.paratoo.tern.org.au:1337/api/lut-soils-microrelief-types> ;
    rdfs:isDefinedBy <https://linked.data.gov.au/def/nrm> ;
    skos:definition "Depressions in limestone country." ;
    skos:notation "K" ;
    skos:prefLabel "Karst microrelief" ;
    schema:url "https://github.com/ternaustralia/dawe-rlp-vocabs/tree/main/vocab_files/categorical_collections/luts/soils-microrelief-types.ttl"^^xsd:anyURI ;
.

<https://linked.data.gov.au/def/test/dawe-cv/5ace7c87-8130-5208-9356-94b0699b34a5>
    a skos:Concept ;
    dcterms:identifier 8 ;
    dcterms:source <http://vocabs.paratoo.tern.org.au:1337/api/lut-soils-microrelief-types> ;
    rdfs:isDefinedBy <https://linked.data.gov.au/def/nrm> ;
    skos:definition "Small hummocks rising above planar surface. They vary from rounded; both planar and vertically; to flat-topped; relatively steep sided and elongate. They are usually closely and regularly spaced; ranging from 0.06 m to 0.6 m in both vertical and horizontal dimensions. They are common in northern Australia on soils with impeded internal drainage and in areas of short seasonal ponding. Many observers consider them to be formed by biological activity." ;
    skos:notation "D" ;
    skos:prefLabel "Debil-debil" ;
    schema:url "https://github.com/ternaustralia/dawe-rlp-vocabs/tree/main/vocab_files/categorical_collections/luts/soils-microrelief-types.ttl"^^xsd:anyURI ;
.

<https://linked.data.gov.au/def/test/dawe-cv/6adae5c9-17eb-5809-b089-3a02778f0bb2>
    a skos:Concept ;
    dcterms:identifier 13 ;
    dcterms:source <http://vocabs.paratoo.tern.org.au:1337/api/lut-soils-microrelief-types> ;
    rdfs:isDefinedBy <https://linked.data.gov.au/def/nrm> ;
    skos:definition "Closed depression with vertical or funnel-shaped sides." ;
    skos:notation "I" ;
    skos:prefLabel "Sinkhole" ;
    schema:url "https://github.com/ternaustralia/dawe-rlp-vocabs/tree/main/vocab_files/categorical_collections/luts/soils-microrelief-types.ttl"^^xsd:anyURI ;
.

<https://linked.data.gov.au/def/test/dawe-cv/6ec7f9f8-b467-59ff-876e-1f6bb4d5444f>
    a skos:Concept ;
    dcterms:identifier 3 ;
    dcterms:source <http://vocabs.paratoo.tern.org.au:1337/api/lut-soils-microrelief-types> ;
    rdfs:isDefinedBy <https://linked.data.gov.au/def/nrm> ;
    skos:definition "Irregularly distributed; small mounds and subcircular depressions varying in size and spacing. Vertical interval usually less than 0.3 m. Horizontal interval usually 3-20 m; surface almost level." ;
    skos:notation "N" ;
    skos:prefLabel "Normal gilgai" ;
    schema:url "https://github.com/ternaustralia/dawe-rlp-vocabs/tree/main/vocab_files/categorical_collections/luts/soils-microrelief-types.ttl"^^xsd:anyURI ;
.

<https://linked.data.gov.au/def/test/dawe-cv/8c5506a1-f661-521c-97ce-438d032be97f>
    a skos:Concept ;
    dcterms:identifier 5 ;
    dcterms:source <http://vocabs.paratoo.tern.org.au:1337/api/lut-soils-microrelief-types> ;
    rdfs:isDefinedBy <https://linked.data.gov.au/def/nrm> ;
    skos:definition "Discontinuous; elongate mounds and/or elongate depressions more or less at right angles to the contour. Usually in sloping lands; commonly between linear gilgai on lower slopes and plains." ;
    skos:notation "A" ;
    skos:prefLabel "Lattice gilgai" ;
    schema:url "https://github.com/ternaustralia/dawe-rlp-vocabs/tree/main/vocab_files/categorical_collections/luts/soils-microrelief-types.ttl"^^xsd:anyURI ;
.

<https://linked.data.gov.au/def/test/dawe-cv/9d791a95-eeaa-5650-b7a0-82bae8d5120e>
    a skos:Concept ;
    dcterms:identifier 11 ;
    dcterms:source <http://vocabs.paratoo.tern.org.au:1337/api/lut-soils-microrelief-types> ;
    rdfs:isDefinedBy <https://linked.data.gov.au/def/nrm> ;
    skos:definition "Undifferentiated; irregularly distributed or isolated mounds and/or depressions set in a planar surface." ;
    skos:notation "U" ;
    skos:prefLabel "Mound/depression" ;
    schema:url "https://github.com/ternaustralia/dawe-rlp-vocabs/tree/main/vocab_files/categorical_collections/luts/soils-microrelief-types.ttl"^^xsd:anyURI ;
.

<https://linked.data.gov.au/def/test/dawe-cv/9f400fbf-84c2-5be9-a69f-bc293cf23a67>
    a skos:Concept ;
    dcterms:identifier 6 ;
    dcterms:source <http://vocabs.paratoo.tern.org.au:1337/api/lut-soils-microrelief-types> ;
    rdfs:isDefinedBy <https://linked.data.gov.au/def/nrm> ;
    skos:definition "Irregularly distributed; large depressions; usually greater than 3 m in diameter or greatest dimension; subcircular or irregular and varying from closely spaced in a network of elongate mounds to isolated depressions set in an undulating shelf with occasional small mounds. Some depressions may also contain sinkholes of gilgai usually greater than 0.3 m; horizontal interval usually 5-6 m; surface almost level." ;
    skos:notation "M" ;
    skos:prefLabel "Melonhole gilgai" ;
    schema:url "https://github.com/ternaustralia/dawe-rlp-vocabs/tree/main/vocab_files/categorical_collections/luts/soils-microrelief-types.ttl"^^xsd:anyURI ;
.

<https://linked.data.gov.au/def/test/dawe-cv/a5ad416b-30ee-53d4-af0b-1166c1e13110>
    a skos:Concept ;
    dcterms:identifier 4 ;
    dcterms:source <http://vocabs.paratoo.tern.org.au:1337/api/lut-soils-microrelief-types> ;
    rdfs:isDefinedBy <https://linked.data.gov.au/def/nrm> ;
    skos:definition "Long; narrow; parallel; elongate mounds and broader elongate depressions more or less at right angles to the contour. Usually in sloping lands. Vertical interval usually less than 0.3 m; Horizontal interval usually 5-8 m." ;
    skos:notation "L" ;
    skos:prefLabel "Linear gilgai" ;
    schema:url "https://github.com/ternaustralia/dawe-rlp-vocabs/tree/main/vocab_files/categorical_collections/luts/soils-microrelief-types.ttl"^^xsd:anyURI ;
.

<https://linked.data.gov.au/def/test/dawe-cv/a848bd11-d330-500d-8cfe-80a44a871d00>
    a skos:Concept ;
    dcterms:identifier 14 ;
    dcterms:source <http://vocabs.paratoo.tern.org.au:1337/api/lut-soils-microrelief-types> ;
    rdfs:isDefinedBy <https://linked.data.gov.au/def/nrm> ;
    skos:definition "Hummocky microrelief on the surface of landslides; slumps; earth flows; debris avalanches." ;
    skos:notation "S" ;
    skos:prefLabel "Mass movement" ;
    schema:url "https://github.com/ternaustralia/dawe-rlp-vocabs/tree/main/vocab_files/categorical_collections/luts/soils-microrelief-types.ttl"^^xsd:anyURI ;
.

<https://linked.data.gov.au/def/test/dawe-cv/a8bf19d8-dc8c-5bfa-9198-100444fb9c6a>
    a skos:Concept ;
    dcterms:identifier 17 ;
    dcterms:source <http://vocabs.paratoo.tern.org.au:1337/api/lut-soils-microrelief-types> ;
    rdfs:isDefinedBy <https://linked.data.gov.au/def/nrm> ;
    skos:definition "Mound associated with water flowing from rock or soil without human intervention." ;
    skos:notation "P" ;
    skos:prefLabel "Spring mound" ;
    schema:url "https://github.com/ternaustralia/dawe-rlp-vocabs/tree/main/vocab_files/categorical_collections/luts/soils-microrelief-types.ttl"^^xsd:anyURI ;
.

<https://linked.data.gov.au/def/test/dawe-cv/abc10ed6-bc34-5188-80b9-4c8767740609>
    a skos:Concept ;
    dcterms:identifier 15 ;
    dcterms:source <http://vocabs.paratoo.tern.org.au:1337/api/lut-soils-microrelief-types> ;
    rdfs:isDefinedBy <https://linked.data.gov.au/def/nrm> ;
    skos:definition "Small terraces on slopes resulting either from soil creep or trampling by hoofed animals." ;
    skos:notation "R" ;
    skos:prefLabel "Terracettes" ;
    schema:url "https://github.com/ternaustralia/dawe-rlp-vocabs/tree/main/vocab_files/categorical_collections/luts/soils-microrelief-types.ttl"^^xsd:anyURI ;
.

<https://linked.data.gov.au/def/test/dawe-cv/ba6428ab-7e7d-54f4-8a1c-c97749febddb>
    a skos:Concept ;
    dcterms:identifier 2 ;
    dcterms:source <http://vocabs.paratoo.tern.org.au:1337/api/lut-soils-microrelief-types> ;
    rdfs:isDefinedBy <https://linked.data.gov.au/def/nrm> ;
    skos:definition "Irregularly distributed; small depressions and mounds separated by a more or less continuous shelf. Vertical interval usually less than 0.3 m. Horizontal interval usually 3-20 m; surface almost level." ;
    skos:notation "C" ;
    skos:prefLabel "Crabhole gilgai" ;
    schema:url "https://github.com/ternaustralia/dawe-rlp-vocabs/tree/main/vocab_files/categorical_collections/luts/soils-microrelief-types.ttl"^^xsd:anyURI ;
.

<https://linked.data.gov.au/def/test/dawe-cv/bb7102b7-aaec-54c9-bc85-bc9d5dc1b2c4>
    a skos:Concept ;
    dcterms:identifier 18 ;
    dcterms:source <http://vocabs.paratoo.tern.org.au:1337/api/lut-soils-microrelief-types> ;
    rdfs:isDefinedBy <https://linked.data.gov.au/def/nrm> ;
    skos:definition "Depression associated with water flowing from rock or soil without human intervention" ;
    skos:notation "H" ;
    skos:prefLabel "Spring hollow" ;
    schema:url "https://github.com/ternaustralia/dawe-rlp-vocabs/tree/main/vocab_files/categorical_collections/luts/soils-microrelief-types.ttl"^^xsd:anyURI ;
.

<https://linked.data.gov.au/def/test/dawe-cv/dd620811-2995-57da-88a0-e113212b07d1>
    a skos:Concept ;
    dcterms:identifier 9 ;
    dcterms:source <http://vocabs.paratoo.tern.org.au:1337/api/lut-soils-microrelief-types> ;
    rdfs:isDefinedBy <https://linked.data.gov.au/def/nrm> ;
    skos:definition "Steep-sided hummocks rising above a flat surface. Hummocks are frequently occupied by trees or shrubs while the lower surface may be vegetation free or occupied by sedges or reeds. They are subject to prolonged seasonal flooding." ;
    skos:notation "W" ;
    skos:prefLabel "Swamp hummock" ;
    schema:url "https://github.com/ternaustralia/dawe-rlp-vocabs/tree/main/vocab_files/categorical_collections/luts/soils-microrelief-types.ttl"^^xsd:anyURI ;
.

<https://linked.data.gov.au/def/test/dawe-cv/deba9223-29d2-5330-a5a8-a7667a4520aa>
    a skos:Concept ;
    dcterms:identifier 19 ;
    dcterms:source <http://vocabs.paratoo.tern.org.au:1337/api/lut-soils-microrelief-types> ;
    rdfs:isDefinedBy <https://linked.data.gov.au/def/nrm> ;
    skos:definition "" ;
    skos:notation "O" ;
    skos:prefLabel "Other (see site notes)" ;
    schema:url "https://github.com/ternaustralia/dawe-rlp-vocabs/tree/main/vocab_files/categorical_collections/luts/soils-microrelief-types.ttl"^^xsd:anyURI ;
.

<https://linked.data.gov.au/def/test/dawe-cv/ee59db14-2399-51cd-bfd0-6746f12f02de>
    a skos:Concept ;
    dcterms:identifier 7 ;
    dcterms:source <http://vocabs.paratoo.tern.org.au:1337/api/lut-soils-microrelief-types> ;
    rdfs:isDefinedBy <https://linked.data.gov.au/def/nrm> ;
    skos:definition "Long; elongate depressions and parallel adjacent downslope mounds; which follow the contour. These depression-mound associations are separated from each other by shelves 10-100 m wide. Mounds are low; usually less than 0.5 m high; and often poorly defined." ;
    skos:notation "G" ;
    skos:prefLabel "Contour gilgai" ;
    schema:url "https://github.com/ternaustralia/dawe-rlp-vocabs/tree/main/vocab_files/categorical_collections/luts/soils-microrelief-types.ttl"^^xsd:anyURI ;
.

