PREFIX dcterms: <http://purl.org/dc/terms/>
PREFIX rdfs: <http://www.w3.org/2000/01/rdf-schema#>
PREFIX schema: <https://schema.org/>
PREFIX skos: <http://www.w3.org/2004/02/skos/core#>
PREFIX xsd: <http://www.w3.org/2001/XMLSchema#>

<https://linked.data.gov.au/def/test/dawe-cv/31d3921f-1fcb-4ec2-99a6-749c7b9e4798>
    a skos:Collection ;
    dcterms:description "A collection of soils horizon suffixes and its codes." ;
    dcterms:source <http://vocabs.paratoo.tern.org.au:1337/api/lut-soils-horizon-suffixes> ;
    rdfs:isDefinedBy <https://linked.data.gov.au/def/nrm> ;
    skos:member
        <https://linked.data.gov.au/def/test/dawe-cv/2d113077-d092-5317-a4b4-bd7385411c7f> ,
        <https://linked.data.gov.au/def/test/dawe-cv/33b116b5-77fd-5e82-a22a-b500e47a0251> ,
        <https://linked.data.gov.au/def/test/dawe-cv/34d19de1-9209-59f2-908a-50d35b021ef8> ,
        <https://linked.data.gov.au/def/test/dawe-cv/35da0dbf-ada0-5a03-99da-00082dae37f4> ,
        <https://linked.data.gov.au/def/test/dawe-cv/39a38d90-d08e-515c-aedd-1fd44e291f60> ,
        <https://linked.data.gov.au/def/test/dawe-cv/3aadcf39-9397-5319-8b89-15b20ca0248d> ,
        <https://linked.data.gov.au/def/test/dawe-cv/3c1db619-d599-5784-a3b1-4239bfe1c90a> ,
        <https://linked.data.gov.au/def/test/dawe-cv/42d61f24-35d3-5122-af45-46a71dacaf62> ,
        <https://linked.data.gov.au/def/test/dawe-cv/5f2658d4-d489-5eb7-bd41-445c1059e164> ,
        <https://linked.data.gov.au/def/test/dawe-cv/654a1590-e380-5e52-92a0-50fec78d9954> ,
        <https://linked.data.gov.au/def/test/dawe-cv/72bad82d-2483-5a1d-8319-d21a310fbea8> ,
        <https://linked.data.gov.au/def/test/dawe-cv/8091fc1d-20a9-596b-bc62-51b8f6c59b49> ,
        <https://linked.data.gov.au/def/test/dawe-cv/9457eb01-739b-5d9e-af3f-4fa0ff3f292e> ,
        <https://linked.data.gov.au/def/test/dawe-cv/abe7bc35-3992-5c46-a804-dfbd36c95a61> ,
        <https://linked.data.gov.au/def/test/dawe-cv/b1ba3c92-b8f4-5d89-8b2f-c339427a9016> ,
        <https://linked.data.gov.au/def/test/dawe-cv/b337f4ff-0365-58cf-af73-a942e2832056> ,
        <https://linked.data.gov.au/def/test/dawe-cv/d4953627-581e-564b-a8d5-1277ca62e9fa> ,
        <https://linked.data.gov.au/def/test/dawe-cv/ddbd79fb-5e25-569d-bfe8-3096fdbd662a> ,
        <https://linked.data.gov.au/def/test/dawe-cv/dfc57f96-0f6a-5ae6-b257-930b1a137660> ,
        <https://linked.data.gov.au/def/test/dawe-cv/f164a23c-1cd5-542f-bb0c-90d7bb679bda> ;
    skos:prefLabel "Soils horizon suffixes codes" ;
    schema:url "https://github.com/ternaustralia/dawe-rlp-vocabs/tree/master/vocab_files/categorical_collections/luts/soils-horizon-suffixes.ttl" ;
.

<https://linked.data.gov.au/def/test/dawe-cv/2d113077-d092-5317-a4b4-bd7385411c7f>
    a skos:Concept ;
    dcterms:identifier 14 ;
    dcterms:source <http://vocabs.paratoo.tern.org.au:1337/api/lut-soils-horizon-suffixes> ;
    rdfs:isDefinedBy <https://linked.data.gov.au/def/nrm> ;
    skos:definition "Horizons with an accumulation of sesquioxide– organic matter complexes in which iron is dominant relative to aluminium. Often used in combination with ‘h’." ;
    skos:notation "s" ;
    skos:prefLabel "s" ;
    schema:url "https://github.com/ternaustralia/dawe-rlp-vocabs/tree/master/vocab_files/categorical_collections/luts/soils-horizon-suffixes.ttl" ;
.

<https://linked.data.gov.au/def/test/dawe-cv/33b116b5-77fd-5e82-a22a-b500e47a0251>
    a skos:Concept ;
    dcterms:identifier 10 ;
    dcterms:source <http://vocabs.paratoo.tern.org.au:1337/api/lut-soils-horizon-suffixes> ;
    rdfs:isDefinedBy <https://linked.data.gov.au/def/nrm> ;
    skos:definition "Horizons with strong cementation or induration." ;
    skos:notation "m" ;
    skos:prefLabel "m" ;
    schema:url "https://github.com/ternaustralia/dawe-rlp-vocabs/tree/master/vocab_files/categorical_collections/luts/soils-horizon-suffixes.ttl" ;
.

<https://linked.data.gov.au/def/test/dawe-cv/34d19de1-9209-59f2-908a-50d35b021ef8>
    a skos:Concept ;
    dcterms:identifier 18 ;
    dcterms:source <http://vocabs.paratoo.tern.org.au:1337/api/lut-soils-horizon-suffixes> ;
    rdfs:isDefinedBy <https://linked.data.gov.au/def/nrm> ;
    skos:definition "Horizons with accumulation of calcium sulfate (gypsum)." ;
    skos:notation "y" ;
    skos:prefLabel "y" ;
    schema:url "https://github.com/ternaustralia/dawe-rlp-vocabs/tree/master/vocab_files/categorical_collections/luts/soils-horizon-suffixes.ttl" ;
.

<https://linked.data.gov.au/def/test/dawe-cv/35da0dbf-ada0-5a03-99da-00082dae37f4>
    a skos:Concept ;
    dcterms:identifier 8 ;
    dcterms:source <http://vocabs.paratoo.tern.org.au:1337/api/lut-soils-horizon-suffixes> ;
    rdfs:isDefinedBy <https://linked.data.gov.au/def/nrm> ;
    skos:definition "Sporadically bleached horizons." ;
    skos:notation "j" ;
    skos:prefLabel "j" ;
    schema:url "https://github.com/ternaustralia/dawe-rlp-vocabs/tree/master/vocab_files/categorical_collections/luts/soils-horizon-suffixes.ttl" ;
.

<https://linked.data.gov.au/def/test/dawe-cv/39a38d90-d08e-515c-aedd-1fd44e291f60>
    a skos:Concept ;
    dcterms:identifier 7 ;
    dcterms:source <http://vocabs.paratoo.tern.org.au:1337/api/lut-soils-horizon-suffixes> ;
    rdfs:isDefinedBy <https://linked.data.gov.au/def/nrm> ;
    skos:definition "Horizons that contain accumulation of amorphous, organic matter–aluminium complexes in which iron contents are very low." ;
    skos:notation "h" ;
    skos:prefLabel "h" ;
    schema:url "https://github.com/ternaustralia/dawe-rlp-vocabs/tree/master/vocab_files/categorical_collections/luts/soils-horizon-suffixes.ttl" ;
.

<https://linked.data.gov.au/def/test/dawe-cv/3aadcf39-9397-5319-8b89-15b20ca0248d>
    a skos:Concept ;
    dcterms:identifier 1 ;
    dcterms:source <http://vocabs.paratoo.tern.org.au:1337/api/lut-soils-horizon-suffixes> ;
    rdfs:isDefinedBy <https://linked.data.gov.au/def/nrm> ;
    skos:definition "Buried soil horizons. Used in mineral soils only." ;
    skos:notation "b" ;
    skos:prefLabel "b" ;
    schema:url "https://github.com/ternaustralia/dawe-rlp-vocabs/tree/master/vocab_files/categorical_collections/luts/soils-horizon-suffixes.ttl" ;
.

<https://linked.data.gov.au/def/test/dawe-cv/3c1db619-d599-5784-a3b1-4239bfe1c90a>
    a skos:Concept ;
    dcterms:identifier 12 ;
    dcterms:source <http://vocabs.paratoo.tern.org.au:1337/api/lut-soils-horizon-suffixes> ;
    rdfs:isDefinedBy <https://linked.data.gov.au/def/nrm> ;
    skos:definition "Horizons with accumulation of secondary silica. If silica cementation is continuous or nearly continuous, ‘qm’ is used." ;
    skos:notation "q" ;
    skos:prefLabel "q" ;
    schema:url "https://github.com/ternaustralia/dawe-rlp-vocabs/tree/master/vocab_files/categorical_collections/luts/soils-horizon-suffixes.ttl" ;
.

<https://linked.data.gov.au/def/test/dawe-cv/42d61f24-35d3-5122-af45-46a71dacaf62>
    a skos:Concept ;
    dcterms:identifier 20 ;
    dcterms:source <http://vocabs.paratoo.tern.org.au:1337/api/lut-soils-horizon-suffixes> ;
    rdfs:isDefinedBy <https://linked.data.gov.au/def/nrm> ;
    skos:definition "Query. Used where doubt is associated with the nomenclature of the horizon, with the query following the horizon notation (e.g. ‘D?’)" ;
    skos:notation "?" ;
    skos:prefLabel "?" ;
    schema:url "https://github.com/ternaustralia/dawe-rlp-vocabs/tree/master/vocab_files/categorical_collections/luts/soils-horizon-suffixes.ttl" ;
.

<https://linked.data.gov.au/def/test/dawe-cv/5f2658d4-d489-5eb7-bd41-445c1059e164>
    a skos:Concept ;
    dcterms:identifier 13 ;
    dcterms:source <http://vocabs.paratoo.tern.org.au:1337/api/lut-soils-horizon-suffixes> ;
    rdfs:isDefinedBy <https://linked.data.gov.au/def/nrm> ;
    skos:definition "Horizons with layers of weathered rock (including saprolite) that, although consolidated, can be dug with hand tools." ;
    skos:notation "r" ;
    skos:prefLabel "r" ;
    schema:url "https://github.com/ternaustralia/dawe-rlp-vocabs/tree/master/vocab_files/categorical_collections/luts/soils-horizon-suffixes.ttl" ;
.

<https://linked.data.gov.au/def/test/dawe-cv/654a1590-e380-5e52-92a0-50fec78d9954>
    a skos:Concept ;
    dcterms:identifier 9 ;
    dcterms:source <http://vocabs.paratoo.tern.org.au:1337/api/lut-soils-horizon-suffixes> ;
    rdfs:isDefinedBy <https://linked.data.gov.au/def/nrm> ;
    skos:definition "Horizons with accumulation of carbonates, commonly calcium carbonate." ;
    skos:notation "k" ;
    skos:prefLabel "k" ;
    schema:url "https://github.com/ternaustralia/dawe-rlp-vocabs/tree/master/vocab_files/categorical_collections/luts/soils-horizon-suffixes.ttl" ;
.

<https://linked.data.gov.au/def/test/dawe-cv/72bad82d-2483-5a1d-8319-d21a310fbea8>
    a skos:Concept ;
    dcterms:identifier 6 ;
    dcterms:source <http://vocabs.paratoo.tern.org.au:1337/api/lut-soils-horizon-suffixes> ;
    rdfs:isDefinedBy <https://linked.data.gov.au/def/nrm> ;
    skos:definition "Indicates strong gleying." ;
    skos:notation "g" ;
    skos:prefLabel "g" ;
    schema:url "https://github.com/ternaustralia/dawe-rlp-vocabs/tree/master/vocab_files/categorical_collections/luts/soils-horizon-suffixes.ttl" ;
.

<https://linked.data.gov.au/def/test/dawe-cv/8091fc1d-20a9-596b-bc62-51b8f6c59b49>
    a skos:Concept ;
    dcterms:identifier 3 ;
    dcterms:source <http://vocabs.paratoo.tern.org.au:1337/api/lut-soils-horizon-suffixes> ;
    rdfs:isDefinedBy <https://linked.data.gov.au/def/nrm> ;
    skos:definition "Densipans. Very fine, sandy, earthy pan." ;
    skos:notation "d" ;
    skos:prefLabel "d" ;
    schema:url "https://github.com/ternaustralia/dawe-rlp-vocabs/tree/master/vocab_files/categorical_collections/luts/soils-horizon-suffixes.ttl" ;
.

<https://linked.data.gov.au/def/test/dawe-cv/9457eb01-739b-5d9e-af3f-4fa0ff3f292e>
    a skos:Concept ;
    dcterms:identifier 17 ;
    dcterms:source <http://vocabs.paratoo.tern.org.au:1337/api/lut-soils-horizon-suffixes> ;
    rdfs:isDefinedBy <https://linked.data.gov.au/def/nrm> ;
    skos:definition "Fragipans or earthy pans." ;
    skos:notation "x" ;
    skos:prefLabel "x" ;
    schema:url "https://github.com/ternaustralia/dawe-rlp-vocabs/tree/master/vocab_files/categorical_collections/luts/soils-horizon-suffixes.ttl" ;
.

<https://linked.data.gov.au/def/test/dawe-cv/abe7bc35-3992-5c46-a804-dfbd36c95a61>
    a skos:Concept ;
    dcterms:identifier 4 ;
    dcterms:source <http://vocabs.paratoo.tern.org.au:1337/api/lut-soils-horizon-suffixes> ;
    rdfs:isDefinedBy <https://linked.data.gov.au/def/nrm> ;
    skos:definition "Conspicuously bleached horizons." ;
    skos:notation "e" ;
    skos:prefLabel "e" ;
    schema:url "https://github.com/ternaustralia/dawe-rlp-vocabs/tree/master/vocab_files/categorical_collections/luts/soils-horizon-suffixes.ttl" ;
.

<https://linked.data.gov.au/def/test/dawe-cv/b1ba3c92-b8f4-5d89-8b2f-c339427a9016>
    a skos:Concept ;
    dcterms:identifier 15 ;
    dcterms:source <http://vocabs.paratoo.tern.org.au:1337/api/lut-soils-horizon-suffixes> ;
    rdfs:isDefinedBy <https://linked.data.gov.au/def/nrm> ;
    skos:definition "Horizons with accumulation of silicate clay (from German ton, clay)." ;
    skos:notation "t" ;
    skos:prefLabel "t" ;
    schema:url "https://github.com/ternaustralia/dawe-rlp-vocabs/tree/master/vocab_files/categorical_collections/luts/soils-horizon-suffixes.ttl" ;
.

<https://linked.data.gov.au/def/test/dawe-cv/b337f4ff-0365-58cf-af73-a942e2832056>
    a skos:Concept ;
    dcterms:identifier 11 ;
    dcterms:source <http://vocabs.paratoo.tern.org.au:1337/api/lut-soils-horizon-suffixes> ;
    rdfs:isDefinedBy <https://linked.data.gov.au/def/nrm> ;
    skos:definition "Horizons where ploughing, tillage practices or other disturbance by humans has occurred (e.g. deep ripping)." ;
    skos:notation "p" ;
    skos:prefLabel "p" ;
    schema:url "https://github.com/ternaustralia/dawe-rlp-vocabs/tree/master/vocab_files/categorical_collections/luts/soils-horizon-suffixes.ttl" ;
.

<https://linked.data.gov.au/def/test/dawe-cv/d4953627-581e-564b-a8d5-1277ca62e9fa>
    a skos:Concept ;
    dcterms:identifier 5 ;
    dcterms:source <http://vocabs.paratoo.tern.org.au:1337/api/lut-soils-horizon-suffixes> ;
    rdfs:isDefinedBy <https://linked.data.gov.au/def/nrm> ;
    skos:definition "Faunal accumulation, such as worm casts, dominates certain A1 horizons." ;
    skos:notation "f" ;
    skos:prefLabel "f" ;
    schema:url "https://github.com/ternaustralia/dawe-rlp-vocabs/tree/master/vocab_files/categorical_collections/luts/soils-horizon-suffixes.ttl" ;
.

<https://linked.data.gov.au/def/test/dawe-cv/ddbd79fb-5e25-569d-bfe8-3096fdbd662a>
    a skos:Concept ;
    dcterms:identifier 16 ;
    dcterms:source <http://vocabs.paratoo.tern.org.au:1337/api/lut-soils-horizon-suffixes> ;
    rdfs:isDefinedBy <https://linked.data.gov.au/def/nrm> ;
    skos:definition "Development of colour and/or structure, or both, observed in the B horizon, with little or no accumulation of sesquioxide– organic matter complexes." ;
    skos:notation "w" ;
    skos:prefLabel "w" ;
    schema:url "https://github.com/ternaustralia/dawe-rlp-vocabs/tree/master/vocab_files/categorical_collections/luts/soils-horizon-suffixes.ttl" ;
.

<https://linked.data.gov.au/def/test/dawe-cv/dfc57f96-0f6a-5ae6-b257-930b1a137660>
    a skos:Concept ;
    dcterms:identifier 2 ;
    dcterms:source <http://vocabs.paratoo.tern.org.au:1337/api/lut-soils-horizon-suffixes> ;
    rdfs:isDefinedBy <https://linked.data.gov.au/def/nrm> ;
    skos:definition "Horizons with accumulation of concretions or nodules of iron and/or aluminium and/or manganese." ;
    skos:notation "c" ;
    skos:prefLabel "c" ;
    schema:url "https://github.com/ternaustralia/dawe-rlp-vocabs/tree/master/vocab_files/categorical_collections/luts/soils-horizon-suffixes.ttl" ;
.

<https://linked.data.gov.au/def/test/dawe-cv/f164a23c-1cd5-542f-bb0c-90d7bb679bda>
    a skos:Concept ;
    dcterms:identifier 19 ;
    dcterms:source <http://vocabs.paratoo.tern.org.au:1337/api/lut-soils-horizon-suffixes> ;
    rdfs:isDefinedBy <https://linked.data.gov.au/def/nrm> ;
    skos:definition "Horizons with accumulation of salts more soluble than calcium sulfate and calcium carbonate." ;
    skos:notation "z" ;
    skos:prefLabel "z" ;
    schema:url "https://github.com/ternaustralia/dawe-rlp-vocabs/tree/master/vocab_files/categorical_collections/luts/soils-horizon-suffixes.ttl" ;
.

