# Do not edit this file directly. This file is generated by `make luts` with endpoints from src/dawe_nrm/api/categorical_values/endpoints.py
PREFIX dcterms: <http://purl.org/dc/terms/>
PREFIX rdfs: <http://www.w3.org/2000/01/rdf-schema#>
PREFIX schema: <https://schema.org/>
PREFIX skos: <http://www.w3.org/2004/02/skos/core#>
PREFIX xsd: <http://www.w3.org/2001/XMLSchema#>

<https://linked.data.gov.au/def/test/dawe-cv/d0fc07a7-3ec9-45ed-8850-885a32828d3c>
    a skos:Collection ;
    dcterms:description "A collection of vegetation growth form types and its codes." ;
    dcterms:source <http://vocabs.paratoo.tern.org.au:1337/api/lut-veg-growth-forms> ;
    rdfs:isDefinedBy <https://linked.data.gov.au/def/nrm> ;
    skos:member
        <https://linked.data.gov.au/def/test/dawe-cv/062132e9-426e-56c8-9c92-2781692bdd0c> ,
        <https://linked.data.gov.au/def/test/dawe-cv/0c0c23e2-47c1-56c7-8fa0-3ac241caf196> ,
        <https://linked.data.gov.au/def/test/dawe-cv/0f6de186-e8a9-5445-87f2-5aaf927a0f6d> ,
        <https://linked.data.gov.au/def/test/dawe-cv/1b532a75-319d-5a3c-af12-76348fa0cec4> ,
        <https://linked.data.gov.au/def/test/dawe-cv/1e3ff92d-f2dc-5b87-827e-d9603c29e537> ,
        <https://linked.data.gov.au/def/test/dawe-cv/2de905be-b280-54ba-b9a7-7c6f088f301c> ,
        <https://linked.data.gov.au/def/test/dawe-cv/37512bb9-f5a9-5cc5-9f66-3c9c94d98958> ,
        <https://linked.data.gov.au/def/test/dawe-cv/5661df01-90d6-5a3a-93c9-ce41bf1f9cb5> ,
        <https://linked.data.gov.au/def/test/dawe-cv/5b669769-cfda-5e2f-a311-acc06cd1ff02> ,
        <https://linked.data.gov.au/def/test/dawe-cv/616c356b-38ff-500e-bc9a-a55b60c6e1e8> ,
        <https://linked.data.gov.au/def/test/dawe-cv/8a2f124b-4c90-5b35-b421-aa7447fb2f30> ,
        <https://linked.data.gov.au/def/test/dawe-cv/8f4fd07c-a8a8-5e6f-81b3-4506a6a2d629> ,
        <https://linked.data.gov.au/def/test/dawe-cv/922ed906-5ab9-5f14-b6ae-d7b24deccdeb> ,
        <https://linked.data.gov.au/def/test/dawe-cv/9882cf8c-6c69-5991-b505-6e34ae02563d> ,
        <https://linked.data.gov.au/def/test/dawe-cv/9dd59dcd-7311-50fc-a657-603703fbf023> ,
        <https://linked.data.gov.au/def/test/dawe-cv/a7e63c10-9eae-5187-af68-f1ddd8e9ea27> ,
        <https://linked.data.gov.au/def/test/dawe-cv/b5a5217d-6d51-5c8a-9728-e4fb5ca8afaf> ,
        <https://linked.data.gov.au/def/test/dawe-cv/b95c55f0-ea57-5a77-a416-2fd6cf378014> ,
        <https://linked.data.gov.au/def/test/dawe-cv/bc5db7f8-3b75-58d3-ab8f-2c0076807221> ,
        <https://linked.data.gov.au/def/test/dawe-cv/c2eae401-0ac0-507e-bbfe-fe0bf9545f66> ,
        <https://linked.data.gov.au/def/test/dawe-cv/cce3d3df-85ee-5609-9e0d-3d7383843b3a> ,
        <https://linked.data.gov.au/def/test/dawe-cv/d647f263-dd3f-5626-bd6e-0e86131e6106> ,
        <https://linked.data.gov.au/def/test/dawe-cv/dfdbbd27-e0d9-52c6-96a0-d88ff882aab7> ,
        <https://linked.data.gov.au/def/test/dawe-cv/e20d86ce-6cd9-5a88-9b4d-ccafbb8e3a51> ,
        <https://linked.data.gov.au/def/test/dawe-cv/ea88802e-3465-51c8-b437-8da61208a395> ,
        <https://linked.data.gov.au/def/test/dawe-cv/eb5f51a6-0a5c-5e67-883d-35883fcf3ba3> ,
        <https://linked.data.gov.au/def/test/dawe-cv/ef6a07fa-47ce-5cf4-ad06-218556c0dde4> ;
    skos:prefLabel "Vegetation growth form codes" ;
    schema:url "https://github.com/ternaustralia/dawe-rlp-vocabs/tree/main/vocab_files/categorical_collections/luts/vegetation-growth-form.ttl"^^xsd:anyURI ;
.

<https://linked.data.gov.au/def/test/dawe-cv/062132e9-426e-56c8-9c92-2781692bdd0c>
    a skos:Concept ;
    dcterms:identifier 2 ;
    dcterms:source <http://vocabs.paratoo.tern.org.au:1337/api/lut-veg-growth-forms> ;
    rdfs:isDefinedBy <https://linked.data.gov.au/def/nrm> ;
    skos:definition "Australian grass trees. Members of the Xanthorroeaceae." ;
    skos:notation "X" ;
    skos:prefLabel "Grass-tree" ;
    schema:url "https://github.com/ternaustralia/dawe-rlp-vocabs/tree/main/vocab_files/categorical_collections/luts/vegetation-growth-form.ttl"^^xsd:anyURI ;
.

<https://linked.data.gov.au/def/test/dawe-cv/0c0c23e2-47c1-56c7-8fa0-3ac241caf196>
    a skos:Concept ;
    dcterms:identifier 3 ;
    dcterms:source <http://vocabs.paratoo.tern.org.au:1337/api/lut-veg-growth-forms> ;
    rdfs:isDefinedBy <https://linked.data.gov.au/def/nrm> ;
    skos:definition " Shrub usually less than 2m, with sclerophyllous leaves having high fibre:protein ratios and with an area of nanophyll or smaller (less than 225 sq. m.). Often a member of one the following families: Epacridaceae, Myrtaceae, Fabaceae and Proteaceae. Commonly occur on nutrient-poor substrates." ;
    skos:notation "Z" ;
    skos:prefLabel "Heath-shrub" ;
    schema:url "https://github.com/ternaustralia/dawe-rlp-vocabs/tree/main/vocab_files/categorical_collections/luts/vegetation-growth-form.ttl"^^xsd:anyURI ;
.

<https://linked.data.gov.au/def/test/dawe-cv/0f6de186-e8a9-5445-87f2-5aaf927a0f6d>
    a skos:Concept ;
    dcterms:identifier 23 ;
    dcterms:source <http://vocabs.paratoo.tern.org.au:1337/api/lut-veg-growth-forms> ;
    rdfs:isDefinedBy <https://linked.data.gov.au/def/nrm> ;
    skos:definition "" ;
    skos:notation "U" ;
    skos:prefLabel "Unknown" ;
    schema:url "https://github.com/ternaustralia/dawe-rlp-vocabs/tree/main/vocab_files/categorical_collections/luts/vegetation-growth-form.ttl"^^xsd:anyURI ;
.

<https://linked.data.gov.au/def/test/dawe-cv/1b532a75-319d-5a3c-af12-76348fa0cec4>
    a skos:Concept ;
    dcterms:identifier 24 ;
    dcterms:source <http://vocabs.paratoo.tern.org.au:1337/api/lut-veg-growth-forms> ;
    rdfs:isDefinedBy <https://linked.data.gov.au/def/nrm> ;
    skos:definition "Genera (of Tribe Salicornioideae, viz.: Halosarcia, Pachycornia, Sarcocornia, Sclerostegia, Tecticorniaand Tegicornia) with articulate branches, fleshy stems and reduced flowers within the Chenopodiaceae family, succulent chenopods (Wilson 1980). Also the genus Suaeda." ;
    skos:notation "SS" ;
    skos:prefLabel "Samphire Shrub" ;
    schema:url "https://github.com/ternaustralia/dawe-rlp-vocabs/tree/main/vocab_files/categorical_collections/luts/vegetation-growth-form.ttl"^^xsd:anyURI ;
.

<https://linked.data.gov.au/def/test/dawe-cv/1e3ff92d-f2dc-5b87-827e-d9603c29e537>
    a skos:Concept ;
    dcterms:identifier 14 ;
    dcterms:source <http://vocabs.paratoo.tern.org.au:1337/api/lut-veg-growth-forms> ;
    rdfs:isDefinedBy <https://linked.data.gov.au/def/nrm> ;
    skos:definition "Epiphytes, mistletoes and parasites. Plant with roots attached to the aerial portions of other plants. Often could also be another growth form, such as fern or forb." ;
    skos:notation "K" ;
    skos:prefLabel "Epiphyte" ;
    schema:url "https://github.com/ternaustralia/dawe-rlp-vocabs/tree/main/vocab_files/categorical_collections/luts/vegetation-growth-form.ttl"^^xsd:anyURI ;
.

<https://linked.data.gov.au/def/test/dawe-cv/2de905be-b280-54ba-b9a7-7c6f088f301c>
    a skos:Concept ;
    dcterms:identifier 17 ;
    dcterms:source <http://vocabs.paratoo.tern.org.au:1337/api/lut-veg-growth-forms> ;
    rdfs:isDefinedBy <https://linked.data.gov.au/def/nrm> ;
    skos:definition "Woody plants multi-stemmed at the base (or within 200mm from ground level) or if single stemmed, less than 2m." ;
    skos:notation "S" ;
    skos:prefLabel "Shrub" ;
    schema:url "https://github.com/ternaustralia/dawe-rlp-vocabs/tree/main/vocab_files/categorical_collections/luts/vegetation-growth-form.ttl"^^xsd:anyURI ;
.

<https://linked.data.gov.au/def/test/dawe-cv/37512bb9-f5a9-5cc5-9f66-3c9c94d98958>
    a skos:Concept ;
    dcterms:identifier 8 ;
    dcterms:source <http://vocabs.paratoo.tern.org.au:1337/api/lut-veg-growth-forms> ;
    rdfs:isDefinedBy <https://linked.data.gov.au/def/nrm> ;
    skos:definition "Lower plant" ;
    skos:notation "FU" ;
    skos:prefLabel "Fungus" ;
    schema:url "https://github.com/ternaustralia/dawe-rlp-vocabs/tree/main/vocab_files/categorical_collections/luts/vegetation-growth-form.ttl"^^xsd:anyURI ;
.

<https://linked.data.gov.au/def/test/dawe-cv/5661df01-90d6-5a3a-93c9-ce41bf1f9cb5>
    a skos:Concept ;
    dcterms:identifier 21 ;
    dcterms:source <http://vocabs.paratoo.tern.org.au:1337/api/lut-veg-growth-forms> ;
    rdfs:isDefinedBy <https://linked.data.gov.au/def/nrm> ;
    skos:definition "Climbing, twining, winding or sprawling plants usually with a woody stem." ;
    skos:notation "L" ;
    skos:prefLabel "Vine" ;
    schema:url "https://github.com/ternaustralia/dawe-rlp-vocabs/tree/main/vocab_files/categorical_collections/luts/vegetation-growth-form.ttl"^^xsd:anyURI ;
.

<https://linked.data.gov.au/def/test/dawe-cv/5b669769-cfda-5e2f-a311-acc06cd1ff02>
    a skos:Concept ;
    dcterms:identifier 15 ;
    dcterms:source <http://vocabs.paratoo.tern.org.au:1337/api/lut-veg-growth-forms> ;
    rdfs:isDefinedBy <https://linked.data.gov.au/def/nrm> ;
    skos:definition "Ferns and fern allies. Characterised by large and usually branched leaves (fronds), herbaceous and terrestrial to aquatic; spores in sporangia on the leaves." ;
    skos:notation "E" ;
    skos:prefLabel "Fern" ;
    schema:url "https://github.com/ternaustralia/dawe-rlp-vocabs/tree/main/vocab_files/categorical_collections/luts/vegetation-growth-form.ttl"^^xsd:anyURI ;
.

<https://linked.data.gov.au/def/test/dawe-cv/616c356b-38ff-500e-bc9a-a55b60c6e1e8>
    a skos:Concept ;
    dcterms:identifier 19 ;
    dcterms:source <http://vocabs.paratoo.tern.org.au:1337/api/lut-veg-growth-forms> ;
    rdfs:isDefinedBy <https://linked.data.gov.au/def/nrm> ;
    skos:definition "Woody perennial plant usually of the genus Eucalyptus. Multi-stemmed with fewer than 5 trunks of which at least 3 exceed 100mm at breast height (1.3m). Usually 8m or more." ;
    skos:notation "M" ;
    skos:prefLabel "Tree Mallee" ;
    schema:url "https://github.com/ternaustralia/dawe-rlp-vocabs/tree/main/vocab_files/categorical_collections/luts/vegetation-growth-form.ttl"^^xsd:anyURI ;
.

<https://linked.data.gov.au/def/test/dawe-cv/8a2f124b-4c90-5b35-b421-aa7447fb2f30>
    a skos:Concept ;
    dcterms:identifier 9 ;
    dcterms:source <http://vocabs.paratoo.tern.org.au:1337/api/lut-veg-growth-forms> ;
    rdfs:isDefinedBy <https://linked.data.gov.au/def/nrm> ;
    skos:definition "Not Collected" ;
    skos:notation "NC" ;
    skos:prefLabel "NC" ;
    schema:url "https://github.com/ternaustralia/dawe-rlp-vocabs/tree/main/vocab_files/categorical_collections/luts/vegetation-growth-form.ttl"^^xsd:anyURI ;
.

<https://linked.data.gov.au/def/test/dawe-cv/8f4fd07c-a8a8-5e6f-81b3-4506a6a2d629>
    a skos:Concept ;
    dcterms:identifier 10 ;
    dcterms:source <http://vocabs.paratoo.tern.org.au:1337/api/lut-veg-growth-forms> ;
    rdfs:isDefinedBy <https://linked.data.gov.au/def/nrm> ;
    skos:definition "Herbaceous or slightly woody, annual or sometimes perennial plant (usually a dicotyledon)." ;
    skos:notation "F" ;
    skos:prefLabel "Forb" ;
    schema:url "https://github.com/ternaustralia/dawe-rlp-vocabs/tree/main/vocab_files/categorical_collections/luts/vegetation-growth-form.ttl"^^xsd:anyURI ;
.

<https://linked.data.gov.au/def/test/dawe-cv/922ed906-5ab9-5f14-b6ae-d7b24deccdeb>
    a skos:Concept ;
    dcterms:identifier 18 ;
    dcterms:source <http://vocabs.paratoo.tern.org.au:1337/api/lut-veg-growth-forms> ;
    rdfs:isDefinedBy <https://linked.data.gov.au/def/nrm> ;
    skos:definition "Commonly less than 8m tall, usually with 5 or more trunks, of which at least three of the largest do not exceed 100mm at breast height (1.3m)." ;
    skos:notation "Y" ;
    skos:prefLabel "Shrub Mallee" ;
    schema:url "https://github.com/ternaustralia/dawe-rlp-vocabs/tree/main/vocab_files/categorical_collections/luts/vegetation-growth-form.ttl"^^xsd:anyURI ;
.

<https://linked.data.gov.au/def/test/dawe-cv/9882cf8c-6c69-5991-b505-6e34ae02563d>
    a skos:Concept ;
    dcterms:identifier 22 ;
    dcterms:source <http://vocabs.paratoo.tern.org.au:1337/api/lut-veg-growth-forms> ;
    rdfs:isDefinedBy <https://linked.data.gov.au/def/nrm> ;
    skos:definition "Member of the family Poaceae, but having neither a distinctive tussock nor hummock appearance. Examples include stoloniferous species such as Cynodon dactylon." ;
    skos:notation "O" ;
    skos:prefLabel "Other Grass" ;
    schema:url "https://github.com/ternaustralia/dawe-rlp-vocabs/tree/main/vocab_files/categorical_collections/luts/vegetation-growth-form.ttl"^^xsd:anyURI ;
.

<https://linked.data.gov.au/def/test/dawe-cv/9dd59dcd-7311-50fc-a657-603703fbf023>
    a skos:Concept ;
    dcterms:identifier 20 ;
    dcterms:source <http://vocabs.paratoo.tern.org.au:1337/api/lut-veg-growth-forms> ;
    rdfs:isDefinedBy <https://linked.data.gov.au/def/nrm> ;
    skos:definition "Forms discrete but open tussocks usually with distinct individual shoots, or if not, then forming a hummock. These are the common agricultural grasses." ;
    skos:notation "G" ;
    skos:prefLabel "Tussock grass" ;
    schema:url "https://github.com/ternaustralia/dawe-rlp-vocabs/tree/main/vocab_files/categorical_collections/luts/vegetation-growth-form.ttl"^^xsd:anyURI ;
.

<https://linked.data.gov.au/def/test/dawe-cv/a7e63c10-9eae-5187-af68-f1ddd8e9ea27>
    a skos:Concept ;
    dcterms:identifier 26 ;
    dcterms:source <http://vocabs.paratoo.tern.org.au:1337/api/lut-veg-growth-forms> ;
    rdfs:isDefinedBy <https://linked.data.gov.au/def/nrm> ;
    skos:definition "Composite plant consisting of a fungus living symbiotically with algae; without true roots, stems or leaves." ;
    skos:notation "P" ;
    skos:prefLabel "Palm" ;
    schema:url "https://github.com/ternaustralia/dawe-rlp-vocabs/tree/main/vocab_files/categorical_collections/luts/vegetation-growth-form.ttl"^^xsd:anyURI ;
.

<https://linked.data.gov.au/def/test/dawe-cv/b5a5217d-6d51-5c8a-9728-e4fb5ca8afaf>
    a skos:Concept ;
    dcterms:identifier 1 ;
    dcterms:source <http://vocabs.paratoo.tern.org.au:1337/api/lut-veg-growth-forms> ;
    rdfs:isDefinedBy <https://linked.data.gov.au/def/nrm> ;
    skos:definition "Herbaceous, usually perennial erect plant generally with a tufted habit and of the families Cyperaceae (true sedges) or Restionaceae (node sedges)." ;
    skos:notation "V" ;
    skos:prefLabel "Sedge" ;
    schema:url "https://github.com/ternaustralia/dawe-rlp-vocabs/tree/main/vocab_files/categorical_collections/luts/vegetation-growth-form.ttl"^^xsd:anyURI ;
.

<https://linked.data.gov.au/def/test/dawe-cv/b95c55f0-ea57-5a77-a416-2fd6cf378014>
    a skos:Concept ;
    dcterms:identifier 5 ;
    dcterms:source <http://vocabs.paratoo.tern.org.au:1337/api/lut-veg-growth-forms> ;
    rdfs:isDefinedBy <https://linked.data.gov.au/def/nrm> ;
    skos:definition "Woody plants, more than 2m tall with a single stem or branches well above the base." ;
    skos:notation "TP" ;
    skos:prefLabel "Tree" ;
    schema:url "https://github.com/ternaustralia/dawe-rlp-vocabs/tree/main/vocab_files/categorical_collections/luts/vegetation-growth-form.ttl"^^xsd:anyURI ;
.

<https://linked.data.gov.au/def/test/dawe-cv/bc5db7f8-3b75-58d3-ab8f-2c0076807221>
    a skos:Concept ;
    dcterms:identifier 16 ;
    dcterms:source <http://vocabs.paratoo.tern.org.au:1337/api/lut-veg-growth-forms> ;
    rdfs:isDefinedBy <https://linked.data.gov.au/def/nrm> ;
    skos:definition "Coarse xeromorphic grass with a mound-like form often dead in the middle; genera are Triodia and Plectrachne." ;
    skos:notation "H" ;
    skos:prefLabel "Hummock grass" ;
    schema:url "https://github.com/ternaustralia/dawe-rlp-vocabs/tree/main/vocab_files/categorical_collections/luts/vegetation-growth-form.ttl"^^xsd:anyURI ;
.

<https://linked.data.gov.au/def/test/dawe-cv/c2eae401-0ac0-507e-bbfe-fe0bf9545f66>
    a skos:Concept ;
    dcterms:identifier 13 ;
    dcterms:source <http://vocabs.paratoo.tern.org.au:1337/api/lut-veg-growth-forms> ;
    rdfs:isDefinedBy <https://linked.data.gov.au/def/nrm> ;
    skos:definition "Single or multi-stemmed, semi-succulent shrub of the family Chenopodiaceae exhibiting drought and salt tolerance." ;
    skos:notation "C" ;
    skos:prefLabel "Chenopod" ;
    schema:url "https://github.com/ternaustralia/dawe-rlp-vocabs/tree/main/vocab_files/categorical_collections/luts/vegetation-growth-form.ttl"^^xsd:anyURI ;
.

<https://linked.data.gov.au/def/test/dawe-cv/cce3d3df-85ee-5609-9e0d-3d7383843b3a>
    a skos:Concept ;
    dcterms:identifier 27 ;
    dcterms:source <http://vocabs.paratoo.tern.org.au:1337/api/lut-veg-growth-forms> ;
    rdfs:isDefinedBy <https://linked.data.gov.au/def/nrm> ;
    skos:definition "Flowering angiosperms forming sparse to dense matsof material at the subtidal and down to 30 m below MSL. Occasionally exposed." ;
    skos:notation "SG" ;
    skos:prefLabel "Seagrass" ;
    schema:url "https://github.com/ternaustralia/dawe-rlp-vocabs/tree/main/vocab_files/categorical_collections/luts/vegetation-growth-form.ttl"^^xsd:anyURI ;
.

<https://linked.data.gov.au/def/test/dawe-cv/d647f263-dd3f-5626-bd6e-0e86131e6106>
    a skos:Concept ;
    dcterms:identifier 25 ;
    dcterms:source <http://vocabs.paratoo.tern.org.au:1337/api/lut-veg-growth-forms> ;
    rdfs:isDefinedBy <https://linked.data.gov.au/def/nrm> ;
    skos:definition "Composite plant consisting of a fungus living symbiotically with algae; without true roots, stems or leaves." ;
    skos:notation "LI" ;
    skos:prefLabel "Lichen" ;
    schema:url "https://github.com/ternaustralia/dawe-rlp-vocabs/tree/main/vocab_files/categorical_collections/luts/vegetation-growth-form.ttl"^^xsd:anyURI ;
.

<https://linked.data.gov.au/def/test/dawe-cv/dfdbbd27-e0d9-52c6-96a0-d88ff882aab7>
    a skos:Concept ;
    dcterms:identifier 12 ;
    dcterms:source <http://vocabs.paratoo.tern.org.au:1337/api/lut-veg-growth-forms> ;
    rdfs:isDefinedBy <https://linked.data.gov.au/def/nrm> ;
    skos:definition "Mosses and Liverworts. Mosses are small plants usually with a slender leaf-bearing stem with no true vascular tissue. Liverworts are often moss-like in appearance or consisting of a flat, ribbon like green thallus." ;
    skos:notation "B" ;
    skos:prefLabel "Bryophyte" ;
    schema:url "https://github.com/ternaustralia/dawe-rlp-vocabs/tree/main/vocab_files/categorical_collections/luts/vegetation-growth-form.ttl"^^xsd:anyURI ;
.

<https://linked.data.gov.au/def/test/dawe-cv/e20d86ce-6cd9-5a88-9b4d-ccafbb8e3a51>
    a skos:Concept ;
    dcterms:identifier 6 ;
    dcterms:source <http://vocabs.paratoo.tern.org.au:1337/api/lut-veg-growth-forms> ;
    rdfs:isDefinedBy <https://linked.data.gov.au/def/nrm> ;
    skos:definition "Characterised by large and usually branched leaves (fronds), arborescent and terrestrial; spores in sporangia on the leaves." ;
    skos:notation "D" ;
    skos:prefLabel "Tree-fern" ;
    schema:url "https://github.com/ternaustralia/dawe-rlp-vocabs/tree/main/vocab_files/categorical_collections/luts/vegetation-growth-form.ttl"^^xsd:anyURI ;
.

<https://linked.data.gov.au/def/test/dawe-cv/ea88802e-3465-51c8-b437-8da61208a395>
    a skos:Concept ;
    dcterms:identifier 11 ;
    dcterms:source <http://vocabs.paratoo.tern.org.au:1337/api/lut-veg-growth-forms> ;
    rdfs:isDefinedBy <https://linked.data.gov.au/def/nrm> ;
    skos:definition "Herbaceous, usually perennial erect monocot that is neither a grass nor a sedge. For the purposes of NVIS, rushes include the monocotyledon families Juncaceae, Typhaceae, Liliaceae, Iridaceae, Xyridaceae and the genus Lomandra. I.e. \"graminoid\" or grass-like genera." ;
    skos:notation "R" ;
    skos:prefLabel "Rush" ;
    schema:url "https://github.com/ternaustralia/dawe-rlp-vocabs/tree/main/vocab_files/categorical_collections/luts/vegetation-growth-form.ttl"^^xsd:anyURI ;
.

<https://linked.data.gov.au/def/test/dawe-cv/eb5f51a6-0a5c-5e67-883d-35883fcf3ba3>
    a skos:Concept ;
    dcterms:identifier 7 ;
    dcterms:source <http://vocabs.paratoo.tern.org.au:1337/api/lut-veg-growth-forms> ;
    rdfs:isDefinedBy <https://linked.data.gov.au/def/nrm> ;
    skos:definition "Members of the families Cycadaceae and Zamiaceae" ;
    skos:notation "CY" ;
    skos:prefLabel "Cycad" ;
    schema:url "https://github.com/ternaustralia/dawe-rlp-vocabs/tree/main/vocab_files/categorical_collections/luts/vegetation-growth-form.ttl"^^xsd:anyURI ;
.

<https://linked.data.gov.au/def/test/dawe-cv/ef6a07fa-47ce-5cf4-ad06-218556c0dde4>
    a skos:Concept ;
    dcterms:identifier 4 ;
    dcterms:source <http://vocabs.paratoo.tern.org.au:1337/api/lut-veg-growth-forms> ;
    rdfs:isDefinedBy <https://linked.data.gov.au/def/nrm> ;
    skos:definition "Plant growing in an inland waterway or wetland with the majority of its biomass under water for most of the year. Fresh, saline or brackish water." ;
    skos:notation "A" ;
    skos:prefLabel "Aquatic" ;
    schema:url "https://github.com/ternaustralia/dawe-rlp-vocabs/tree/main/vocab_files/categorical_collections/luts/vegetation-growth-form.ttl"^^xsd:anyURI ;
.

