# Do not edit this file directly. This file is generated by `make luts` with endpoints from src/dawe_nrm/api/categorical_values/endpoints.py
PREFIX dcterms: <http://purl.org/dc/terms/>
PREFIX rdfs: <http://www.w3.org/2000/01/rdf-schema#>
PREFIX schema: <https://schema.org/>
PREFIX skos: <http://www.w3.org/2004/02/skos/core#>
PREFIX urnc: <urn:class:>
PREFIX urnp: <urn:property:>
PREFIX xsd: <http://www.w3.org/2001/XMLSchema#>

<https://linked.data.gov.au/def/nrm/1fe9c3c7-c3aa-5378-80f4-871b04bc7973>
    a urnc:CategoricalConceptMeta ;
    schema:url "https://github.com/ternaustralia/dawe-rlp-vocabs/tree/main/vocab_files/categorical_collections/luts/weather-cloud-covers.ttl"^^xsd:anyURI ;
    urnp:categoricalCollection <https://linked.data.gov.au/def/nrm/b001aab8-d5c2-4268-a750-bed499386691> ;
    urnp:categoricalConcept <https://linked.data.gov.au/def/nrm/7773b3e9-83e7-5057-b7d6-6a025e0b6a2b> ;
    urnp:conceptDefinition "Predominantly more clear sky than cloud. Cloud covering ¼ - ¾ of the sky. For example, the sun would be regularly obscured by cloud for short periods of time." ;
    urnp:conceptIdentifier 3 ;
    urnp:conceptNotation "PC" ;
    urnp:conceptSource <https://core.vocabs.paratoo.tern.org.au/api/lut-weather-cloud-covers> ;
.

<https://linked.data.gov.au/def/nrm/1fee9ebd-2af4-554a-ac7e-f3c293da7973>
    a urnc:CategoricalConceptMeta ;
    schema:url "https://github.com/ternaustralia/dawe-rlp-vocabs/tree/main/vocab_files/categorical_collections/luts/weather-cloud-covers.ttl"^^xsd:anyURI ;
    urnp:categoricalCollection <https://linked.data.gov.au/def/nrm/b001aab8-d5c2-4268-a750-bed499386691> ;
    urnp:categoricalConcept <https://linked.data.gov.au/def/nrm/94d0cbdd-9631-5bda-b70e-00b77e80fc8e> ;
    urnp:conceptDefinition "Sky completely covered with cloud. Cloud expected to cover all of the sky." ;
    urnp:conceptIdentifier 5 ;
    urnp:conceptNotation "O" ;
    urnp:conceptSource <https://core.vocabs.paratoo.tern.org.au/api/lut-weather-cloud-covers> ;
.

<https://linked.data.gov.au/def/nrm/7016e976-dc44-53c7-9c39-8803d129e427>
    a urnc:CategoricalConceptMeta ;
    schema:url "https://github.com/ternaustralia/dawe-rlp-vocabs/tree/main/vocab_files/categorical_collections/luts/weather-cloud-covers.ttl"^^xsd:anyURI ;
    urnp:categoricalCollection <https://linked.data.gov.au/def/nrm/b001aab8-d5c2-4268-a750-bed499386691> ;
    urnp:categoricalConcept <https://linked.data.gov.au/def/nrm/bd978c4a-0f90-5863-aa0e-02fa0cc2828a> ;
    urnp:conceptDefinition "Little chance of the sun being obscured by cloud. Cloud covering < ¼ of the sky. Note: High level cirrus clouds are often thin and wispy, allowing a considerable amount of sunlight to penetrate them, sufficient to produce shadows. In this case the day could be termed 'sunny' even though the sky may consist of cirrus cloud." ;
    urnp:conceptIdentifier 1 ;
    urnp:conceptNotation "SU" ;
    urnp:conceptSource <https://core.vocabs.paratoo.tern.org.au/api/lut-weather-cloud-covers> ;
.

<https://linked.data.gov.au/def/nrm/9564cac8-9de0-5ad5-881a-a6da1f17937c>
    a urnc:CategoricalConceptMeta ;
    schema:url "https://github.com/ternaustralia/dawe-rlp-vocabs/tree/main/vocab_files/categorical_collections/luts/weather-cloud-covers.ttl"^^xsd:anyURI ;
    urnp:categoricalCollection <https://linked.data.gov.au/def/nrm/b001aab8-d5c2-4268-a750-bed499386691> ;
    urnp:categoricalConcept <https://linked.data.gov.au/def/nrm/34e20339-1dc9-55f8-b466-a080c969eb70> ;
    urnp:conceptDefinition "Predominantly more cloud than clear sky. Cloud covering ¾ - nearly all of the sky. For example, the sun would be obscured by cloud for substantial periods of time." ;
    urnp:conceptIdentifier 4 ;
    urnp:conceptNotation "C" ;
    urnp:conceptSource <https://core.vocabs.paratoo.tern.org.au/api/lut-weather-cloud-covers> ;
.

<https://linked.data.gov.au/def/nrm/a66a2f92-a4b6-5cad-930a-333751c1bc95>
    a urnc:CategoricalConceptMeta ;
    schema:url "https://github.com/ternaustralia/dawe-rlp-vocabs/tree/main/vocab_files/categorical_collections/luts/weather-cloud-covers.ttl"^^xsd:anyURI ;
    urnp:categoricalCollection <https://linked.data.gov.au/def/nrm/b001aab8-d5c2-4268-a750-bed499386691> ;
    urnp:categoricalConcept <https://linked.data.gov.au/def/nrm/449a90bc-53c3-5aab-b259-89a39c278d33> ;
    urnp:conceptDefinition "Predominantly more clear sky than cloud. Cloud covering ¼ of the sky. For example, the sun would be obscured by cloud for short periods of time.Predominantly more clear sky than cloud. Cloud covering ¼ of the sky. For example, the sun would be obscured by cloud for short periods of time." ;
    urnp:conceptIdentifier 2 ;
    urnp:conceptNotation "MS" ;
    urnp:conceptSource <https://core.vocabs.paratoo.tern.org.au/api/lut-weather-cloud-covers> ;
.

<https://linked.data.gov.au/def/nrm/34e20339-1dc9-55f8-b466-a080c969eb70>
    a skos:Concept ;
    dcterms:identifier 4 ;
    dcterms:source <https://core.vocabs.paratoo.tern.org.au/api/lut-weather-cloud-covers> ;
    rdfs:isDefinedBy <https://linked.data.gov.au/def/nrm> ;
    skos:definition "Predominantly more cloud than clear sky. Cloud covering ¾ - nearly all of the sky. For example, the sun would be obscured by cloud for substantial periods of time." ;
    skos:notation "C" ;
    skos:prefLabel "Cloudy" ;
    schema:url "https://github.com/ternaustralia/dawe-rlp-vocabs/tree/main/vocab_files/categorical_collections/luts/weather-cloud-covers.ttl"^^xsd:anyURI ;
.

<https://linked.data.gov.au/def/nrm/449a90bc-53c3-5aab-b259-89a39c278d33>
    a skos:Concept ;
    dcterms:identifier 2 ;
    dcterms:source <https://core.vocabs.paratoo.tern.org.au/api/lut-weather-cloud-covers> ;
    rdfs:isDefinedBy <https://linked.data.gov.au/def/nrm> ;
    skos:definition "Predominantly more clear sky than cloud. Cloud covering ¼ of the sky. For example, the sun would be obscured by cloud for short periods of time.Predominantly more clear sky than cloud. Cloud covering ¼ of the sky. For example, the sun would be obscured by cloud for short periods of time." ;
    skos:notation "MS" ;
    skos:prefLabel "Mostly Sunny" ;
    schema:url "https://github.com/ternaustralia/dawe-rlp-vocabs/tree/main/vocab_files/categorical_collections/luts/weather-cloud-covers.ttl"^^xsd:anyURI ;
.

<https://linked.data.gov.au/def/nrm/7773b3e9-83e7-5057-b7d6-6a025e0b6a2b>
    a skos:Concept ;
    dcterms:identifier 3 ;
    dcterms:source <https://core.vocabs.paratoo.tern.org.au/api/lut-weather-cloud-covers> ;
    rdfs:isDefinedBy <https://linked.data.gov.au/def/nrm> ;
    skos:definition "Predominantly more clear sky than cloud. Cloud covering ¼ - ¾ of the sky. For example, the sun would be regularly obscured by cloud for short periods of time." ;
    skos:notation "PC" ;
    skos:prefLabel "Partly Cloudy" ;
    schema:url "https://github.com/ternaustralia/dawe-rlp-vocabs/tree/main/vocab_files/categorical_collections/luts/weather-cloud-covers.ttl"^^xsd:anyURI ;
.

<https://linked.data.gov.au/def/nrm/94d0cbdd-9631-5bda-b70e-00b77e80fc8e>
    a skos:Concept ;
    dcterms:identifier 5 ;
    dcterms:source <https://core.vocabs.paratoo.tern.org.au/api/lut-weather-cloud-covers> ;
    rdfs:isDefinedBy <https://linked.data.gov.au/def/nrm> ;
    skos:definition "Sky completely covered with cloud. Cloud expected to cover all of the sky." ;
    skos:notation "O" ;
    skos:prefLabel "Overcast" ;
    schema:url "https://github.com/ternaustralia/dawe-rlp-vocabs/tree/main/vocab_files/categorical_collections/luts/weather-cloud-covers.ttl"^^xsd:anyURI ;
.

<https://linked.data.gov.au/def/nrm/bd978c4a-0f90-5863-aa0e-02fa0cc2828a>
    a skos:Concept ;
    dcterms:identifier 1 ;
    dcterms:source <https://core.vocabs.paratoo.tern.org.au/api/lut-weather-cloud-covers> ;
    rdfs:isDefinedBy <https://linked.data.gov.au/def/nrm> ;
    skos:definition "Little chance of the sun being obscured by cloud. Cloud covering < ¼ of the sky. Note: High level cirrus clouds are often thin and wispy, allowing a considerable amount of sunlight to penetrate them, sufficient to produce shadows. In this case the day could be termed 'sunny' even though the sky may consist of cirrus cloud." ;
    skos:notation "SU" ;
    skos:prefLabel "Sunny" ;
    schema:url "https://github.com/ternaustralia/dawe-rlp-vocabs/tree/main/vocab_files/categorical_collections/luts/weather-cloud-covers.ttl"^^xsd:anyURI ;
.

<https://linked.data.gov.au/def/nrm/b001aab8-d5c2-4268-a750-bed499386691>
    a skos:Collection ;
    dcterms:description "A collection of weather cloud covers and its codes." ;
    dcterms:source <https://core.vocabs.paratoo.tern.org.au/api/lut-weather-cloud-covers> ;
    rdfs:isDefinedBy <https://linked.data.gov.au/def/nrm> ;
    skos:member
        <https://linked.data.gov.au/def/nrm/34e20339-1dc9-55f8-b466-a080c969eb70> ,
        <https://linked.data.gov.au/def/nrm/449a90bc-53c3-5aab-b259-89a39c278d33> ,
        <https://linked.data.gov.au/def/nrm/7773b3e9-83e7-5057-b7d6-6a025e0b6a2b> ,
        <https://linked.data.gov.au/def/nrm/94d0cbdd-9631-5bda-b70e-00b77e80fc8e> ,
        <https://linked.data.gov.au/def/nrm/bd978c4a-0f90-5863-aa0e-02fa0cc2828a> ;
    skos:prefLabel "Weather cloud covers codes" ;
    schema:url "https://github.com/ternaustralia/dawe-rlp-vocabs/tree/main/vocab_files/categorical_collections/luts/weather-cloud-covers.ttl"^^xsd:anyURI ;
.

